<?xml version="1.0"?>
<rdf:RDF xmlns="http://www.semanticweb.org/suhaspai/ontologies/2021/4/untitled-ontology-14"
     xml:base="http://www.semanticweb.org/suhaspai/ontologies/2021/4/untitled-ontology-14"
     xmlns:owl="http://www.w3.org/2002/07/owl#"
     xmlns:rdf="http://www.w3.org/1999/02/22-rdf-syntax-ns#"
     xmlns:xml="http://www.w3.org/XML/1998/namespace"
     xmlns:xsd="http://www.w3.org/2001/XMLSchema#"
     xmlns:rdfs="http://www.w3.org/2000/01/rdf-schema#"
     xmlns:UnivFAQ="http://www.semanticweb.org/suhaspai/ontologies/2021/4/UnivFAQ#">
    <owl:Ontology rdf:about="http://www.semanticweb.org/suhaspai/ontologies/2021/4/UnivFAQ"/>
    


    <!-- 
    ///////////////////////////////////////////////////////////////////////////////////////
    //
    // Object Properties
    //
    ///////////////////////////////////////////////////////////////////////////////////////
     -->

    


    <!-- http://www.semanticweb.org/suhaspai/ontologies/2021/4/UnivFAQ#advises -->

    <owl:ObjectProperty rdf:about="http://www.semanticweb.org/suhaspai/ontologies/2021/4/UnivFAQ#advises">
        <owl:inverseOf rdf:resource="http://www.semanticweb.org/suhaspai/ontologies/2021/4/UnivFAQ#isAdvisedBy"/>
        <rdfs:domain rdf:resource="http://www.semanticweb.org/suhaspai/ontologies/2021/4/UnivFAQ#Person"/>
        <rdfs:range rdf:resource="http://www.semanticweb.org/suhaspai/ontologies/2021/4/UnivFAQ#Person"/>
    </owl:ObjectProperty>
    


    <!-- http://www.semanticweb.org/suhaspai/ontologies/2021/4/UnivFAQ#belongsTo -->

    <owl:ObjectProperty rdf:about="http://www.semanticweb.org/suhaspai/ontologies/2021/4/UnivFAQ#belongsTo">
        <rdfs:domain rdf:resource="http://www.semanticweb.org/suhaspai/ontologies/2021/4/UnivFAQ#Professors"/>
        <rdfs:range rdf:resource="http://www.semanticweb.org/suhaspai/ontologies/2021/4/UnivFAQ#Department"/>
    </owl:ObjectProperty>
    


    <!-- http://www.semanticweb.org/suhaspai/ontologies/2021/4/UnivFAQ#enrolledIn -->

    <owl:ObjectProperty rdf:about="http://www.semanticweb.org/suhaspai/ontologies/2021/4/UnivFAQ#enrolledIn">
        <rdfs:domain rdf:resource="http://www.semanticweb.org/suhaspai/ontologies/2021/4/UnivFAQ#Student"/>
        <rdfs:range rdf:resource="http://www.semanticweb.org/suhaspai/ontologies/2021/4/UnivFAQ#Programs"/>
    </owl:ObjectProperty>
    


    <!-- http://www.semanticweb.org/suhaspai/ontologies/2021/4/UnivFAQ#hasAdmissionRequisites -->

    <owl:ObjectProperty rdf:about="http://www.semanticweb.org/suhaspai/ontologies/2021/4/UnivFAQ#hasAdmissionRequisites">
        <rdfs:domain rdf:resource="http://www.semanticweb.org/suhaspai/ontologies/2021/4/UnivFAQ#Programs"/>
        <rdfs:range>
            <owl:Class>
                <owl:unionOf rdf:parseType="Collection">
                    <rdf:Description rdf:about="http://www.semanticweb.org/suhaspai/ontologies/2021/4/UnivFAQ#Qualifications"/>
                    <rdf:Description rdf:about="http://www.semanticweb.org/suhaspai/ontologies/2021/4/UnivFAQ#StandardizedTests"/>
                </owl:unionOf>
            </owl:Class>
        </rdfs:range>
    </owl:ObjectProperty>
    


    <!-- http://www.semanticweb.org/suhaspai/ontologies/2021/4/UnivFAQ#hasFacility -->

    <owl:ObjectProperty rdf:about="http://www.semanticweb.org/suhaspai/ontologies/2021/4/UnivFAQ#hasFacility">
        <rdfs:domain rdf:resource="http://www.semanticweb.org/suhaspai/ontologies/2021/4/UnivFAQ#Department"/>
        <rdfs:range rdf:resource="http://www.semanticweb.org/suhaspai/ontologies/2021/4/UnivFAQ#InstituteFacilities"/>
    </owl:ObjectProperty>
    


    <!-- http://www.semanticweb.org/suhaspai/ontologies/2021/4/UnivFAQ#hasMinimumCriterion -->

    <owl:ObjectProperty rdf:about="http://www.semanticweb.org/suhaspai/ontologies/2021/4/UnivFAQ#hasMinimumCriterion">
        <rdfs:domain rdf:resource="http://www.semanticweb.org/suhaspai/ontologies/2021/4/UnivFAQ#Programs"/>
        <rdfs:range rdf:resource="http://www.semanticweb.org/suhaspai/ontologies/2021/4/UnivFAQ#Qualifications"/>
    </owl:ObjectProperty>
    


    <!-- http://www.semanticweb.org/suhaspai/ontologies/2021/4/UnivFAQ#hasPrerequisite -->

    <owl:ObjectProperty rdf:about="http://www.semanticweb.org/suhaspai/ontologies/2021/4/UnivFAQ#hasPrerequisite">
        <owl:inverseOf rdf:resource="http://www.semanticweb.org/suhaspai/ontologies/2021/4/UnivFAQ#isPrerequisiteFor"/>
        <rdf:type rdf:resource="http://www.w3.org/2002/07/owl#TransitiveProperty"/>
    </owl:ObjectProperty>
    


    <!-- http://www.semanticweb.org/suhaspai/ontologies/2021/4/UnivFAQ#hasPublication -->

    <owl:ObjectProperty rdf:about="http://www.semanticweb.org/suhaspai/ontologies/2021/4/UnivFAQ#hasPublication">
        <owl:inverseOf rdf:resource="http://www.semanticweb.org/suhaspai/ontologies/2021/4/UnivFAQ#inResearchField"/>
        <rdfs:domain rdf:resource="http://www.semanticweb.org/suhaspai/ontologies/2021/4/UnivFAQ#ResearchFields"/>
        <rdfs:range rdf:resource="http://www.semanticweb.org/suhaspai/ontologies/2021/4/UnivFAQ#Publication"/>
    </owl:ObjectProperty>
    


    <!-- http://www.semanticweb.org/suhaspai/ontologies/2021/4/UnivFAQ#hasPublished -->

    <owl:ObjectProperty rdf:about="http://www.semanticweb.org/suhaspai/ontologies/2021/4/UnivFAQ#hasPublished">
        <owl:inverseOf rdf:resource="http://www.semanticweb.org/suhaspai/ontologies/2021/4/UnivFAQ#publishedBy"/>
        <rdfs:domain rdf:resource="http://www.semanticweb.org/suhaspai/ontologies/2021/4/UnivFAQ#Professors"/>
        <rdfs:range rdf:resource="http://www.semanticweb.org/suhaspai/ontologies/2021/4/UnivFAQ#Publication"/>
    </owl:ObjectProperty>
    


    <!-- http://www.semanticweb.org/suhaspai/ontologies/2021/4/UnivFAQ#hasScholarship -->

    <owl:ObjectProperty rdf:about="http://www.semanticweb.org/suhaspai/ontologies/2021/4/UnivFAQ#hasScholarship">
        <rdfs:domain rdf:resource="http://www.semanticweb.org/suhaspai/ontologies/2021/4/UnivFAQ#Programs"/>
        <rdfs:range rdf:resource="http://www.semanticweb.org/suhaspai/ontologies/2021/4/UnivFAQ#FinancialScholarship"/>
    </owl:ObjectProperty>
    


    <!-- http://www.semanticweb.org/suhaspai/ontologies/2021/4/UnivFAQ#headsDepartment -->

    <owl:ObjectProperty rdf:about="http://www.semanticweb.org/suhaspai/ontologies/2021/4/UnivFAQ#headsDepartment">
        <rdfs:domain rdf:resource="http://www.semanticweb.org/suhaspai/ontologies/2021/4/UnivFAQ#Professors"/>
        <rdfs:range rdf:resource="http://www.semanticweb.org/suhaspai/ontologies/2021/4/UnivFAQ#Department"/>
    </owl:ObjectProperty>
    


    <!-- http://www.semanticweb.org/suhaspai/ontologies/2021/4/UnivFAQ#inResearchField -->

    <owl:ObjectProperty rdf:about="http://www.semanticweb.org/suhaspai/ontologies/2021/4/UnivFAQ#inResearchField"/>
    


    <!-- http://www.semanticweb.org/suhaspai/ontologies/2021/4/UnivFAQ#isAdvisedBy -->

    <owl:ObjectProperty rdf:about="http://www.semanticweb.org/suhaspai/ontologies/2021/4/UnivFAQ#isAdvisedBy"/>
    


    <!-- http://www.semanticweb.org/suhaspai/ontologies/2021/4/UnivFAQ#isPrerequisiteFor -->

    <owl:ObjectProperty rdf:about="http://www.semanticweb.org/suhaspai/ontologies/2021/4/UnivFAQ#isPrerequisiteFor">
        <rdf:type rdf:resource="http://www.w3.org/2002/07/owl#TransitiveProperty"/>
        <rdfs:domain rdf:resource="http://www.semanticweb.org/suhaspai/ontologies/2021/4/UnivFAQ#Courses"/>
        <rdfs:range rdf:resource="http://www.semanticweb.org/suhaspai/ontologies/2021/4/UnivFAQ#Courses"/>
    </owl:ObjectProperty>
    


    <!-- http://www.semanticweb.org/suhaspai/ontologies/2021/4/UnivFAQ#isSpecializedIn -->

    <owl:ObjectProperty rdf:about="http://www.semanticweb.org/suhaspai/ontologies/2021/4/UnivFAQ#isSpecializedIn">
        <rdfs:domain rdf:resource="http://www.semanticweb.org/suhaspai/ontologies/2021/4/UnivFAQ#Professors"/>
        <rdfs:range rdf:resource="http://www.semanticweb.org/suhaspai/ontologies/2021/4/UnivFAQ#ResearchFields"/>
    </owl:ObjectProperty>
    


    <!-- http://www.semanticweb.org/suhaspai/ontologies/2021/4/UnivFAQ#offeredBy -->

    <owl:ObjectProperty rdf:about="http://www.semanticweb.org/suhaspai/ontologies/2021/4/UnivFAQ#offeredBy">
        <owl:inverseOf rdf:resource="http://www.semanticweb.org/suhaspai/ontologies/2021/4/UnivFAQ#offers"/>
    </owl:ObjectProperty>
    


    <!-- http://www.semanticweb.org/suhaspai/ontologies/2021/4/UnivFAQ#offers -->

    <owl:ObjectProperty rdf:about="http://www.semanticweb.org/suhaspai/ontologies/2021/4/UnivFAQ#offers">
        <rdfs:domain rdf:resource="http://www.semanticweb.org/suhaspai/ontologies/2021/4/UnivFAQ#Department"/>
        <rdfs:range>
            <owl:Class>
                <owl:unionOf rdf:parseType="Collection">
                    <rdf:Description rdf:about="http://www.semanticweb.org/suhaspai/ontologies/2021/4/UnivFAQ#Courses"/>
                    <rdf:Description rdf:about="http://www.semanticweb.org/suhaspai/ontologies/2021/4/UnivFAQ#Programs"/>
                </owl:unionOf>
            </owl:Class>
        </rdfs:range>
    </owl:ObjectProperty>
    


    <!-- http://www.semanticweb.org/suhaspai/ontologies/2021/4/UnivFAQ#publishedBy -->

    <owl:ObjectProperty rdf:about="http://www.semanticweb.org/suhaspai/ontologies/2021/4/UnivFAQ#publishedBy"/>
    


    <!-- http://www.semanticweb.org/suhaspai/ontologies/2021/4/UnivFAQ#requiredForMajor -->

    <owl:ObjectProperty rdf:about="http://www.semanticweb.org/suhaspai/ontologies/2021/4/UnivFAQ#requiredForMajor">
        <rdfs:domain rdf:resource="http://www.semanticweb.org/suhaspai/ontologies/2021/4/UnivFAQ#Programs"/>
        <rdfs:range rdf:resource="http://www.semanticweb.org/suhaspai/ontologies/2021/4/UnivFAQ#Courses"/>
    </owl:ObjectProperty>
    


    <!-- http://www.semanticweb.org/suhaspai/ontologies/2021/4/UnivFAQ#requiredForMinor -->

    <owl:ObjectProperty rdf:about="http://www.semanticweb.org/suhaspai/ontologies/2021/4/UnivFAQ#requiredForMinor"/>
    


    <!-- http://www.semanticweb.org/suhaspai/ontologies/2021/4/UnivFAQ#taughtBy -->

    <owl:ObjectProperty rdf:about="http://www.semanticweb.org/suhaspai/ontologies/2021/4/UnivFAQ#taughtBy">
        <owl:inverseOf rdf:resource="http://www.semanticweb.org/suhaspai/ontologies/2021/4/UnivFAQ#teaches"/>
    </owl:ObjectProperty>
    


    <!-- http://www.semanticweb.org/suhaspai/ontologies/2021/4/UnivFAQ#teaches -->

    <owl:ObjectProperty rdf:about="http://www.semanticweb.org/suhaspai/ontologies/2021/4/UnivFAQ#teaches">
        <rdfs:domain rdf:resource="http://www.semanticweb.org/suhaspai/ontologies/2021/4/UnivFAQ#Professors"/>
        <rdfs:range rdf:resource="http://www.semanticweb.org/suhaspai/ontologies/2021/4/UnivFAQ#Courses"/>
    </owl:ObjectProperty>
    


    <!-- 
    ///////////////////////////////////////////////////////////////////////////////////////
    //
    // Data properties
    //
    ///////////////////////////////////////////////////////////////////////////////////////
     -->

    


    <!-- http://www.semanticweb.org/suhaspai/ontologies/2021/4/UnivFAQ#name -->

    <owl:DatatypeProperty rdf:about="http://www.semanticweb.org/suhaspai/ontologies/2021/4/UnivFAQ#name">
        <rdf:type rdf:resource="http://www.w3.org/2002/07/owl#FunctionalProperty"/>
        <rdfs:domain>
            <owl:Class>
                <owl:unionOf rdf:parseType="Collection">
                    <rdf:Description rdf:about="http://www.semanticweb.org/suhaspai/ontologies/2021/4/UnivFAQ#Courses"/>
                    <rdf:Description rdf:about="http://www.semanticweb.org/suhaspai/ontologies/2021/4/UnivFAQ#Department"/>
                    <rdf:Description rdf:about="http://www.semanticweb.org/suhaspai/ontologies/2021/4/UnivFAQ#Professors"/>
                    <rdf:Description rdf:about="http://www.semanticweb.org/suhaspai/ontologies/2021/4/UnivFAQ#Programs"/>
                    <rdf:Description rdf:about="http://www.semanticweb.org/suhaspai/ontologies/2021/4/UnivFAQ#Student"/>
                </owl:unionOf>
            </owl:Class>
        </rdfs:domain>
        <rdfs:range rdf:resource="http://www.w3.org/2001/XMLSchema#string"/>
    </owl:DatatypeProperty>
    


    <!-- http://www.semanticweb.org/suhaspai/ontologies/2021/4/UnivFAQ#testProp -->

    <owl:DatatypeProperty rdf:about="http://www.semanticweb.org/suhaspai/ontologies/2021/4/UnivFAQ#testProp">
        <rdf:type rdf:resource="http://www.w3.org/2002/07/owl#FunctionalProperty"/>
        <rdfs:domain>
            <owl:Class>
                <owl:unionOf rdf:parseType="Collection">
                    <rdf:Description rdf:about="http://www.semanticweb.org/suhaspai/ontologies/2021/4/UnivFAQ#Courses"/>
                    <rdf:Description rdf:about="http://www.semanticweb.org/suhaspai/ontologies/2021/4/UnivFAQ#Professors"/>
                </owl:unionOf>
            </owl:Class>
        </rdfs:domain>
        <rdfs:range rdf:resource="http://www.w3.org/2001/XMLSchema#string"/>
    </owl:DatatypeProperty>
    


    <!-- 
    ///////////////////////////////////////////////////////////////////////////////////////
    //
    // Classes
    //
    ///////////////////////////////////////////////////////////////////////////////////////
     -->

    


    <!-- http://www.semanticweb.org/suhaspai/ontologies/2021/4/UnivFAQ#AdminStaff -->

    <owl:Class rdf:about="http://www.semanticweb.org/suhaspai/ontologies/2021/4/UnivFAQ#AdminStaff">
        <rdfs:subClassOf rdf:resource="http://www.semanticweb.org/suhaspai/ontologies/2021/4/UnivFAQ#Person"/>
    </owl:Class>
    


    <!-- http://www.semanticweb.org/suhaspai/ontologies/2021/4/UnivFAQ#Alumni -->

    <owl:Class rdf:about="http://www.semanticweb.org/suhaspai/ontologies/2021/4/UnivFAQ#Alumni">
        <rdfs:subClassOf rdf:resource="http://www.semanticweb.org/suhaspai/ontologies/2021/4/UnivFAQ#Person"/>
    </owl:Class>
    


    <!-- http://www.semanticweb.org/suhaspai/ontologies/2021/4/UnivFAQ#AssistantProfessor -->

    <owl:Class rdf:about="http://www.semanticweb.org/suhaspai/ontologies/2021/4/UnivFAQ#AssistantProfessor">
        <rdfs:subClassOf rdf:resource="http://www.semanticweb.org/suhaspai/ontologies/2021/4/UnivFAQ#Professors"/>
    </owl:Class>
    


    <!-- http://www.semanticweb.org/suhaspai/ontologies/2021/4/UnivFAQ#AssociateProfessor -->

    <owl:Class rdf:about="http://www.semanticweb.org/suhaspai/ontologies/2021/4/UnivFAQ#AssociateProfessor">
        <rdfs:subClassOf rdf:resource="http://www.semanticweb.org/suhaspai/ontologies/2021/4/UnivFAQ#Professors"/>
    </owl:Class>
    


    <!-- http://www.semanticweb.org/suhaspai/ontologies/2021/4/UnivFAQ#BTech. -->

    <owl:Class rdf:about="http://www.semanticweb.org/suhaspai/ontologies/2021/4/UnivFAQ#BTech.">
        <rdfs:subClassOf rdf:resource="http://www.semanticweb.org/suhaspai/ontologies/2021/4/UnivFAQ#UndergradPrograms"/>
    </owl:Class>
    


    <!-- http://www.semanticweb.org/suhaspai/ontologies/2021/4/UnivFAQ#Courses -->

    <owl:Class rdf:about="http://www.semanticweb.org/suhaspai/ontologies/2021/4/UnivFAQ#Courses"/>
    


    <!-- http://www.semanticweb.org/suhaspai/ontologies/2021/4/UnivFAQ#Department -->

    <owl:Class rdf:about="http://www.semanticweb.org/suhaspai/ontologies/2021/4/UnivFAQ#Department"/>
    


    <!-- http://www.semanticweb.org/suhaspai/ontologies/2021/4/UnivFAQ#Dual_Degree -->

    <owl:Class rdf:about="http://www.semanticweb.org/suhaspai/ontologies/2021/4/UnivFAQ#Dual_Degree">
        <rdfs:subClassOf rdf:resource="http://www.semanticweb.org/suhaspai/ontologies/2021/4/UnivFAQ#UndergradPrograms"/>
    </owl:Class>
    


    <!-- http://www.semanticweb.org/suhaspai/ontologies/2021/4/UnivFAQ#FinancialScholarship -->

    <owl:Class rdf:about="http://www.semanticweb.org/suhaspai/ontologies/2021/4/UnivFAQ#FinancialScholarship"/>
    


    <!-- http://www.semanticweb.org/suhaspai/ontologies/2021/4/UnivFAQ#InstituteFacilities -->

    <owl:Class rdf:about="http://www.semanticweb.org/suhaspai/ontologies/2021/4/UnivFAQ#InstituteFacilities"/>
    


    <!-- http://www.semanticweb.org/suhaspai/ontologies/2021/4/UnivFAQ#MS -->

    <owl:Class rdf:about="http://www.semanticweb.org/suhaspai/ontologies/2021/4/UnivFAQ#MS">
        <rdfs:subClassOf rdf:resource="http://www.semanticweb.org/suhaspai/ontologies/2021/4/UnivFAQ#PostgradPrograms"/>
    </owl:Class>
    


    <!-- http://www.semanticweb.org/suhaspai/ontologies/2021/4/UnivFAQ#MTech. -->

    <owl:Class rdf:about="http://www.semanticweb.org/suhaspai/ontologies/2021/4/UnivFAQ#MTech.">
        <rdfs:subClassOf rdf:resource="http://www.semanticweb.org/suhaspai/ontologies/2021/4/UnivFAQ#PostgradPrograms"/>
    </owl:Class>
    


    <!-- http://www.semanticweb.org/suhaspai/ontologies/2021/4/UnivFAQ#Person -->

    <owl:Class rdf:about="http://www.semanticweb.org/suhaspai/ontologies/2021/4/UnivFAQ#Person"/>
    


    <!-- http://www.semanticweb.org/suhaspai/ontologies/2021/4/UnivFAQ#PhD -->

    <owl:Class rdf:about="http://www.semanticweb.org/suhaspai/ontologies/2021/4/UnivFAQ#PhD">
        <rdfs:subClassOf rdf:resource="http://www.semanticweb.org/suhaspai/ontologies/2021/4/UnivFAQ#PostgradPrograms"/>
    </owl:Class>
    


    <!-- http://www.semanticweb.org/suhaspai/ontologies/2021/4/UnivFAQ#PostgradCourses -->

    <owl:Class rdf:about="http://www.semanticweb.org/suhaspai/ontologies/2021/4/UnivFAQ#PostgradCourses">
        <rdfs:subClassOf rdf:resource="http://www.semanticweb.org/suhaspai/ontologies/2021/4/UnivFAQ#Courses"/>
    </owl:Class>
    


    <!-- http://www.semanticweb.org/suhaspai/ontologies/2021/4/UnivFAQ#PostgradPrograms -->

    <owl:Class rdf:about="http://www.semanticweb.org/suhaspai/ontologies/2021/4/UnivFAQ#PostgradPrograms">
        <rdfs:subClassOf rdf:resource="http://www.semanticweb.org/suhaspai/ontologies/2021/4/UnivFAQ#Programs"/>
    </owl:Class>
    


    <!-- http://www.semanticweb.org/suhaspai/ontologies/2021/4/UnivFAQ#Professor -->

    <owl:Class rdf:about="http://www.semanticweb.org/suhaspai/ontologies/2021/4/UnivFAQ#Professor">
        <rdfs:subClassOf rdf:resource="http://www.semanticweb.org/suhaspai/ontologies/2021/4/UnivFAQ#Professors"/>
    </owl:Class>
    


    <!-- http://www.semanticweb.org/suhaspai/ontologies/2021/4/UnivFAQ#Professors -->

    <owl:Class rdf:about="http://www.semanticweb.org/suhaspai/ontologies/2021/4/UnivFAQ#Professors">
        <rdfs:subClassOf rdf:resource="http://www.semanticweb.org/suhaspai/ontologies/2021/4/UnivFAQ#Person"/>
    </owl:Class>
    


    <!-- http://www.semanticweb.org/suhaspai/ontologies/2021/4/UnivFAQ#Programs -->

    <owl:Class rdf:about="http://www.semanticweb.org/suhaspai/ontologies/2021/4/UnivFAQ#Programs"/>
    


    <!-- http://www.semanticweb.org/suhaspai/ontologies/2021/4/UnivFAQ#Publication -->

    <owl:Class rdf:about="http://www.semanticweb.org/suhaspai/ontologies/2021/4/UnivFAQ#Publication"/>
    


    <!-- http://www.semanticweb.org/suhaspai/ontologies/2021/4/UnivFAQ#Qualifications -->

    <owl:Class rdf:about="http://www.semanticweb.org/suhaspai/ontologies/2021/4/UnivFAQ#Qualifications"/>
    


    <!-- http://www.semanticweb.org/suhaspai/ontologies/2021/4/UnivFAQ#ResearchFields -->

    <owl:Class rdf:about="http://www.semanticweb.org/suhaspai/ontologies/2021/4/UnivFAQ#ResearchFields"/>
    


    <!-- http://www.semanticweb.org/suhaspai/ontologies/2021/4/UnivFAQ#ResearchStudents -->

    <owl:Class rdf:about="http://www.semanticweb.org/suhaspai/ontologies/2021/4/UnivFAQ#ResearchStudents">
        <owl:equivalentClass>
            <owl:Class>
                <owl:intersectionOf rdf:parseType="Collection">
                    <rdf:Description rdf:about="http://www.semanticweb.org/suhaspai/ontologies/2021/4/UnivFAQ#Student"/>
                    <owl:Restriction>
                        <owl:onProperty rdf:resource="http://www.semanticweb.org/suhaspai/ontologies/2021/4/UnivFAQ#isAdvisedBy"/>
                        <owl:someValuesFrom rdf:resource="http://www.semanticweb.org/suhaspai/ontologies/2021/4/UnivFAQ#Professors"/>
                    </owl:Restriction>
                </owl:intersectionOf>
            </owl:Class>
        </owl:equivalentClass>
    </owl:Class>
    


    <!-- http://www.semanticweb.org/suhaspai/ontologies/2021/4/UnivFAQ#StandardizedTests -->

    <owl:Class rdf:about="http://www.semanticweb.org/suhaspai/ontologies/2021/4/UnivFAQ#StandardizedTests"/>
    


    <!-- http://www.semanticweb.org/suhaspai/ontologies/2021/4/UnivFAQ#Student -->

    <owl:Class rdf:about="http://www.semanticweb.org/suhaspai/ontologies/2021/4/UnivFAQ#Student">
        <rdfs:subClassOf rdf:resource="http://www.semanticweb.org/suhaspai/ontologies/2021/4/UnivFAQ#Person"/>
        <rdfs:subClassOf>
            <owl:Restriction>
                <owl:onProperty rdf:resource="http://www.semanticweb.org/suhaspai/ontologies/2021/4/UnivFAQ#enrolledIn"/>
                <owl:someValuesFrom rdf:resource="http://www.semanticweb.org/suhaspai/ontologies/2021/4/UnivFAQ#Programs"/>
            </owl:Restriction>
        </rdfs:subClassOf>
    </owl:Class>
    


    <!-- http://www.semanticweb.org/suhaspai/ontologies/2021/4/UnivFAQ#UndergradCourses -->

    <owl:Class rdf:about="http://www.semanticweb.org/suhaspai/ontologies/2021/4/UnivFAQ#UndergradCourses">
        <rdfs:subClassOf rdf:resource="http://www.semanticweb.org/suhaspai/ontologies/2021/4/UnivFAQ#Courses"/>
    </owl:Class>
    


    <!-- http://www.semanticweb.org/suhaspai/ontologies/2021/4/UnivFAQ#UndergradPrograms -->

    <owl:Class rdf:about="http://www.semanticweb.org/suhaspai/ontologies/2021/4/UnivFAQ#UndergradPrograms">
        <rdfs:subClassOf rdf:resource="http://www.semanticweb.org/suhaspai/ontologies/2021/4/UnivFAQ#Programs"/>
    </owl:Class>
    


    <!-- http://www.semanticweb.org/suhaspai/ontologies/2021/4/UnivFAQ#VistingProfessor -->

    <owl:Class rdf:about="http://www.semanticweb.org/suhaspai/ontologies/2021/4/UnivFAQ#VistingProfessor">
        <rdfs:subClassOf rdf:resource="http://www.semanticweb.org/suhaspai/ontologies/2021/4/UnivFAQ#Professors"/>
    </owl:Class>
    


    <!-- 
    ///////////////////////////////////////////////////////////////////////////////////////
    //
    // Individuals
    //
    ///////////////////////////////////////////////////////////////////////////////////////
     -->

    


    <!-- http://www.semanticweb.org/suhaspai/ontologies/2021/4/UnivFAQ#AIDB_Lab -->

    <owl:NamedIndividual rdf:about="http://www.semanticweb.org/suhaspai/ontologies/2021/4/UnivFAQ#AIDB_Lab">
        <rdf:type rdf:resource="http://www.semanticweb.org/suhaspai/ontologies/2021/4/UnivFAQ#InstituteFacilities"/>
        <rdfs:comment>Artificial Intelligence and Databases</rdfs:comment>
        <rdfs:label>AIDB Lab</rdfs:label>
    </owl:NamedIndividual>
    


    <!-- http://www.semanticweb.org/suhaspai/ontologies/2021/4/UnivFAQ#A_Differentially_Private_Stochastic_Gradient_Descent_Algorithm_for_Multiparty_Classification -->

    <owl:NamedIndividual rdf:about="http://www.semanticweb.org/suhaspai/ontologies/2021/4/UnivFAQ#A_Differentially_Private_Stochastic_Gradient_Descent_Algorithm_for_Multiparty_Classification">
        <rdf:type rdf:resource="http://www.semanticweb.org/suhaspai/ontologies/2021/4/UnivFAQ#Publication"/>
        <UnivFAQ:inResearchField rdf:resource="http://www.semanticweb.org/suhaspai/ontologies/2021/4/UnivFAQ#Artificial_Intelligence"/>
        <UnivFAQ:publishedBy rdf:resource="http://www.semanticweb.org/suhaspai/ontologies/2021/4/UnivFAQ#Arun_Rajkumar"/>
        <rdfs:label>A Differentially Private Stochastic Gradient Descent Algorithm for Multiparty Classification</rdfs:label>
    </owl:NamedIndividual>
    


    <!-- http://www.semanticweb.org/suhaspai/ontologies/2021/4/UnivFAQ#A_Newtonian_rheological_model_for_the_interface_of_microbubble_contrast_agents -->

    <owl:NamedIndividual rdf:about="http://www.semanticweb.org/suhaspai/ontologies/2021/4/UnivFAQ#A_Newtonian_rheological_model_for_the_interface_of_microbubble_contrast_agents">
        <rdf:type rdf:resource="http://www.semanticweb.org/suhaspai/ontologies/2021/4/UnivFAQ#Publication"/>
        <UnivFAQ:inResearchField rdf:resource="http://www.semanticweb.org/suhaspai/ontologies/2021/4/UnivFAQ#Fluid_Mechanics"/>
        <UnivFAQ:publishedBy rdf:resource="http://www.semanticweb.org/suhaspai/ontologies/2021/4/UnivFAQ#Dhiman_Chatterjee"/>
        <rdfs:label>A Newtonian rheological model for the interface of microbubble contrast agents</rdfs:label>
    </owl:NamedIndividual>
    


    <!-- http://www.semanticweb.org/suhaspai/ontologies/2021/4/UnivFAQ#A_Seshadri_Sekhar -->

    <owl:NamedIndividual rdf:about="http://www.semanticweb.org/suhaspai/ontologies/2021/4/UnivFAQ#A_Seshadri_Sekhar">
        <rdf:type rdf:resource="http://www.semanticweb.org/suhaspai/ontologies/2021/4/UnivFAQ#Professor"/>
        <UnivFAQ:headsDepartment rdf:resource="http://www.semanticweb.org/suhaspai/ontologies/2021/4/UnivFAQ#Mechanical_Engineering"/>
        <UnivFAQ:isSpecializedIn rdf:resource="http://www.semanticweb.org/suhaspai/ontologies/2021/4/UnivFAQ#Rotordynamics"/>
        <UnivFAQ:teaches rdf:resource="http://www.semanticweb.org/suhaspai/ontologies/2021/4/UnivFAQ#ME2200"/>
        <UnivFAQ:name rdf:datatype="http://www.w3.org/2001/XMLSchema#string">A Seshadri Sekhar</UnivFAQ:name>
        <rdfs:label rdf:datatype="http://www.w3.org/2001/XMLSchema#string">A Seshadri Sekhar</rdfs:label>
    </owl:NamedIndividual>
    


    <!-- http://www.semanticweb.org/suhaspai/ontologies/2021/4/UnivFAQ#A_compact_kinetic_model_for_biomass_pyrolysis_at_gasification_conditions -->

    <owl:NamedIndividual rdf:about="http://www.semanticweb.org/suhaspai/ontologies/2021/4/UnivFAQ#A_compact_kinetic_model_for_biomass_pyrolysis_at_gasification_conditions">
        <rdf:type rdf:resource="http://www.semanticweb.org/suhaspai/ontologies/2021/4/UnivFAQ#Publication"/>
        <UnivFAQ:inResearchField rdf:resource="http://www.semanticweb.org/suhaspai/ontologies/2021/4/UnivFAQ#Clean_Energy"/>
        <UnivFAQ:publishedBy rdf:resource="http://www.semanticweb.org/suhaspai/ontologies/2021/4/UnivFAQ#Himanshu_Goyal"/>
        <rdfs:label>A compact kinetic model for biomass pyrolysis at gasification conditions</rdfs:label>
    </owl:NamedIndividual>
    


    <!-- http://www.semanticweb.org/suhaspai/ontologies/2021/4/UnivFAQ#A_heuristic_for_placement_of_limited_range_wavelength_converters_in_all-optical_networks -->

    <owl:NamedIndividual rdf:about="http://www.semanticweb.org/suhaspai/ontologies/2021/4/UnivFAQ#A_heuristic_for_placement_of_limited_range_wavelength_converters_in_all-optical_networks">
        <rdf:type rdf:resource="http://www.semanticweb.org/suhaspai/ontologies/2021/4/UnivFAQ#Publication"/>
        <UnivFAQ:inResearchField rdf:resource="http://www.semanticweb.org/suhaspai/ontologies/2021/4/UnivFAQ#Ontologies_and_Application"/>
        <UnivFAQ:publishedBy rdf:resource="http://www.semanticweb.org/suhaspai/ontologies/2021/4/UnivFAQ#Sreenivasa_Kumar"/>
        <rdfs:label>A heuristic for placement of limited range wavelength converters in all-optical networks</rdfs:label>
    </owl:NamedIndividual>
    


    <!-- http://www.semanticweb.org/suhaspai/ontologies/2021/4/UnivFAQ#A_quantitative_study_of_irregular_programs_on_GPUs -->

    <owl:NamedIndividual rdf:about="http://www.semanticweb.org/suhaspai/ontologies/2021/4/UnivFAQ#A_quantitative_study_of_irregular_programs_on_GPUs">
        <rdf:type rdf:resource="http://www.semanticweb.org/suhaspai/ontologies/2021/4/UnivFAQ#Publication"/>
        <UnivFAQ:inResearchField rdf:resource="http://www.semanticweb.org/suhaspai/ontologies/2021/4/UnivFAQ#Compilers"/>
        <UnivFAQ:publishedBy rdf:resource="http://www.semanticweb.org/suhaspai/ontologies/2021/4/UnivFAQ#Rupesh_Nasre"/>
        <rdfs:label>A quantitative study of irregular programs on GPUs</rdfs:label>
    </owl:NamedIndividual>
    


    <!-- http://www.semanticweb.org/suhaspai/ontologies/2021/4/UnivFAQ#Abishek_Sinha -->

    <owl:NamedIndividual rdf:about="http://www.semanticweb.org/suhaspai/ontologies/2021/4/UnivFAQ#Abishek_Sinha">
        <rdf:type rdf:resource="http://www.semanticweb.org/suhaspai/ontologies/2021/4/UnivFAQ#AssistantProfessor"/>
        <UnivFAQ:isSpecializedIn rdf:resource="http://www.semanticweb.org/suhaspai/ontologies/2021/4/UnivFAQ#Information_Theory"/>
        <UnivFAQ:isSpecializedIn rdf:resource="http://www.semanticweb.org/suhaspai/ontologies/2021/4/UnivFAQ#Network_Control"/>
        <UnivFAQ:teaches rdf:resource="http://www.semanticweb.org/suhaspai/ontologies/2021/4/UnivFAQ#EE6112"/>
        <UnivFAQ:name>Abishek Sinha</UnivFAQ:name>
        <rdfs:label>Abishek Sinha</rdfs:label>
    </owl:NamedIndividual>
    


    <!-- http://www.semanticweb.org/suhaspai/ontologies/2021/4/UnivFAQ#An_autoencoder_approach_to_learning_bilingual_word_representations -->

    <owl:NamedIndividual rdf:about="http://www.semanticweb.org/suhaspai/ontologies/2021/4/UnivFAQ#An_autoencoder_approach_to_learning_bilingual_word_representations">
        <rdf:type rdf:resource="http://www.semanticweb.org/suhaspai/ontologies/2021/4/UnivFAQ#Publication"/>
        <UnivFAQ:inResearchField rdf:resource="http://www.semanticweb.org/suhaspai/ontologies/2021/4/UnivFAQ#Reinforcement_Learning"/>
        <UnivFAQ:publishedBy rdf:resource="http://www.semanticweb.org/suhaspai/ontologies/2021/4/UnivFAQ#B_Ravindran"/>
        <rdfs:label>An autoencoder approach to learning bilingual word representations</rdfs:label>
    </owl:NamedIndividual>
    


    <!-- http://www.semanticweb.org/suhaspai/ontologies/2021/4/UnivFAQ#Analog -->

    <owl:NamedIndividual rdf:about="http://www.semanticweb.org/suhaspai/ontologies/2021/4/UnivFAQ#Analog">
        <rdf:type rdf:resource="http://www.semanticweb.org/suhaspai/ontologies/2021/4/UnivFAQ#ResearchFields"/>
        <rdfs:label>Analog</rdfs:label>
    </owl:NamedIndividual>
    


    <!-- http://www.semanticweb.org/suhaspai/ontologies/2021/4/UnivFAQ#Arnav_Mhaske -->

    <owl:NamedIndividual rdf:about="http://www.semanticweb.org/suhaspai/ontologies/2021/4/UnivFAQ#Arnav_Mhaske">
        <rdf:type rdf:resource="http://www.semanticweb.org/suhaspai/ontologies/2021/4/UnivFAQ#Student"/>
        <UnivFAQ:enrolledIn rdf:resource="http://www.semanticweb.org/suhaspai/ontologies/2021/4/UnivFAQ#DD_Computer_Science"/>
        <UnivFAQ:isAdvisedBy rdf:resource="http://www.semanticweb.org/suhaspai/ontologies/2021/4/UnivFAQ#Chandra_Sekhar"/>
        <rdfs:label>Arnav Mhaske</rdfs:label>
    </owl:NamedIndividual>
    


    <!-- http://www.semanticweb.org/suhaspai/ontologies/2021/4/UnivFAQ#Artificial_Intelligence -->

    <owl:NamedIndividual rdf:about="http://www.semanticweb.org/suhaspai/ontologies/2021/4/UnivFAQ#Artificial_Intelligence">
        <rdf:type rdf:resource="http://www.semanticweb.org/suhaspai/ontologies/2021/4/UnivFAQ#ResearchFields"/>
        <rdfs:comment>Artificial intelligence is intelligence demonstrated by machines, as opposed to natural intelligence displayed by animals including humans.</rdfs:comment>
        <rdfs:label>Artificial Intelligence</rdfs:label>
    </owl:NamedIndividual>
    


    <!-- http://www.semanticweb.org/suhaspai/ontologies/2021/4/UnivFAQ#Arun_Rajkumar -->

    <owl:NamedIndividual rdf:about="http://www.semanticweb.org/suhaspai/ontologies/2021/4/UnivFAQ#Arun_Rajkumar">
        <rdf:type rdf:resource="http://www.semanticweb.org/suhaspai/ontologies/2021/4/UnivFAQ#AssistantProfessor"/>
        <UnivFAQ:isSpecializedIn rdf:resource="http://www.semanticweb.org/suhaspai/ontologies/2021/4/UnivFAQ#Machine_Learning"/>
        <UnivFAQ:teaches rdf:resource="http://www.semanticweb.org/suhaspai/ontologies/2021/4/UnivFAQ#CS1100"/>
        <UnivFAQ:name>Arun Rajkumar</UnivFAQ:name>
        <rdfs:label>Arun Rajkumar</rdfs:label>
    </owl:NamedIndividual>
    


    <!-- http://www.semanticweb.org/suhaspai/ontologies/2021/4/UnivFAQ#Automation_In_Manufacturing_Research -->

    <owl:NamedIndividual rdf:about="http://www.semanticweb.org/suhaspai/ontologies/2021/4/UnivFAQ#Automation_In_Manufacturing_Research">
        <rdf:type rdf:resource="http://www.semanticweb.org/suhaspai/ontologies/2021/4/UnivFAQ#ResearchFields"/>
        <rdfs:comment>Automation, in the context of manufacturing, is the use of equipment to automate systems or production processes.</rdfs:comment>
        <rdfs:label>Automation In Manfacturing</rdfs:label>
    </owl:NamedIndividual>
    


    <!-- http://www.semanticweb.org/suhaspai/ontologies/2021/4/UnivFAQ#BTech._Chemical_Engineering -->

    <owl:NamedIndividual rdf:about="http://www.semanticweb.org/suhaspai/ontologies/2021/4/UnivFAQ#BTech._Chemical_Engineering">
        <rdf:type rdf:resource="http://www.semanticweb.org/suhaspai/ontologies/2021/4/UnivFAQ#BTech."/>
        <UnivFAQ:hasAdmissionRequisites rdf:resource="http://www.semanticweb.org/suhaspai/ontologies/2021/4/UnivFAQ#JEE_Advanced"/>
        <UnivFAQ:hasAdmissionRequisites rdf:resource="http://www.semanticweb.org/suhaspai/ontologies/2021/4/UnivFAQ#12th_Standard"/>
        <UnivFAQ:offeredBy rdf:resource="http://www.semanticweb.org/suhaspai/ontologies/2021/4/UnivFAQ#Chemical_Engineering"/>
        <rdfs:comment>The chemical engineering B.Tech program is a comprehensive one consisting of 12 core courses spanning various areas including mathematical methods, thermodynamics, reaction engineering, heat and mass transport, and process control. The newly revamped curriculum also involves 8 laboratory courses that serve as companions to the theory courses. Students are also encouraged to take up electives in process systems, computational fluid dynamics, catalysis, colloids, polymer rheology, and so on.</rdfs:comment>
        <rdfs:label>BTech. Chemical Engineering</rdfs:label>
    </owl:NamedIndividual>
    


    <!-- http://www.semanticweb.org/suhaspai/ontologies/2021/4/UnivFAQ#BTech._Computer_Science -->

    <owl:NamedIndividual rdf:about="http://www.semanticweb.org/suhaspai/ontologies/2021/4/UnivFAQ#BTech._Computer_Science">
        <rdf:type rdf:resource="http://www.semanticweb.org/suhaspai/ontologies/2021/4/UnivFAQ#BTech."/>
        <UnivFAQ:hasAdmissionRequisites rdf:resource="http://www.semanticweb.org/suhaspai/ontologies/2021/4/UnivFAQ#JEE_Advanced"/>
        <UnivFAQ:hasAdmissionRequisites rdf:resource="http://www.semanticweb.org/suhaspai/ontologies/2021/4/UnivFAQ#12th_Standard"/>
        <rdfs:comment>The B.Tech. program is a four-year course oriented undergraduate program. The course work is spread accross all the semesters. The courses include a set of core courses offered by the department, a set of departmental electives and some free electives. In total, the academic activities include 7 department electives and 8 free electives. A B.Tech project is optional and the student can take 2 additional department electives in lieu of the B.Tech project.</rdfs:comment>
        <rdfs:label>BTech. Computer Science</rdfs:label>
    </owl:NamedIndividual>
    


    <!-- http://www.semanticweb.org/suhaspai/ontologies/2021/4/UnivFAQ#BTech._Electrical_Engineering -->

    <owl:NamedIndividual rdf:about="http://www.semanticweb.org/suhaspai/ontologies/2021/4/UnivFAQ#BTech._Electrical_Engineering">
        <rdf:type rdf:resource="http://www.semanticweb.org/suhaspai/ontologies/2021/4/UnivFAQ#BTech."/>
        <UnivFAQ:hasAdmissionRequisites rdf:resource="http://www.semanticweb.org/suhaspai/ontologies/2021/4/UnivFAQ#JEE_Advanced"/>
        <UnivFAQ:hasAdmissionRequisites rdf:resource="http://www.semanticweb.org/suhaspai/ontologies/2021/4/UnivFAQ#12th_Standard"/>
        <rdfs:comment>The coveted Bachelors of Technology program awards students an undergraduate degree in an engineering discipline after four years of study. Entrance to the B.Tech programme is through the Joint Engineering Entrance (JEE) (Mains) and JEE (Advanced); conducted at various centres across the country. Admission to the particular branch of study is decided by the Joint Admission Committee.</rdfs:comment>
        <rdfs:label>BTech. Electrical Engineering</rdfs:label>
    </owl:NamedIndividual>
    


    <!-- http://www.semanticweb.org/suhaspai/ontologies/2021/4/UnivFAQ#BTech._Mechanical_Engineering -->

    <owl:NamedIndividual rdf:about="http://www.semanticweb.org/suhaspai/ontologies/2021/4/UnivFAQ#BTech._Mechanical_Engineering">
        <rdf:type rdf:resource="http://www.semanticweb.org/suhaspai/ontologies/2021/4/UnivFAQ#BTech."/>
        <UnivFAQ:hasAdmissionRequisites rdf:resource="http://www.semanticweb.org/suhaspai/ontologies/2021/4/UnivFAQ#JEE_Advanced"/>
        <UnivFAQ:hasAdmissionRequisites rdf:resource="http://www.semanticweb.org/suhaspai/ontologies/2021/4/UnivFAQ#12th_Standard"/>
        <UnivFAQ:offeredBy rdf:resource="http://www.semanticweb.org/suhaspai/ontologies/2021/4/UnivFAQ#Mechanical_Engineering"/>
        <rdfs:comment>Our undergraduate courses offer a unique blend of rigour, creativity and practicality. The underlying science is taught by experts at the leading edge of international research.

The students are admitted through JEE. For a general introduction to our 4-year undergraduate programs, please look through our online prospectus and the student handbook for current undergraduates available at: https://mitr.iitm.ac.in/main/index.php/downloads.</rdfs:comment>
        <rdfs:label>BTech. Mechanical Engineering</rdfs:label>
    </owl:NamedIndividual>
    


    <!-- http://www.semanticweb.org/suhaspai/ontologies/2021/4/UnivFAQ#B_Ravindran -->

    <owl:NamedIndividual rdf:about="http://www.semanticweb.org/suhaspai/ontologies/2021/4/UnivFAQ#B_Ravindran">
        <rdf:type rdf:resource="http://www.semanticweb.org/suhaspai/ontologies/2021/4/UnivFAQ#Professor"/>
        <UnivFAQ:isSpecializedIn rdf:resource="http://www.semanticweb.org/suhaspai/ontologies/2021/4/UnivFAQ#Reinforcement_Learning"/>
        <UnivFAQ:teaches rdf:resource="http://www.semanticweb.org/suhaspai/ontologies/2021/4/UnivFAQ#CS6700"/>
        <UnivFAQ:name rdf:datatype="http://www.w3.org/2001/XMLSchema#string">Balaram Ravindran</UnivFAQ:name>
        <rdfs:label rdf:datatype="http://www.w3.org/2001/XMLSchema#string">Balaram Ravindran</rdfs:label>
    </owl:NamedIndividual>
    


    <!-- http://www.semanticweb.org/suhaspai/ontologies/2021/4/UnivFAQ#CH1020 -->

    <owl:NamedIndividual rdf:about="http://www.semanticweb.org/suhaspai/ontologies/2021/4/UnivFAQ#CH1020">
        <rdf:type rdf:resource="http://www.semanticweb.org/suhaspai/ontologies/2021/4/UnivFAQ#Courses"/>
        <UnivFAQ:taughtBy rdf:resource="http://www.semanticweb.org/suhaspai/ontologies/2021/4/UnivFAQ#Preeti_Aghalayam"/>
        <rdfs:comment>The main objectives of this course are to write material and energy balances for various chemical process units and combination of units. It is an introductory course that serves as an important precursor to all other Chemical Engg courses</rdfs:comment>
        <rdfs:label>Principles &amp; Calculations in Chemical</rdfs:label>
    </owl:NamedIndividual>
    


    <!-- http://www.semanticweb.org/suhaspai/ontologies/2021/4/UnivFAQ#CH4250 -->

    <owl:NamedIndividual rdf:about="http://www.semanticweb.org/suhaspai/ontologies/2021/4/UnivFAQ#CH4250">
        <rdf:type rdf:resource="http://www.semanticweb.org/suhaspai/ontologies/2021/4/UnivFAQ#Courses"/>
        <rdfs:comment>By the end of this course, students would be able to develop a process flowsheet to produce a specified product at given production rates. Towards this, they would specifically be able to: • Conduct surveys for information on available technologies, markets, prices, safety/environment impacts • Develop a process flowsheet based on chemical engineering principles and heuristics • Perform preliminary &amp; detailed economic analysis of the process • Analyse material and energy balances for a complete integrated process using flowsheeting software such as Aspen Plus • Develop a complete process flow diagram (PFD) for a process • Carry out Chemical Engineering design of major items of equipment such as reactors, distillation columns, heat exchangers, pumps, compressors, etc • Carry out Mechanical design of one or more equipment with reference to appropriate codes and design standards • Conduct safety, health, and sustainability analysis of an integrated process</rdfs:comment>
        <rdfs:label>Process Engineering</rdfs:label>
    </owl:NamedIndividual>
    


    <!-- http://www.semanticweb.org/suhaspai/ontologies/2021/4/UnivFAQ#CH5030 -->

    <owl:NamedIndividual rdf:about="http://www.semanticweb.org/suhaspai/ontologies/2021/4/UnivFAQ#CH5030">
        <rdf:type rdf:resource="http://www.semanticweb.org/suhaspai/ontologies/2021/4/UnivFAQ#Courses"/>
        <rdfs:comment>know the constitutive relationships in mass, momentum, and energy transport - know the generalized equations for mass, momentum, and energy conservation - recognize the transport phenomena involved in an engineering problem - be able to apply the generalized equations for mass, momentum, and energy conservation for practical problems - be able to mathematically represent the practical transport phenomena problems - be able to solve one-dimensional transport phenomena problems</rdfs:comment>
        <rdfs:label>Transport Phenomena</rdfs:label>
    </owl:NamedIndividual>
    


    <!-- http://www.semanticweb.org/suhaspai/ontologies/2021/4/UnivFAQ#CH5370 -->

    <owl:NamedIndividual rdf:about="http://www.semanticweb.org/suhaspai/ontologies/2021/4/UnivFAQ#CH5370">
        <rdf:type rdf:resource="http://www.semanticweb.org/suhaspai/ontologies/2021/4/UnivFAQ#Courses"/>
        <UnivFAQ:hasFacility rdf:resource="http://www.semanticweb.org/suhaspai/ontologies/2021/4/UnivFAQ#IACE_Lab"/>
        <rdfs:comment>To provide a fundamental understanding of pollutants, their characteristics and the mechanisms underlying the fate and transport of pollutants in the environment. The course is meant for environmental engineers.</rdfs:comment>
        <rdfs:label>Environmental Quality Monitoring &amp; Analysis</rdfs:label>
    </owl:NamedIndividual>
    


    <!-- http://www.semanticweb.org/suhaspai/ontologies/2021/4/UnivFAQ#CS1100 -->

    <owl:NamedIndividual rdf:about="http://www.semanticweb.org/suhaspai/ontologies/2021/4/UnivFAQ#CS1100">
        <rdf:type rdf:resource="http://www.semanticweb.org/suhaspai/ontologies/2021/4/UnivFAQ#UndergradCourses"/>
        <UnivFAQ:isPrerequisiteFor rdf:resource="http://www.semanticweb.org/suhaspai/ontologies/2021/4/UnivFAQ#CS1200"/>
        <UnivFAQ:isPrerequisiteFor rdf:resource="http://www.semanticweb.org/suhaspai/ontologies/2021/4/UnivFAQ#CS2800"/>
        <UnivFAQ:isPrerequisiteFor rdf:resource="http://www.semanticweb.org/suhaspai/ontologies/2021/4/UnivFAQ#CS3700"/>
        <UnivFAQ:isPrerequisiteFor rdf:resource="http://www.semanticweb.org/suhaspai/ontologies/2021/4/UnivFAQ#CS6023"/>
        <UnivFAQ:isPrerequisiteFor rdf:resource="http://www.semanticweb.org/suhaspai/ontologies/2021/4/UnivFAQ#CS6910"/>
        <rdfs:comment>The introductory computer science course - teaches basic programming to fresher students</rdfs:comment>
        <rdfs:label>Introduction to Programming</rdfs:label>
    </owl:NamedIndividual>
    


    <!-- http://www.semanticweb.org/suhaspai/ontologies/2021/4/UnivFAQ#CS1200 -->

    <owl:NamedIndividual rdf:about="http://www.semanticweb.org/suhaspai/ontologies/2021/4/UnivFAQ#CS1200">
        <rdf:type rdf:resource="http://www.semanticweb.org/suhaspai/ontologies/2021/4/UnivFAQ#UndergradCourses"/>
        <rdfs:comment>The course is about sets which are discrete in nature. It starts from ways of describing them, then size estimates of sets (combinatorics), and then culminates in studying structured sets. After completing the course, the student will be able to: (1) Use logical notation to define and reason mathematically about the fundamental data types and structures (such as numbers, sets) used in computer algorithms and systems. (2) Comprehend and Evaluate rigour in the definitions and conclusions about mathematical models and identify fallacious reasoning and statements. (3) Identify and Apply properties of combinatorial structures and properties - know the basic techniques in combinatorics and counting. (4) Analyze sets with operations, and identify their structure. (5) Reason and Conclude properties about the structure based on the observations. (6) Gain the conceptual background needed to be able to identify structures of algebraic nature, and discover, prove and use properties about them.</rdfs:comment>
        <rdfs:label>Discrete Mathematics</rdfs:label>
    </owl:NamedIndividual>
    


    <!-- http://www.semanticweb.org/suhaspai/ontologies/2021/4/UnivFAQ#CS2800 -->

    <owl:NamedIndividual rdf:about="http://www.semanticweb.org/suhaspai/ontologies/2021/4/UnivFAQ#CS2800">
        <rdf:type rdf:resource="http://www.semanticweb.org/suhaspai/ontologies/2021/4/UnivFAQ#Courses"/>
        <UnivFAQ:offeredBy rdf:resource="http://www.semanticweb.org/suhaspai/ontologies/2021/4/UnivFAQ#Computer_Science"/>
        <rdfs:comment>The objective of the course is to teach techniques for effective problem solving incomputing. The use of different paradigms of problem solving will be used to illustrate cleverand efficient ways to solve a given problem. In each case emphasis will be placed onrigorously proving correctness of the algorithm. In addition, the analysis of the algorithm will beused to show the efficiency of the algorithm over the naive techniques.</rdfs:comment>
        <rdfs:label>Design and Analysis of Algorithms</rdfs:label>
    </owl:NamedIndividual>
    


    <!-- http://www.semanticweb.org/suhaspai/ontologies/2021/4/UnivFAQ#CS3700 -->

    <owl:NamedIndividual rdf:about="http://www.semanticweb.org/suhaspai/ontologies/2021/4/UnivFAQ#CS3700">
        <rdf:type rdf:resource="http://www.semanticweb.org/suhaspai/ontologies/2021/4/UnivFAQ#Courses"/>
        <UnivFAQ:isPrerequisiteFor rdf:resource="http://www.semanticweb.org/suhaspai/ontologies/2021/4/UnivFAQ#CS6852"/>
        <rdfs:comment>General introduction to database systems; Database - DBMS disctinction, approaches to building a database, data models, database management system, three-schema architecture of a database, challenges in building a DBMS, various components of a DBMS. E/R Model - Conceptual data modeling - motivation, entities, entity types, various types of attributes, relationships, relationship types, E/R diagram notation, examples. Relational Data Model - Concept of relations, schema-instance distinction, keys, referential integrity and foreign keys, relational algebra operators: selection, projection, cross product, various types of joins, division, example queries, tuple relation calculus, domain relational calculus, converting the database specification in E/R notation to the relational schema. SQL - Introduction, data definition in SQL, table, key and foreign key definitions, update behaviors. Querying in SQL - basic select-from-where block and its semantics, nested queries - correlated and uncorrelated, notion of aggregation, aggregation functions group by and having clauses, embedded SQL. Dependencies and Normal forms - Importance of a good schema design, problems encountered with bad schema designs, motivation for normal forms, dependency theory - functional dependencies, Armstrong&apos;s axioms for FD&apos;s, closure of a set of FD&apos;s, minimal covers, definitions of 1NF, 2NF, 3NF and BCNF, decompositions and desirable properties of them, algorithms for 3NF and BCNF normalization, multi-valued dependencies and 4NF, join dependencies and definition of 5NF. Data Storage and Indexes - file organizations, primary, secondary index structures, various index structures - hash-based, dynamic hashing techniques, multi-level indexes, B+ trees. Transaction processing and Error recovery - concepts of transaction processing, ACID properties, concurrency control, locking based protocols for CC, error recovery and logging, undo, redo, undo-redo logging and recovery methods.</rdfs:comment>
        <rdfs:label>Introduction to Database Systems</rdfs:label>
    </owl:NamedIndividual>
    


    <!-- http://www.semanticweb.org/suhaspai/ontologies/2021/4/UnivFAQ#CS6023 -->

    <owl:NamedIndividual rdf:about="http://www.semanticweb.org/suhaspai/ontologies/2021/4/UnivFAQ#CS6023">
        <rdf:type rdf:resource="http://www.semanticweb.org/suhaspai/ontologies/2021/4/UnivFAQ#Courses"/>
        <UnivFAQ:offeredBy rdf:resource="http://www.semanticweb.org/suhaspai/ontologies/2021/4/UnivFAQ#Computer_Science"/>
        <rdfs:comment>To learn parallel programming with graphics processing units (GPUs) Outcomes: Students would learn concepts in parallel programming, implementation of programs on GPUs, debugging and profiling parallel programs.</rdfs:comment>
        <rdfs:label>GPU Programming</rdfs:label>
    </owl:NamedIndividual>
    


    <!-- http://www.semanticweb.org/suhaspai/ontologies/2021/4/UnivFAQ#CS6700 -->

    <owl:NamedIndividual rdf:about="http://www.semanticweb.org/suhaspai/ontologies/2021/4/UnivFAQ#CS6700">
        <rdf:type rdf:resource="http://www.semanticweb.org/suhaspai/ontologies/2021/4/UnivFAQ#Courses"/>
        <UnivFAQ:offeredBy rdf:resource="http://www.semanticweb.org/suhaspai/ontologies/2021/4/UnivFAQ#Computer_Science"/>
        <rdfs:comment>The Reinforcement Learning problem : evaluative feedback, non-associative learning, Rewards and returns, Markov Decision Processes, Value functions, optimality and approximation. Dynamic programming : value iteration, policy iteration, asynchronous DP, generalized policy iteration. Monta-Carlo methods : policy evaluation, roll outs, on policy and off policy learning, importance sampling. Temporal Difference learning : TD prediction, Optimality of TD(0), SARSA, Q-learning, R-learning, Games and after states. Eligibility traces : n-step TD prediction, TD (lambda), forward and backward views, Q (lambda), SARSA (lambda), replacing traces and accumulating traces. Function Approximation : Value prediction, gradient descent methods, linear function approximation, ANN based function approximation, lazy learning, instability issues Policy Gradient methods : non-associative learning – REINFORCE algorithm, exact gradient methods, estimating gradients, approximate policy gradient algorithms, actor-critic methods. Planning and Learning : Model based learning and planning, prioritized sweeping, Dyna, heuristic search, trajectory sampling, E 3 algorithm Hierarchical RL : MAXQ framework, Options framework, HAM framework, airport algorithm, hierarchical policy gradient Case studies : Elevator dispatching, Samuel’s checker player, TDgammon, Acrobot, Helicopter piloting</rdfs:comment>
        <rdfs:label>Reinforcement Learning</rdfs:label>
    </owl:NamedIndividual>
    


    <!-- http://www.semanticweb.org/suhaspai/ontologies/2021/4/UnivFAQ#CS6852 -->

    <owl:NamedIndividual rdf:about="http://www.semanticweb.org/suhaspai/ontologies/2021/4/UnivFAQ#CS6852">
        <rdf:type rdf:resource="http://www.semanticweb.org/suhaspai/ontologies/2021/4/UnivFAQ#Courses"/>
        <UnivFAQ:offeredBy rdf:resource="http://www.semanticweb.org/suhaspai/ontologies/2021/4/UnivFAQ#Computer_Science"/>
        <rdfs:comment>To discuss topics in the emerging areas of Semantic Web Technology, Ontologies for Knowledge Representation and their Applications.</rdfs:comment>
        <rdfs:label>Theory and Applications of Ontologies</rdfs:label>
    </owl:NamedIndividual>
    


    <!-- http://www.semanticweb.org/suhaspai/ontologies/2021/4/UnivFAQ#CS6910 -->

    <owl:NamedIndividual rdf:about="http://www.semanticweb.org/suhaspai/ontologies/2021/4/UnivFAQ#CS6910">
        <rdf:type rdf:resource="http://www.semanticweb.org/suhaspai/ontologies/2021/4/UnivFAQ#Courses"/>
        <UnivFAQ:offeredBy rdf:resource="http://www.semanticweb.org/suhaspai/ontologies/2021/4/UnivFAQ#Computer_Science"/>
        <rdfs:comment>Neural Networks have made tremendous impact on various AI fields in the recent past. In this course, we study the basics of Neural Networks and their various variants such as the Convolutional Neural Networks and Recurrent Neural Networks. We also study the different ways in which they can be used to solve problems in various domains such as Computer Vision, Speech and NLP. We also look at the latest results and trends in the field.</rdfs:comment>
        <rdfs:label>Deep Learning</rdfs:label>
    </owl:NamedIndividual>
    


    <!-- http://www.semanticweb.org/suhaspai/ontologies/2021/4/UnivFAQ#C_Gautam -->

    <owl:NamedIndividual rdf:about="http://www.semanticweb.org/suhaspai/ontologies/2021/4/UnivFAQ#C_Gautam">
        <rdf:type rdf:resource="http://www.semanticweb.org/suhaspai/ontologies/2021/4/UnivFAQ#Student"/>
        <UnivFAQ:enrolledIn rdf:resource="http://www.semanticweb.org/suhaspai/ontologies/2021/4/UnivFAQ#DD_Computer_Science"/>
        <UnivFAQ:isAdvisedBy rdf:resource="http://www.semanticweb.org/suhaspai/ontologies/2021/4/UnivFAQ#N_S_Narayanaswamy"/>
        <rdfs:label>C Gautam</rdfs:label>
    </owl:NamedIndividual>
    


    <!-- http://www.semanticweb.org/suhaspai/ontologies/2021/4/UnivFAQ#Chandra_Sekhar -->

    <owl:NamedIndividual rdf:about="http://www.semanticweb.org/suhaspai/ontologies/2021/4/UnivFAQ#Chandra_Sekhar">
        <rdf:type rdf:resource="http://www.semanticweb.org/suhaspai/ontologies/2021/4/UnivFAQ#Professor"/>
        <UnivFAQ:headsDepartment rdf:resource="http://www.semanticweb.org/suhaspai/ontologies/2021/4/UnivFAQ#Computer_Science"/>
        <UnivFAQ:isSpecializedIn rdf:resource="http://www.semanticweb.org/suhaspai/ontologies/2021/4/UnivFAQ#Artificial_Intelligence"/>
        <UnivFAQ:isSpecializedIn rdf:resource="http://www.semanticweb.org/suhaspai/ontologies/2021/4/UnivFAQ#Reinforcement_Learning"/>
        <UnivFAQ:teaches rdf:resource="http://www.semanticweb.org/suhaspai/ontologies/2021/4/UnivFAQ#CS6910"/>
        <UnivFAQ:name rdf:datatype="http://www.w3.org/2001/XMLSchema#string">C Chandra Sekhar</UnivFAQ:name>
        <rdfs:label rdf:datatype="http://www.w3.org/2001/XMLSchema#string">C Chandra Sekhar</rdfs:label>
    </owl:NamedIndividual>
    


    <!-- http://www.semanticweb.org/suhaspai/ontologies/2021/4/UnivFAQ#Chemical_Engineering -->

    <owl:NamedIndividual rdf:about="http://www.semanticweb.org/suhaspai/ontologies/2021/4/UnivFAQ#Chemical_Engineering">
        <rdf:type rdf:resource="http://www.semanticweb.org/suhaspai/ontologies/2021/4/UnivFAQ#Department"/>
        <UnivFAQ:offers rdf:resource="http://www.semanticweb.org/suhaspai/ontologies/2021/4/UnivFAQ#CH1020"/>
        <UnivFAQ:offers rdf:resource="http://www.semanticweb.org/suhaspai/ontologies/2021/4/UnivFAQ#CH4250"/>
        <UnivFAQ:offers rdf:resource="http://www.semanticweb.org/suhaspai/ontologies/2021/4/UnivFAQ#CH5030"/>
        <UnivFAQ:offers rdf:resource="http://www.semanticweb.org/suhaspai/ontologies/2021/4/UnivFAQ#CH5370"/>
        <rdfs:comment>Chemical Engineering is a constantly evolving discipline which keeps pace with the developing world. Our department reflects this in its teaching curriculum, research thrusts, industry partnerships and entrepreneurial initiatives. Founded in 1959 along with the rest of the Institute, the Department in its early days bore the imprint of German collaboration in nearly every functional aspect. The laboratories were well equipped with large-scale equipment that are still fully operational. While the trend towards miniaturization has led to ongoing replacement, faculty still carry out consultancy assignments for industry using these. They also give the students an early appreciation of the “shop floor” in factories.

The recent re-introduction of an “Introduction to Chemical Engineering” course for first-year undergraduates has been widely welcomed by the students. Combining a variety of lectures by faculty and industry practitioners with visits to manufacturing locations, the course is an eye-opener for many who choose the discipline without quite knowing its scope. Core courses that emphasize the fundamentals, electives that broaden the horizon, and laboratories—for UGs and graduate students– that reinforce classroom learning ensure that we graduate students who are equally capable of pursuing higher degrees and industry careers.

Undergraduates are encouraged to take up research projects in their 2nd year and carry them through to their Senior Year. They undertake one mandatory summer internship in Indian industry, and usually Doctoral candidates and postdoctoral Fellows ensure a research focus that is ever-intensifying. With an average of 5-6 Ph.D. students and 1-2 PDFs per faculty, research Groups are now reaching critical mass. Publication metrics, conference participation and patent filings are among the best in India, befitting an Institution that has been ranked # 1 in India four years in a row, and most recently, was also recognized as one that has the best innovation/ incubation ecosystem. Nearly 20% of the faculty in ChE are actively involved in start-up’s, facilitated by India’s first and still only University-based Research Park located next door.</rdfs:comment>
        <rdfs:label>Chemical Engineering Department</rdfs:label>
    </owl:NamedIndividual>
    


    <!-- http://www.semanticweb.org/suhaspai/ontologies/2021/4/UnivFAQ#Clean_Energy -->

    <owl:NamedIndividual rdf:about="http://www.semanticweb.org/suhaspai/ontologies/2021/4/UnivFAQ#Clean_Energy">
        <rdf:type rdf:resource="http://www.semanticweb.org/suhaspai/ontologies/2021/4/UnivFAQ#ResearchFields"/>
        <rdfs:comment>Clean energy is energy that comes from renewable, zero emission sources that do not pollute the atmosphere when used</rdfs:comment>
        <rdfs:label>Clean Energy</rdfs:label>
    </owl:NamedIndividual>
    


    <!-- http://www.semanticweb.org/suhaspai/ontologies/2021/4/UnivFAQ#Comparison_of_Millimeter_Quadrature_VCOs_for_28GHz_5G_applications -->

    <owl:NamedIndividual rdf:about="http://www.semanticweb.org/suhaspai/ontologies/2021/4/UnivFAQ#Comparison_of_Millimeter_Quadrature_VCOs_for_28GHz_5G_applications">
        <rdf:type rdf:resource="http://www.semanticweb.org/suhaspai/ontologies/2021/4/UnivFAQ#Publication"/>
        <UnivFAQ:inResearchField rdf:resource="http://www.semanticweb.org/suhaspai/ontologies/2021/4/UnivFAQ#RFIC_Design"/>
        <UnivFAQ:publishedBy rdf:resource="http://www.semanticweb.org/suhaspai/ontologies/2021/4/UnivFAQ#S_Aniruddhan"/>
        <rdfs:label>Comparison of Millimeter Quadrature VCOs for 28GHz 5G applications</rdfs:label>
    </owl:NamedIndividual>
    


    <!-- http://www.semanticweb.org/suhaspai/ontologies/2021/4/UnivFAQ#Compilers -->

    <owl:NamedIndividual rdf:about="http://www.semanticweb.org/suhaspai/ontologies/2021/4/UnivFAQ#Compilers">
        <rdf:type rdf:resource="http://www.semanticweb.org/suhaspai/ontologies/2021/4/UnivFAQ#ResearchFields"/>
        <rdfs:comment>research into foundational software tools helping scientists to program for speed, interoperability, interactivity, flexibility, and reproducibility.</rdfs:comment>
        <rdfs:label>Compilers</rdfs:label>
    </owl:NamedIndividual>
    


    <!-- http://www.semanticweb.org/suhaspai/ontologies/2021/4/UnivFAQ#Computer_Science -->

    <owl:NamedIndividual rdf:about="http://www.semanticweb.org/suhaspai/ontologies/2021/4/UnivFAQ#Computer_Science">
        <rdf:type rdf:resource="http://www.semanticweb.org/suhaspai/ontologies/2021/4/UnivFAQ#Department"/>
        <UnivFAQ:hasFacility rdf:resource="http://www.semanticweb.org/suhaspai/ontologies/2021/4/UnivFAQ#AIDB_Lab"/>
        <UnivFAQ:hasFacility rdf:resource="http://www.semanticweb.org/suhaspai/ontologies/2021/4/UnivFAQ#DCF_Lab"/>
        <UnivFAQ:hasFacility rdf:resource="http://www.semanticweb.org/suhaspai/ontologies/2021/4/UnivFAQ#PACE_Lab"/>
        <UnivFAQ:offers rdf:resource="http://www.semanticweb.org/suhaspai/ontologies/2021/4/UnivFAQ#BTech._Computer_Science"/>
        <UnivFAQ:offers rdf:resource="http://www.semanticweb.org/suhaspai/ontologies/2021/4/UnivFAQ#CS1100"/>
        <UnivFAQ:offers rdf:resource="http://www.semanticweb.org/suhaspai/ontologies/2021/4/UnivFAQ#CS1200"/>
        <UnivFAQ:offers rdf:resource="http://www.semanticweb.org/suhaspai/ontologies/2021/4/UnivFAQ#CS3700"/>
        <rdfs:comment>Global excellence and local relevance in research, teaching, and technology development is the vision of the Department. The Department was started as the Computer Centre in 1973 with the acquisition of an IBM 370, perhaps the most powerful computer in India at that time. It offered M.Tech, M.S and PhD degree programmes. In 1983, the B.Tech degree programme was started.

Today the Department has a vibrant student body numbering about 700. Over 60% are postgraduate, mostly supported by scholarships. The Department also offers several attractive industry-sponsored Fellowships for outstanding PhD scholars and liberally supports participation in top-ranking international conferences.

The department has been funded by FIST program from DST, Govt. of India in 2002 and 2017. The Secure Systems Laboratory is funded by FIST program 2017.</rdfs:comment>
        <rdfs:label>Computer Science Department</rdfs:label>
    </owl:NamedIndividual>
    


    <!-- http://www.semanticweb.org/suhaspai/ontologies/2021/4/UnivFAQ#Converter_placement_in_all-optical_networks_using_genetic_algorithms -->

    <owl:NamedIndividual rdf:about="http://www.semanticweb.org/suhaspai/ontologies/2021/4/UnivFAQ#Converter_placement_in_all-optical_networks_using_genetic_algorithms">
        <rdf:type rdf:resource="http://www.semanticweb.org/suhaspai/ontologies/2021/4/UnivFAQ#Publication"/>
        <UnivFAQ:inResearchField rdf:resource="http://www.semanticweb.org/suhaspai/ontologies/2021/4/UnivFAQ#Genetic_Algorithms"/>
        <UnivFAQ:publishedBy rdf:resource="http://www.semanticweb.org/suhaspai/ontologies/2021/4/UnivFAQ#Sreenivasa_Kumar"/>
        <rdfs:label>Converter placement in all-optical networks using genetic algorithms</rdfs:label>
    </owl:NamedIndividual>
    


    <!-- http://www.semanticweb.org/suhaspai/ontologies/2021/4/UnivFAQ#Cryptography -->

    <owl:NamedIndividual rdf:about="http://www.semanticweb.org/suhaspai/ontologies/2021/4/UnivFAQ#Cryptography">
        <rdf:type rdf:resource="http://www.semanticweb.org/suhaspai/ontologies/2021/4/UnivFAQ#ResearchFields"/>
        <rdfs:comment>Cryptography, or cryptology, is the practice and study of techniques for secure communication in the presence of adversarial behavior.</rdfs:comment>
        <rdfs:label>Cryptography</rdfs:label>
    </owl:NamedIndividual>
    


    <!-- http://www.semanticweb.org/suhaspai/ontologies/2021/4/UnivFAQ#DCF_Lab -->

    <owl:NamedIndividual rdf:about="http://www.semanticweb.org/suhaspai/ontologies/2021/4/UnivFAQ#DCF_Lab">
        <rdf:type rdf:resource="http://www.semanticweb.org/suhaspai/ontologies/2021/4/UnivFAQ#InstituteFacilities"/>
        <rdfs:comment>Departmental Computing Facility (DCF) is an exclusive departmental digital laboratory with sophisticated technology</rdfs:comment>
        <rdfs:label>DCF Lab</rdfs:label>
    </owl:NamedIndividual>
    


    <!-- http://www.semanticweb.org/suhaspai/ontologies/2021/4/UnivFAQ#DD_Computer_Science -->

    <owl:NamedIndividual rdf:about="http://www.semanticweb.org/suhaspai/ontologies/2021/4/UnivFAQ#DD_Computer_Science">
        <rdf:type rdf:resource="http://www.semanticweb.org/suhaspai/ontologies/2021/4/UnivFAQ#Dual_Degree"/>
        <UnivFAQ:hasAdmissionRequisites rdf:resource="http://www.semanticweb.org/suhaspai/ontologies/2021/4/UnivFAQ#JEE_Advanced"/>
        <UnivFAQ:hasAdmissionRequisites rdf:resource="http://www.semanticweb.org/suhaspai/ontologies/2021/4/UnivFAQ#12th_Standard"/>
        <UnivFAQ:offeredBy rdf:resource="http://www.semanticweb.org/suhaspai/ontologies/2021/4/UnivFAQ#Computer_Science"/>
        <rdfs:comment>The Dual Degree program is a five year program. At the end of five years, the student is awarded both a B.Tech. and M.Tech. degree.</rdfs:comment>
        <rdfs:label>Dual Degree (BTech. + MTech.) Computer Science</rdfs:label>
    </owl:NamedIndividual>
    


    <!-- http://www.semanticweb.org/suhaspai/ontologies/2021/4/UnivFAQ#DD_Electrical_Engineering -->

    <owl:NamedIndividual rdf:about="http://www.semanticweb.org/suhaspai/ontologies/2021/4/UnivFAQ#DD_Electrical_Engineering">
        <rdf:type rdf:resource="http://www.semanticweb.org/suhaspai/ontologies/2021/4/UnivFAQ#Dual_Degree"/>
        <rdfs:comment>Dual Degree programs offered in select engineering and sciences disciplines earns a student an undergraduate and a master’s degree after five years of study. Entrance to the programme is through the Joint Engineering Entrance (JEE) (Mains) and JEE (Advanced); conducted at various centres across the country.</rdfs:comment>
        <rdfs:label>Dual Degree (BTech. + MTech.) Electrical Engineering</rdfs:label>
    </owl:NamedIndividual>
    


    <!-- http://www.semanticweb.org/suhaspai/ontologies/2021/4/UnivFAQ#Dhiman_Chatterjee -->

    <owl:NamedIndividual rdf:about="http://www.semanticweb.org/suhaspai/ontologies/2021/4/UnivFAQ#Dhiman_Chatterjee">
        <rdf:type rdf:resource="http://www.semanticweb.org/suhaspai/ontologies/2021/4/UnivFAQ#Professor"/>
        <UnivFAQ:isSpecializedIn rdf:resource="http://www.semanticweb.org/suhaspai/ontologies/2021/4/UnivFAQ#Fluid_Mechanics"/>
        <UnivFAQ:teaches rdf:resource="http://www.semanticweb.org/suhaspai/ontologies/2021/4/UnivFAQ#ME1100"/>
        <UnivFAQ:name rdf:datatype="http://www.w3.org/2001/XMLSchema#string">Dhiman Chatterjee</UnivFAQ:name>
        <rdfs:label rdf:datatype="http://www.w3.org/2001/XMLSchema#string">Dhiman Chatterjee</rdfs:label>
    </owl:NamedIndividual>
    


    <!-- http://www.semanticweb.org/suhaspai/ontologies/2021/4/UnivFAQ#EE3002 -->

    <owl:NamedIndividual rdf:about="http://www.semanticweb.org/suhaspai/ontologies/2021/4/UnivFAQ#EE3002">
        <rdf:type rdf:resource="http://www.semanticweb.org/suhaspai/ontologies/2021/4/UnivFAQ#Courses"/>
        <rdfs:comment>Learning objectives:This course is an introduction to amplifiers using transistors. Students will be introduced to MOS transistors, their characteristics, techniques for biasing them, and amplifiers using them. The basic transistor amplifier stages are seen as realizations of different controlled sources using negative feedback. Small- and large-signal characteristics of each amplifier will be discussed. Frequency ompensation techniques to stabilise higher order systems will be discussed.Learning Outcomes:At the end of this course, students should be able to recognize and analyze the basic amplifiers and biasing arrangements using MOS or bipolar transistors. Students should also be able to perform dominant-pole compensation of higher order systems and stabilise them.</rdfs:comment>
        <rdfs:label>Analog Circuits</rdfs:label>
    </owl:NamedIndividual>
    


    <!-- http://www.semanticweb.org/suhaspai/ontologies/2021/4/UnivFAQ#EE6112 -->

    <owl:NamedIndividual rdf:about="http://www.semanticweb.org/suhaspai/ontologies/2021/4/UnivFAQ#EE6112">
        <rdf:type rdf:resource="http://www.semanticweb.org/suhaspai/ontologies/2021/4/UnivFAQ#Courses"/>
        <rdfs:comment>This is proposed as an advanced graduate course, dealing predominantly with martingale techniques and concentration of probability measures, along with a few allied topics of interest in probability theory. Martingale and measure concentration techniques are becoming increasingly popular is various active areas of research, such as machine learning, resource allocation, complex networks, information theory and coding theory. It is hoped that this course would equip the students with the requisite familiarity and conceptual grasp to tackle various contemporary analysis and proof techniques.</rdfs:comment>
        <rdfs:label>Topics in Random Processes and Concentrations</rdfs:label>
    </owl:NamedIndividual>
    


    <!-- http://www.semanticweb.org/suhaspai/ontologies/2021/4/UnivFAQ#EE6150 -->

    <owl:NamedIndividual rdf:about="http://www.semanticweb.org/suhaspai/ontologies/2021/4/UnivFAQ#EE6150">
        <rdf:type rdf:resource="http://www.semanticweb.org/suhaspai/ontologies/2021/4/UnivFAQ#Courses"/>
        <rdfs:comment>A short tour through basics (not very measure theoretic) of axiomatic probability theory, convergence, and laws of large numbers. 2. Discrete time Markov chains: class properties, stationary distribution, hitting and mixing times, coupling, and applications to queues and social networks. 3. Renewal theory: elementary renewal theorem, Wald’s lemma, renewal reward theorem, and batch biasing (brief discussion on Key and Blackwell’s renewal theorem). 4. Poisson process. 5. Continuous time Markov chains: stationarity, time reversal, Kelly’s lemma, reversibility, and applications to social networks and queues. 6. (If time permits) Chernoff bound and introduction to large deviations; Martingales and concentration</rdfs:comment>
        <rdfs:label>Stochastic Modeling and the Theory of Queues</rdfs:label>
    </owl:NamedIndividual>
    


    <!-- http://www.semanticweb.org/suhaspai/ontologies/2021/4/UnivFAQ#Electrical_Engineering -->

    <owl:NamedIndividual rdf:about="http://www.semanticweb.org/suhaspai/ontologies/2021/4/UnivFAQ#Electrical_Engineering">
        <rdf:type rdf:resource="http://www.semanticweb.org/suhaspai/ontologies/2021/4/UnivFAQ#Department"/>
        <UnivFAQ:hasFacility rdf:resource="http://www.semanticweb.org/suhaspai/ontologies/2021/4/UnivFAQ#Microelectronics_and_MEMS_laboratory"/>
        <UnivFAQ:hasFacility rdf:resource="http://www.semanticweb.org/suhaspai/ontologies/2021/4/UnivFAQ#VLSI_Lab"/>
        <UnivFAQ:offers rdf:resource="http://www.semanticweb.org/suhaspai/ontologies/2021/4/UnivFAQ#BTech._Electrical_Engineering"/>
        <UnivFAQ:offers rdf:resource="http://www.semanticweb.org/suhaspai/ontologies/2021/4/UnivFAQ#DD_Electrical_Engineering"/>
        <UnivFAQ:offers rdf:resource="http://www.semanticweb.org/suhaspai/ontologies/2021/4/UnivFAQ#EE3002"/>
        <UnivFAQ:offers rdf:resource="http://www.semanticweb.org/suhaspai/ontologies/2021/4/UnivFAQ#EE6112"/>
        <UnivFAQ:offers rdf:resource="http://www.semanticweb.org/suhaspai/ontologies/2021/4/UnivFAQ#EE6150"/>
        <UnivFAQ:offers rdf:resource="http://www.semanticweb.org/suhaspai/ontologies/2021/4/UnivFAQ#MTech._Electrical_Engineering"/>
        <UnivFAQ:offers rdf:resource="http://www.semanticweb.org/suhaspai/ontologies/2021/4/UnivFAQ#PHD._Electrical_Engineering"/>
        <rdfs:comment>The Electrical Engineering department was established in 1959. We currently have about 1000 students, 60 faculty members, 30 supporting staff members and 2 post-doctoral fellows with us.

We perform a variety of research work from absolute fundamentals to component design to system integration to deployment/commercialisation. We have strong industry interaction and have been involved in development of state-of-art products. We house extensive fabrication, calibration and testing facilities for carrying out academic projects, sponsored research and consultancy projects.</rdfs:comment>
        <rdfs:label>Electrical Engineering Department</rdfs:label>
    </owl:NamedIndividual>
    


    <!-- http://www.semanticweb.org/suhaspai/ontologies/2021/4/UnivFAQ#Faster_parameterized_algorithms_using_linear_programming -->

    <owl:NamedIndividual rdf:about="http://www.semanticweb.org/suhaspai/ontologies/2021/4/UnivFAQ#Faster_parameterized_algorithms_using_linear_programming">
        <rdf:type rdf:resource="http://www.semanticweb.org/suhaspai/ontologies/2021/4/UnivFAQ#Publication"/>
        <UnivFAQ:inResearchField rdf:resource="http://www.semanticweb.org/suhaspai/ontologies/2021/4/UnivFAQ#Theoretical_Computer_Science"/>
        <UnivFAQ:publishedBy rdf:resource="http://www.semanticweb.org/suhaspai/ontologies/2021/4/UnivFAQ#N_S_Narayanaswamy"/>
        <rdfs:label>Faster parameterized algorithms using linear programming</rdfs:label>
    </owl:NamedIndividual>
    


    <!-- http://www.semanticweb.org/suhaspai/ontologies/2021/4/UnivFAQ#Fault_Diagnosis_and_Prognosis -->

    <owl:NamedIndividual rdf:about="http://www.semanticweb.org/suhaspai/ontologies/2021/4/UnivFAQ#Fault_Diagnosis_and_Prognosis">
        <rdf:type rdf:resource="http://www.semanticweb.org/suhaspai/ontologies/2021/4/UnivFAQ#ResearchFields"/>
        <rdfs:comment>Prognosis is the capability to use available observations to predict upcoming states of machine or forecast the fault before it occurs.</rdfs:comment>
        <rdfs:label>Fault Diagnosis and Prognosis</rdfs:label>
    </owl:NamedIndividual>
    


    <!-- http://www.semanticweb.org/suhaspai/ontologies/2021/4/UnivFAQ#Fault_detection_in_rotor_bearing_systems_using_time_frequency_techniques -->

    <owl:NamedIndividual rdf:about="http://www.semanticweb.org/suhaspai/ontologies/2021/4/UnivFAQ#Fault_detection_in_rotor_bearing_systems_using_time_frequency_techniques">
        <rdf:type rdf:resource="http://www.semanticweb.org/suhaspai/ontologies/2021/4/UnivFAQ#Publication"/>
        <UnivFAQ:inResearchField rdf:resource="http://www.semanticweb.org/suhaspai/ontologies/2021/4/UnivFAQ#Rotordynamics"/>
        <UnivFAQ:publishedBy rdf:resource="http://www.semanticweb.org/suhaspai/ontologies/2021/4/UnivFAQ#A_Seshadri_Sekhar"/>
        <rdfs:label>Fault detection in rotor bearing systems using time frequency techniques</rdfs:label>
    </owl:NamedIndividual>
    


    <!-- http://www.semanticweb.org/suhaspai/ontologies/2021/4/UnivFAQ#Fluid_Mechanics -->

    <owl:NamedIndividual rdf:about="http://www.semanticweb.org/suhaspai/ontologies/2021/4/UnivFAQ#Fluid_Mechanics">
        <rdf:type rdf:resource="http://www.semanticweb.org/suhaspai/ontologies/2021/4/UnivFAQ#ResearchFields"/>
        <rdfs:comment>Fluid mechanics is the branch of physics concerned with the mechanics of fluids and the forces on them.</rdfs:comment>
        <rdfs:label>Fluid Mechanics</rdfs:label>
    </owl:NamedIndividual>
    


    <!-- http://www.semanticweb.org/suhaspai/ontologies/2021/4/UnivFAQ#GATE -->

    <owl:NamedIndividual rdf:about="http://www.semanticweb.org/suhaspai/ontologies/2021/4/UnivFAQ#GATE">
        <rdf:type rdf:resource="http://www.semanticweb.org/suhaspai/ontologies/2021/4/UnivFAQ#StandardizedTests"/>
        <rdfs:comment>Candidate must have passed the GATE exam.</rdfs:comment>
        <rdfs:label>GATE</rdfs:label>
    </owl:NamedIndividual>
    


    <!-- http://www.semanticweb.org/suhaspai/ontologies/2021/4/UnivFAQ#Genetic_Algorithms -->

    <owl:NamedIndividual rdf:about="http://www.semanticweb.org/suhaspai/ontologies/2021/4/UnivFAQ#Genetic_Algorithms">
        <rdf:type rdf:resource="http://www.semanticweb.org/suhaspai/ontologies/2021/4/UnivFAQ#ResearchFields"/>
        <rdfs:label>Genetic Algorithms</rdfs:label>
    </owl:NamedIndividual>
    


    <!-- http://www.semanticweb.org/suhaspai/ontologies/2021/4/UnivFAQ#HTTP_Lab -->

    <owl:NamedIndividual rdf:about="http://www.semanticweb.org/suhaspai/ontologies/2021/4/UnivFAQ#HTTP_Lab">
        <rdf:type rdf:resource="http://www.semanticweb.org/suhaspai/ontologies/2021/4/UnivFAQ#InstituteFacilities"/>
        <rdfs:comment>Heat Transfer and Thermal Power Labarotory.

-Studies on Thermal Conductivity of Two-Phase Systems
-Porous Medium and Biological Transport Process Studies
-Nano to Macro Scale Heat Transport Studies
-Nanofluid, Bio-MEMS and Microfluidics Studies
-Multi-Mode and Inverse Heat Transfer Studies
-Fluidized Bed Combustion Studies for Biomass and Coal</rdfs:comment>
        <rdfs:label>HTTP Lab</rdfs:label>
    </owl:NamedIndividual>
    


    <!-- http://www.semanticweb.org/suhaspai/ontologies/2021/4/UnivFAQ#Himanshu_Goyal -->

    <owl:NamedIndividual rdf:about="http://www.semanticweb.org/suhaspai/ontologies/2021/4/UnivFAQ#Himanshu_Goyal">
        <rdf:type rdf:resource="http://www.semanticweb.org/suhaspai/ontologies/2021/4/UnivFAQ#AssistantProfessor"/>
        <UnivFAQ:isSpecializedIn rdf:resource="http://www.semanticweb.org/suhaspai/ontologies/2021/4/UnivFAQ#Clean_Energy"/>
        <UnivFAQ:teaches rdf:resource="http://www.semanticweb.org/suhaspai/ontologies/2021/4/UnivFAQ#CH5030"/>
        <rdfs:label>Himanshu Goyal</rdfs:label>
    </owl:NamedIndividual>
    


    <!-- http://www.semanticweb.org/suhaspai/ontologies/2021/4/UnivFAQ#IACE_Lab -->

    <owl:NamedIndividual rdf:about="http://www.semanticweb.org/suhaspai/ontologies/2021/4/UnivFAQ#IACE_Lab">
        <rdf:type rdf:resource="http://www.semanticweb.org/suhaspai/ontologies/2021/4/UnivFAQ#InstituteFacilities"/>
        <rdfs:comment>Laboratory for
Intelligent Applications in Chemical Engineering</rdfs:comment>
        <rdfs:label>IACE Lab</rdfs:label>
    </owl:NamedIndividual>
    


    <!-- http://www.semanticweb.org/suhaspai/ontologies/2021/4/UnivFAQ#Information_Theory -->

    <owl:NamedIndividual rdf:about="http://www.semanticweb.org/suhaspai/ontologies/2021/4/UnivFAQ#Information_Theory">
        <rdf:type rdf:resource="http://www.semanticweb.org/suhaspai/ontologies/2021/4/UnivFAQ#ResearchFields"/>
        <rdfs:comment>Information theory is the scientific study of the quantification, storage, and communication of digital information.[1] The field was fundamentally established by the works of Harry Nyquist and Ralph Hartley, in the 1920s, and Claude Shannon in the 1940s. The field is at the intersection of probability theory, statistics, computer science, statistical mechanics, information engineering, and electrical engineering.</rdfs:comment>
        <rdfs:label>Information Theory</rdfs:label>
    </owl:NamedIndividual>
    


    <!-- http://www.semanticweb.org/suhaspai/ontologies/2021/4/UnivFAQ#JEE_Advanced -->

    <owl:NamedIndividual rdf:about="http://www.semanticweb.org/suhaspai/ontologies/2021/4/UnivFAQ#JEE_Advanced">
        <rdf:type rdf:resource="http://www.semanticweb.org/suhaspai/ontologies/2021/4/UnivFAQ#StandardizedTests"/>
        <rdfs:comment>Candidate must have passed JEE Advanced exam</rdfs:comment>
        <rdfs:label>JEE Advanced</rdfs:label>
    </owl:NamedIndividual>
    


    <!-- http://www.semanticweb.org/suhaspai/ontologies/2021/4/UnivFAQ#JEE_Mains -->

    <owl:NamedIndividual rdf:about="http://www.semanticweb.org/suhaspai/ontologies/2021/4/UnivFAQ#JEE_Mains">
        <rdf:type rdf:resource="http://www.semanticweb.org/suhaspai/ontologies/2021/4/UnivFAQ#StandardizedTests"/>
        <rdfs:comment>Candidate must have passed JEE Mains exam.</rdfs:comment>
        <rdfs:label>JEE Mains</rdfs:label>
    </owl:NamedIndividual>
    


    <!-- http://www.semanticweb.org/suhaspai/ontologies/2021/4/UnivFAQ#Krishna_Jagannathan -->

    <owl:NamedIndividual rdf:about="http://www.semanticweb.org/suhaspai/ontologies/2021/4/UnivFAQ#Krishna_Jagannathan">
        <rdf:type rdf:resource="http://www.semanticweb.org/suhaspai/ontologies/2021/4/UnivFAQ#AssociateProfessor"/>
        <UnivFAQ:isSpecializedIn rdf:resource="http://www.semanticweb.org/suhaspai/ontologies/2021/4/UnivFAQ#Network_Control"/>
        <UnivFAQ:isSpecializedIn rdf:resource="http://www.semanticweb.org/suhaspai/ontologies/2021/4/UnivFAQ#Transportation_Networks"/>
        <UnivFAQ:teaches rdf:resource="http://www.semanticweb.org/suhaspai/ontologies/2021/4/UnivFAQ#EE6150"/>
        <UnivFAQ:name rdf:datatype="http://www.w3.org/2001/XMLSchema#string">Krishna Jagannathan</UnivFAQ:name>
        <rdfs:label rdf:datatype="http://www.w3.org/2001/XMLSchema#string">Krishna Jagannathan</rdfs:label>
    </owl:NamedIndividual>
    


    <!-- http://www.semanticweb.org/suhaspai/ontologies/2021/4/UnivFAQ#ME1100 -->

    <owl:NamedIndividual rdf:about="http://www.semanticweb.org/suhaspai/ontologies/2021/4/UnivFAQ#ME1100">
        <rdf:type rdf:resource="http://www.semanticweb.org/suhaspai/ontologies/2021/4/UnivFAQ#Courses"/>
        <UnivFAQ:offeredBy rdf:resource="http://www.semanticweb.org/suhaspai/ontologies/2021/4/UnivFAQ#Mechanical_Engineering"/>
        <rdfs:comment>To learn the first and second laws of thermodynamics and their application to equipment and devices of relevance to mechanical engineering.</rdfs:comment>
        <rdfs:label>Thermodynamics</rdfs:label>
    </owl:NamedIndividual>
    


    <!-- http://www.semanticweb.org/suhaspai/ontologies/2021/4/UnivFAQ#ME1480 -->

    <owl:NamedIndividual rdf:about="http://www.semanticweb.org/suhaspai/ontologies/2021/4/UnivFAQ#ME1480">
        <rdf:type rdf:resource="http://www.semanticweb.org/suhaspai/ontologies/2021/4/UnivFAQ#Courses"/>
        <rdfs:comment>To introduce students to manual and computer aided drawing</rdfs:comment>
        <rdfs:label>Engineering Drawing</rdfs:label>
    </owl:NamedIndividual>
    


    <!-- http://www.semanticweb.org/suhaspai/ontologies/2021/4/UnivFAQ#ME2200 -->

    <owl:NamedIndividual rdf:about="http://www.semanticweb.org/suhaspai/ontologies/2021/4/UnivFAQ#ME2200">
        <rdf:type rdf:resource="http://www.semanticweb.org/suhaspai/ontologies/2021/4/UnivFAQ#Courses"/>
        <UnivFAQ:hasPrerequisite rdf:resource="http://www.semanticweb.org/suhaspai/ontologies/2021/4/UnivFAQ#ME1480"/>
        <rdfs:comment>Fundamental understanding of the correlation between the structure and properties of materials forms an integral part of any successful design. The main objective of this course is to provide a basic knowledge concerning the internal structure of materials, their mechanical properties and various methods to quantify their mechanical integrity and failure criteria. Phases and heat treatment methods to tailor the properties of Fe-C alloys, which forms perhaps the most important set of engineering</rdfs:comment>
        <rdfs:label>Materials and Design</rdfs:label>
    </owl:NamedIndividual>
    


    <!-- http://www.semanticweb.org/suhaspai/ontologies/2021/4/UnivFAQ#ME3302 -->

    <owl:NamedIndividual rdf:about="http://www.semanticweb.org/suhaspai/ontologies/2021/4/UnivFAQ#ME3302">
        <rdf:type rdf:resource="http://www.semanticweb.org/suhaspai/ontologies/2021/4/UnivFAQ#Courses"/>
        <UnivFAQ:offeredBy rdf:resource="http://www.semanticweb.org/suhaspai/ontologies/2021/4/UnivFAQ#Mechanical_Engineering"/>
        <rdfs:comment>To understand the importance of automation in the of field machine tool based manufacturing To get the knowledge of various elements of manufacturing automation – CAD/CAM, sensors, pneumatics, hydraulics, CNC etc To know the product design and manufacturing by considering manufacturing automation</rdfs:comment>
        <rdfs:label>Automation in manufacturing</rdfs:label>
    </owl:NamedIndividual>
    


    <!-- http://www.semanticweb.org/suhaspai/ontologies/2021/4/UnivFAQ#MES_Lab -->

    <owl:NamedIndividual rdf:about="http://www.semanticweb.org/suhaspai/ontologies/2021/4/UnivFAQ#MES_Lab">
        <rdf:type rdf:resource="http://www.semanticweb.org/suhaspai/ontologies/2021/4/UnivFAQ#InstituteFacilities"/>
        <rdfs:comment>The Manufacturing Engineering Section is spread over three laboratories: one housed in the Ranganathan Building, one in the Machine Tool Laboratory in the workshop building, and the third in MSB. We are served by 13 faculty, 5 technical staff and 2 administrative staff.</rdfs:comment>
        <rdfs:label>MES Lab</rdfs:label>
    </owl:NamedIndividual>
    


    <!-- http://www.semanticweb.org/suhaspai/ontologies/2021/4/UnivFAQ#MTech._Computer_Science -->

    <owl:NamedIndividual rdf:about="http://www.semanticweb.org/suhaspai/ontologies/2021/4/UnivFAQ#MTech._Computer_Science">
        <rdf:type rdf:resource="http://www.semanticweb.org/suhaspai/ontologies/2021/4/UnivFAQ#MTech."/>
        <UnivFAQ:hasAdmissionRequisites rdf:resource="http://www.semanticweb.org/suhaspai/ontologies/2021/4/UnivFAQ#GATE"/>
        <UnivFAQ:hasAdmissionRequisites rdf:resource="http://www.semanticweb.org/suhaspai/ontologies/2021/4/UnivFAQ#Undergraduates_With_BTech"/>
        <UnivFAQ:offeredBy rdf:resource="http://www.semanticweb.org/suhaspai/ontologies/2021/4/UnivFAQ#Computer_Science"/>
        <rdfs:comment>The M.Tech. program is a two-year course oriented graduate program. The student has to take a set of core courses and a set of electives. The course work is spread accross the first two semesters with an option of taking one elective in the third semester. This is followed by a project in the third and fourth semester in which the student can take up a project of his or her interest, supervised by a faculty member.</rdfs:comment>
        <rdfs:label>MTech. Computer Science</rdfs:label>
    </owl:NamedIndividual>
    


    <!-- http://www.semanticweb.org/suhaspai/ontologies/2021/4/UnivFAQ#MTech._Electrical_Engineering -->

    <owl:NamedIndividual rdf:about="http://www.semanticweb.org/suhaspai/ontologies/2021/4/UnivFAQ#MTech._Electrical_Engineering">
        <rdf:type rdf:resource="http://www.semanticweb.org/suhaspai/ontologies/2021/4/UnivFAQ#MTech."/>
        <rdfs:comment>The four-semester M.Tech programmes offered in various disciplines and programmes by different departments of the institute are based on the credit system and provide a student with a wide choice of courses. Each programme comprises several core and elective courses, project work and has a faculty advisor to help the students in the choice of academic options for elective courses. Students may be permitted to do their project work in industries and other approved organizations.</rdfs:comment>
        <rdfs:label>MTech. Electrical Engineering</rdfs:label>
    </owl:NamedIndividual>
    


    <!-- http://www.semanticweb.org/suhaspai/ontologies/2021/4/UnivFAQ#Machine_Learning -->

    <owl:NamedIndividual rdf:about="http://www.semanticweb.org/suhaspai/ontologies/2021/4/UnivFAQ#Machine_Learning">
        <rdf:type rdf:resource="http://www.semanticweb.org/suhaspai/ontologies/2021/4/UnivFAQ#ResearchFields"/>
        <rdfs:comment>Machine learning is the study of computer algorithms that can improve automatically through experience and by the use of data. It is seen as a part of artificial intelligence</rdfs:comment>
        <rdfs:label>Machine Learning</rdfs:label>
    </owl:NamedIndividual>
    


    <!-- http://www.semanticweb.org/suhaspai/ontologies/2021/4/UnivFAQ#Mechanical_Engineering -->

    <owl:NamedIndividual rdf:about="http://www.semanticweb.org/suhaspai/ontologies/2021/4/UnivFAQ#Mechanical_Engineering">
        <rdf:type rdf:resource="http://www.semanticweb.org/suhaspai/ontologies/2021/4/UnivFAQ#Department"/>
        <UnivFAQ:hasFacility rdf:resource="http://www.semanticweb.org/suhaspai/ontologies/2021/4/UnivFAQ#HTTP_Lab"/>
        <UnivFAQ:hasFacility rdf:resource="http://www.semanticweb.org/suhaspai/ontologies/2021/4/UnivFAQ#MES_Lab"/>
        <UnivFAQ:offers rdf:resource="http://www.semanticweb.org/suhaspai/ontologies/2021/4/UnivFAQ#ME1480"/>
        <UnivFAQ:offers rdf:resource="http://www.semanticweb.org/suhaspai/ontologies/2021/4/UnivFAQ#ME2200"/>
        <rdfs:comment>Mechanical Engineering is one of the major activities in the engineering profession and its principles are involved in the design, study, development and construction of nearly all of the physical devices and systems. Continued research and development have led to better machines and processes helping the mankind.

The Department of Mechanical Engineering at IIT Madras is as old as the Institute itself. Its impact on the institute and on society is easily demonstrated by noting the alignment of the department&apos;s evolution with key events and technological advances in the India and elsewhere. Today, the department of Mechanical engineering of IIT Madras attracts and features an extraordinary rich diversity and quantity of talented individuals, with nearly 700 undergraduates, 500 graduate students and over 60 faculty members. The impressive array of students makes the department as the largest in the country and one of the largest in Asia.

In addition to teaching undergraduate and graduate students, the faculty of Mechanical Engineering actively pursues research through graduate students. The current graduate students include nearly 150 Master of Technology students (M.Tech), 170 Master of Science (by research) students (M.S.) and 300 students pursuing their doctoral programme (Ph.D).</rdfs:comment>
        <rdfs:label>Mechanical Engineering Department</rdfs:label>
    </owl:NamedIndividual>
    


    <!-- http://www.semanticweb.org/suhaspai/ontologies/2021/4/UnivFAQ#Microelectronics_and_MEMS_laboratory -->

    <owl:NamedIndividual rdf:about="http://www.semanticweb.org/suhaspai/ontologies/2021/4/UnivFAQ#Microelectronics_and_MEMS_laboratory">
        <rdfs:comment>Microelectronics and MEMS Lab is well-equipped for semiconductor device and MEMS fabrication, characterization, modeling and simulation. It has Class-100 and Class-1000 clean rooms which house the major facilities that include a Mask writer, double-sided lithography facility, substrate bond aligner, LPCVD for polysilicon deposition, PECVD for dielectrics, diffusion furnaces, e-beam metallization unit and RIE for dry etching. DC and RF probe stations, parametric analyzer and LCR meter are used for electrical characterization, while a non-contact surface profiler and ellipsometer are used for process characterization. ATLAS, SenTaurus, Coventorware and Intellisuite are some of the commercial softwares used for simulation. The facilities have been used for fabrication and characterization of devices based on Silicon, GaAs and InP based materials, and for modeling various types of devices as listed below. Some activity has also been initiated on GaN and silicon based photonic devices. A wide array of devices, e.g. polysilicon gate n-channel MOSFETs, bipolar junction transistors, pressure sensors with integrated amplifiers, GaAs MESFETs, pigtailed InGaAs/InP PIN photodiodes and variable optical attenuators have been fabricated in the laboratory.</rdfs:comment>
        <rdfs:label>Microelectronics and MEMS laboratory</rdfs:label>
    </owl:NamedIndividual>
    


    <!-- http://www.semanticweb.org/suhaspai/ontologies/2021/4/UnivFAQ#N_S_Narayanaswamy -->

    <owl:NamedIndividual rdf:about="http://www.semanticweb.org/suhaspai/ontologies/2021/4/UnivFAQ#N_S_Narayanaswamy">
        <rdf:type rdf:resource="http://www.semanticweb.org/suhaspai/ontologies/2021/4/UnivFAQ#Professor"/>
        <UnivFAQ:isSpecializedIn rdf:resource="http://www.semanticweb.org/suhaspai/ontologies/2021/4/UnivFAQ#Artificial_Intelligence"/>
        <UnivFAQ:isSpecializedIn rdf:resource="http://www.semanticweb.org/suhaspai/ontologies/2021/4/UnivFAQ#Theoretical_Computer_Science"/>
        <UnivFAQ:teaches rdf:resource="http://www.semanticweb.org/suhaspai/ontologies/2021/4/UnivFAQ#CS1200"/>
        <UnivFAQ:name rdf:datatype="http://www.w3.org/2001/XMLSchema#string">N.S. Narayanaswamy</UnivFAQ:name>
        <rdfs:label rdf:datatype="http://www.w3.org/2001/XMLSchema#string">N.S. Narayanaswamy</rdfs:label>
    </owl:NamedIndividual>
    


    <!-- http://www.semanticweb.org/suhaspai/ontologies/2021/4/UnivFAQ#Network_Control -->

    <owl:NamedIndividual rdf:about="http://www.semanticweb.org/suhaspai/ontologies/2021/4/UnivFAQ#Network_Control">
        <rdf:type rdf:resource="http://www.semanticweb.org/suhaspai/ontologies/2021/4/UnivFAQ#ResearchFields"/>
        <rdfs:comment>A Networked Control System (NCS) is a control system wherein the control loops are closed through a communication network. The defining feature of an NCS is that control and feedback signals are exchanged among the system&apos;s components in the form of information packages through a network.</rdfs:comment>
        <rdfs:label>Network Control</rdfs:label>
    </owl:NamedIndividual>
    


    <!-- http://www.semanticweb.org/suhaspai/ontologies/2021/4/UnivFAQ#Online_handwritten_character_recognition_of_devanagari_and_telugu_characters_using_support_vector_machines -->

    <owl:NamedIndividual rdf:about="http://www.semanticweb.org/suhaspai/ontologies/2021/4/UnivFAQ#Online_handwritten_character_recognition_of_devanagari_and_telugu_characters_using_support_vector_machines">
        <rdf:type rdf:resource="http://www.semanticweb.org/suhaspai/ontologies/2021/4/UnivFAQ#Publication"/>
        <UnivFAQ:inResearchField rdf:resource="http://www.semanticweb.org/suhaspai/ontologies/2021/4/UnivFAQ#Reinforcement_Learning"/>
        <UnivFAQ:publishedBy rdf:resource="http://www.semanticweb.org/suhaspai/ontologies/2021/4/UnivFAQ#Chandra_Sekhar"/>
        <rdfs:label>Online handwritten character recognition of devanagari and telugu characters using support vector machines</rdfs:label>
    </owl:NamedIndividual>
    


    <!-- http://www.semanticweb.org/suhaspai/ontologies/2021/4/UnivFAQ#Ontologies_and_Application -->

    <owl:NamedIndividual rdf:about="http://www.semanticweb.org/suhaspai/ontologies/2021/4/UnivFAQ#Ontologies_and_Application">
        <rdf:type rdf:resource="http://www.semanticweb.org/suhaspai/ontologies/2021/4/UnivFAQ#ResearchFields"/>
        <rdfs:comment>An ontology is the specification of conceptualizations, used to help programs and humans share knowledge. An Ontology is a formal and explicit specification of a shared conceptualization.</rdfs:comment>
        <rdfs:label>Ontologies and Applications</rdfs:label>
    </owl:NamedIndividual>
    


    <!-- http://www.semanticweb.org/suhaspai/ontologies/2021/4/UnivFAQ#PACE_Lab -->

    <owl:NamedIndividual rdf:about="http://www.semanticweb.org/suhaspai/ontologies/2021/4/UnivFAQ#PACE_Lab">
        <rdf:type rdf:resource="http://www.semanticweb.org/suhaspai/ontologies/2021/4/UnivFAQ#InstituteFacilities"/>
        <rdfs:comment>Programming Languages, Architecture and Compilers Education Laboratory</rdfs:comment>
        <rdfs:label>PACE Lab</rdfs:label>
    </owl:NamedIndividual>
    


    <!-- http://www.semanticweb.org/suhaspai/ontologies/2021/4/UnivFAQ#PHD._Chemical_Engineering -->

    <owl:NamedIndividual rdf:about="http://www.semanticweb.org/suhaspai/ontologies/2021/4/UnivFAQ#PHD._Chemical_Engineering">
        <rdf:type rdf:resource="http://www.semanticweb.org/suhaspai/ontologies/2021/4/UnivFAQ#PhD"/>
        <UnivFAQ:offeredBy rdf:resource="http://www.semanticweb.org/suhaspai/ontologies/2021/4/UnivFAQ#Chemical_Engineering"/>
        <rdfs:comment>PhD. programs are postgraduate research oriented programs. The scholar works in an area of his/her interest under the supervision of a faculty member. The scholar has to obtain a minimum number of credits by taking courses. The highlight of the program is the independent research work taken by scholar, leading to a dissertation at the end of the program. The average duration of a PhD. program is between four to five years.</rdfs:comment>
        <rdfs:label>PHD Chemical Engineering</rdfs:label>
    </owl:NamedIndividual>
    


    <!-- http://www.semanticweb.org/suhaspai/ontologies/2021/4/UnivFAQ#PHD._Computer_Science -->

    <owl:NamedIndividual rdf:about="http://www.semanticweb.org/suhaspai/ontologies/2021/4/UnivFAQ#PHD._Computer_Science">
        <rdf:type rdf:resource="http://www.semanticweb.org/suhaspai/ontologies/2021/4/UnivFAQ#PhD"/>
        <UnivFAQ:offeredBy rdf:resource="http://www.semanticweb.org/suhaspai/ontologies/2021/4/UnivFAQ#Computer_Science"/>
        <rdfs:comment>PhD. programs are postgraduate research oriented programs. The scholar works in an area of his/her interest under the supervision of a faculty member. The scholar has to obtain a minimum number of credits by taking courses. The highlight of the program is the independent research work taken by scholar, leading to a dissertation at the end of the program. The average duration of a PhD. program is between four to five years.</rdfs:comment>
        <rdfs:label>PHD. Computer Science</rdfs:label>
    </owl:NamedIndividual>
    


    <!-- http://www.semanticweb.org/suhaspai/ontologies/2021/4/UnivFAQ#PHD._Electrical_Engineering -->

    <owl:NamedIndividual rdf:about="http://www.semanticweb.org/suhaspai/ontologies/2021/4/UnivFAQ#PHD._Electrical_Engineering">
        <rdf:type rdf:resource="http://www.semanticweb.org/suhaspai/ontologies/2021/4/UnivFAQ#PhD"/>
        <rdfs:comment>Course work :   Introduction to Research (ID 6020), two core courses and two elective courses. The core courses and list of electives are prescribed individually for each student by the Doctoral Committee (DC). ID 6020 is a compulsory course for all Ph.D. students and is usually taken in the first semester. The courses must be completed within three semesters after enrollment into the Ph.D.

Comprehensive exam :   All students must clear the comprehensive exam within the one and half years of joining the program. Details of the comprehensive exam are provided on the department web site (see the useful links section below).

Research :    All students are expected to do high quality research resulting in publications in reputed international journals.</rdfs:comment>
        <rdfs:label>PHD Electrical Engineering</rdfs:label>
    </owl:NamedIndividual>
    


    <!-- http://www.semanticweb.org/suhaspai/ontologies/2021/4/UnivFAQ#PHD._Mechanical_Engineering -->

    <owl:NamedIndividual rdf:about="http://www.semanticweb.org/suhaspai/ontologies/2021/4/UnivFAQ#PHD._Mechanical_Engineering">
        <rdf:type rdf:resource="http://www.semanticweb.org/suhaspai/ontologies/2021/4/UnivFAQ#PhD"/>
        <UnivFAQ:offeredBy rdf:resource="http://www.semanticweb.org/suhaspai/ontologies/2021/4/UnivFAQ#Mechanical_Engineering"/>
        <rdfs:comment>PhD. programs are postgraduate research oriented programs. The scholar works in an area of his/her interest under the supervision of a faculty member. The scholar has to obtain a minimum number of credits by taking courses. The highlight of the program is the independent research work taken by scholar, leading to a dissertation at the end of the program. The average duration of a PhD. program is between four to five years.</rdfs:comment>
        <rdfs:label>PHD Mechanical Engineering</rdfs:label>
    </owl:NamedIndividual>
    


    <!-- http://www.semanticweb.org/suhaspai/ontologies/2021/4/UnivFAQ#Photocatalytic_degradation_of_gaseous_organic_species_on_photonic_band-gap_titania -->

    <owl:NamedIndividual rdf:about="http://www.semanticweb.org/suhaspai/ontologies/2021/4/UnivFAQ#Photocatalytic_degradation_of_gaseous_organic_species_on_photonic_band-gap_titania">
        <rdf:type rdf:resource="http://www.semanticweb.org/suhaspai/ontologies/2021/4/UnivFAQ#Publication"/>
        <UnivFAQ:inResearchField rdf:resource="http://www.semanticweb.org/suhaspai/ontologies/2021/4/UnivFAQ#Treatment_and_Control_Processes"/>
        <UnivFAQ:publishedBy rdf:resource="http://www.semanticweb.org/suhaspai/ontologies/2021/4/UnivFAQ#R_Ravi_Krishna"/>
        <rdfs:label>Photocatalytic degradation of gaseous organic species on photonic band-gap titania</rdfs:label>
    </owl:NamedIndividual>
    


    <!-- http://www.semanticweb.org/suhaspai/ontologies/2021/4/UnivFAQ#Piyush_Shakya -->

    <owl:NamedIndividual rdf:about="http://www.semanticweb.org/suhaspai/ontologies/2021/4/UnivFAQ#Piyush_Shakya">
        <rdf:type rdf:resource="http://www.semanticweb.org/suhaspai/ontologies/2021/4/UnivFAQ#AssistantProfessor"/>
        <UnivFAQ:isSpecializedIn rdf:resource="http://www.semanticweb.org/suhaspai/ontologies/2021/4/UnivFAQ#Fault_Diagnosis_and_Prognosis"/>
        <UnivFAQ:teaches rdf:resource="http://www.semanticweb.org/suhaspai/ontologies/2021/4/UnivFAQ#ME1480"/>
        <UnivFAQ:name rdf:datatype="http://www.w3.org/2001/XMLSchema#string">Piyush Shakya</UnivFAQ:name>
        <rdfs:label rdf:datatype="http://www.w3.org/2001/XMLSchema#string">Piyush Shakya</rdfs:label>
    </owl:NamedIndividual>
    


    <!-- http://www.semanticweb.org/suhaspai/ontologies/2021/4/UnivFAQ#Preeti_Aghalayam -->

    <owl:NamedIndividual rdf:about="http://www.semanticweb.org/suhaspai/ontologies/2021/4/UnivFAQ#Preeti_Aghalayam">
        <rdf:type rdf:resource="http://www.semanticweb.org/suhaspai/ontologies/2021/4/UnivFAQ#Professor"/>
        <UnivFAQ:isSpecializedIn rdf:resource="http://www.semanticweb.org/suhaspai/ontologies/2021/4/UnivFAQ#Underground_Coal_Gasification"/>
        <rdfs:label>Preeti Aghalayam</rdfs:label>
    </owl:NamedIndividual>
    


    <!-- http://www.semanticweb.org/suhaspai/ontologies/2021/4/UnivFAQ#Process_System_Engineering -->

    <owl:NamedIndividual rdf:about="http://www.semanticweb.org/suhaspai/ontologies/2021/4/UnivFAQ#Process_System_Engineering">
        <rdf:type rdf:resource="http://www.semanticweb.org/suhaspai/ontologies/2021/4/UnivFAQ#ResearchFields"/>
        <rdfs:comment>Process Systems Engineering (PSEng) is a broad category of engineering that deals with the process design for the purpose of converting raw goods to usable end products, including energy</rdfs:comment>
        <rdfs:label>Process System Engineering</rdfs:label>
    </owl:NamedIndividual>
    


    <!-- http://www.semanticweb.org/suhaspai/ontologies/2021/4/UnivFAQ#RFIC_Design -->

    <owl:NamedIndividual rdf:about="http://www.semanticweb.org/suhaspai/ontologies/2021/4/UnivFAQ#RFIC_Design">
        <rdf:type rdf:resource="http://www.semanticweb.org/suhaspai/ontologies/2021/4/UnivFAQ#ResearchFields"/>
        <rdfs:comment>RF IC design, much like niche areas of analog IC design, is often a custom process that is aided by one, or often, many EDA tools. Part of the precise nature of RF IC design is that parasitics and packaging characteristics have first-order impact on the performance of RF circuits. Therefore, RF IC design is often an iterative process that involves the extensive use of EM simulation, parasitic modeling, and package modeling throughout the IC design process.</rdfs:comment>
        <rdfs:label>RFIC Design</rdfs:label>
    </owl:NamedIndividual>
    


    <!-- http://www.semanticweb.org/suhaspai/ontologies/2021/4/UnivFAQ#R_Ravi_Krishna -->

    <owl:NamedIndividual rdf:about="http://www.semanticweb.org/suhaspai/ontologies/2021/4/UnivFAQ#R_Ravi_Krishna">
        <rdf:type rdf:resource="http://www.semanticweb.org/suhaspai/ontologies/2021/4/UnivFAQ#AssociateProfessor"/>
        <UnivFAQ:headsDepartment rdf:resource="http://www.semanticweb.org/suhaspai/ontologies/2021/4/UnivFAQ#Chemical_Engineering"/>
        <UnivFAQ:isSpecializedIn rdf:resource="http://www.semanticweb.org/suhaspai/ontologies/2021/4/UnivFAQ#Treatment_and_Control_Processes"/>
        <UnivFAQ:teaches rdf:resource="http://www.semanticweb.org/suhaspai/ontologies/2021/4/UnivFAQ#CH5370"/>
        <UnivFAQ:name rdf:datatype="http://www.w3.org/2001/XMLSchema#string">R Ravi Krishna</UnivFAQ:name>
        <rdfs:label rdf:datatype="http://www.w3.org/2001/XMLSchema#string">R Ravi Krishna</rdfs:label>
    </owl:NamedIndividual>
    


    <!-- http://www.semanticweb.org/suhaspai/ontologies/2021/4/UnivFAQ#Rajagopalan_Srinivasan -->

    <owl:NamedIndividual rdf:about="http://www.semanticweb.org/suhaspai/ontologies/2021/4/UnivFAQ#Rajagopalan_Srinivasan">
        <rdf:type rdf:resource="http://www.semanticweb.org/suhaspai/ontologies/2021/4/UnivFAQ#Professor"/>
        <UnivFAQ:isSpecializedIn rdf:resource="http://www.semanticweb.org/suhaspai/ontologies/2021/4/UnivFAQ#Process_System_Engineering"/>
        <UnivFAQ:teaches rdf:resource="http://www.semanticweb.org/suhaspai/ontologies/2021/4/UnivFAQ#CH4250"/>
        <rdfs:label>Rajagopalan Srinivasan</rdfs:label>
    </owl:NamedIndividual>
    


    <!-- http://www.semanticweb.org/suhaspai/ontologies/2021/4/UnivFAQ#Reinforcement_Learning -->

    <owl:NamedIndividual rdf:about="http://www.semanticweb.org/suhaspai/ontologies/2021/4/UnivFAQ#Reinforcement_Learning">
        <rdf:type rdf:resource="http://www.semanticweb.org/suhaspai/ontologies/2021/4/UnivFAQ#ResearchFields"/>
        <rdfs:label>Reinforcement Learning</rdfs:label>
    </owl:NamedIndividual>
    


    <!-- http://www.semanticweb.org/suhaspai/ontologies/2021/4/UnivFAQ#Rotordynamics -->

    <owl:NamedIndividual rdf:about="http://www.semanticweb.org/suhaspai/ontologies/2021/4/UnivFAQ#Rotordynamics">
        <rdf:type rdf:resource="http://www.semanticweb.org/suhaspai/ontologies/2021/4/UnivFAQ#ResearchFields"/>
        <rdfs:comment>Rotordynamics, also known as rotor dynamics, is a specialized branch of applied mechanics concerned with the behavior and diagnosis of rotating structures.</rdfs:comment>
        <rdfs:label>Rotordynamics</rdfs:label>
    </owl:NamedIndividual>
    


    <!-- http://www.semanticweb.org/suhaspai/ontologies/2021/4/UnivFAQ#Rupesh_Nasre -->

    <owl:NamedIndividual rdf:about="http://www.semanticweb.org/suhaspai/ontologies/2021/4/UnivFAQ#Rupesh_Nasre">
        <rdf:type rdf:resource="http://www.semanticweb.org/suhaspai/ontologies/2021/4/UnivFAQ#AssociateProfessor"/>
        <UnivFAQ:isSpecializedIn rdf:resource="http://www.semanticweb.org/suhaspai/ontologies/2021/4/UnivFAQ#Compilers"/>
        <UnivFAQ:teaches rdf:resource="http://www.semanticweb.org/suhaspai/ontologies/2021/4/UnivFAQ#CS6023"/>
        <UnivFAQ:name rdf:datatype="http://www.w3.org/2001/XMLSchema#string">Rupesh Nasre</UnivFAQ:name>
        <rdfs:label rdf:datatype="http://www.w3.org/2001/XMLSchema#string">Rupesh Nasre</rdfs:label>
    </owl:NamedIndividual>
    


    <!-- http://www.semanticweb.org/suhaspai/ontologies/2021/4/UnivFAQ#S_Aniruddhan -->

    <owl:NamedIndividual rdf:about="http://www.semanticweb.org/suhaspai/ontologies/2021/4/UnivFAQ#S_Aniruddhan">
        <rdf:type rdf:resource="http://www.semanticweb.org/suhaspai/ontologies/2021/4/UnivFAQ#AssociateProfessor"/>
        <UnivFAQ:isSpecializedIn rdf:resource="http://www.semanticweb.org/suhaspai/ontologies/2021/4/UnivFAQ#Analog"/>
        <UnivFAQ:isSpecializedIn rdf:resource="http://www.semanticweb.org/suhaspai/ontologies/2021/4/UnivFAQ#RFIC_Design"/>
        <UnivFAQ:teaches rdf:resource="http://www.semanticweb.org/suhaspai/ontologies/2021/4/UnivFAQ#EE3002"/>
        <UnivFAQ:name rdf:datatype="http://www.w3.org/2001/XMLSchema#string">S Aniruddhan</UnivFAQ:name>
        <rdfs:label rdf:datatype="http://www.w3.org/2001/XMLSchema#string">S Aniruddhan</rdfs:label>
    </owl:NamedIndividual>
    


    <!-- http://www.semanticweb.org/suhaspai/ontologies/2021/4/UnivFAQ#Sathyan_Subbiah -->

    <owl:NamedIndividual rdf:about="http://www.semanticweb.org/suhaspai/ontologies/2021/4/UnivFAQ#Sathyan_Subbiah">
        <rdf:type rdf:resource="http://www.semanticweb.org/suhaspai/ontologies/2021/4/UnivFAQ#Professor"/>
        <UnivFAQ:isSpecializedIn rdf:resource="http://www.semanticweb.org/suhaspai/ontologies/2021/4/UnivFAQ#Automation_In_Manufacturing_Research"/>
        <UnivFAQ:teaches rdf:resource="http://www.semanticweb.org/suhaspai/ontologies/2021/4/UnivFAQ#ME3302"/>
        <rdfs:label>Sathyan Subbiah</rdfs:label>
    </owl:NamedIndividual>
    


    <!-- http://www.semanticweb.org/suhaspai/ontologies/2021/4/UnivFAQ#Scheduling_policies_for_minimizing_age_of_information_in_broadcast_wireless_networks -->

    <owl:NamedIndividual rdf:about="http://www.semanticweb.org/suhaspai/ontologies/2021/4/UnivFAQ#Scheduling_policies_for_minimizing_age_of_information_in_broadcast_wireless_networks">
        <rdf:type rdf:resource="http://www.semanticweb.org/suhaspai/ontologies/2021/4/UnivFAQ#Publication"/>
        <UnivFAQ:inResearchField rdf:resource="http://www.semanticweb.org/suhaspai/ontologies/2021/4/UnivFAQ#Network_Control"/>
        <UnivFAQ:publishedBy rdf:resource="http://www.semanticweb.org/suhaspai/ontologies/2021/4/UnivFAQ#Abishek_Sinha"/>
        <rdfs:label>Scheduling policies for minimizing age of information in broadcast wireless networks</rdfs:label>
    </owl:NamedIndividual>
    


    <!-- http://www.semanticweb.org/suhaspai/ontologies/2021/4/UnivFAQ#Scholarship_1 -->

    <owl:NamedIndividual rdf:about="http://www.semanticweb.org/suhaspai/ontologies/2021/4/UnivFAQ#Scholarship_1"/>
    


    <!-- http://www.semanticweb.org/suhaspai/ontologies/2021/4/UnivFAQ#Shweta_Agarwal -->

    <owl:NamedIndividual rdf:about="http://www.semanticweb.org/suhaspai/ontologies/2021/4/UnivFAQ#Shweta_Agarwal">
        <rdf:type rdf:resource="http://www.semanticweb.org/suhaspai/ontologies/2021/4/UnivFAQ#AssociateProfessor"/>
        <UnivFAQ:isSpecializedIn rdf:resource="http://www.semanticweb.org/suhaspai/ontologies/2021/4/UnivFAQ#Cryptography"/>
        <UnivFAQ:teaches rdf:resource="http://www.semanticweb.org/suhaspai/ontologies/2021/4/UnivFAQ#CS2800"/>
        <UnivFAQ:name rdf:datatype="http://www.w3.org/2001/XMLSchema#string">Shweta Agarwal</UnivFAQ:name>
        <rdfs:comment>Cryptography, or cryptology, is the practice and study of techniques for secure communication in the presence of adversarial behavior.</rdfs:comment>
        <rdfs:label rdf:datatype="http://www.w3.org/2001/XMLSchema#string">Shweta Agarwal</rdfs:label>
    </owl:NamedIndividual>
    


    <!-- http://www.semanticweb.org/suhaspai/ontologies/2021/4/UnivFAQ#Sreenivasa_Kumar -->

    <owl:NamedIndividual rdf:about="http://www.semanticweb.org/suhaspai/ontologies/2021/4/UnivFAQ#Sreenivasa_Kumar">
        <rdf:type rdf:resource="http://www.semanticweb.org/suhaspai/ontologies/2021/4/UnivFAQ#Professor"/>
        <UnivFAQ:isSpecializedIn rdf:resource="http://www.semanticweb.org/suhaspai/ontologies/2021/4/UnivFAQ#Ontologies_and_Application"/>
        <UnivFAQ:teaches rdf:resource="http://www.semanticweb.org/suhaspai/ontologies/2021/4/UnivFAQ#CS3700"/>
        <UnivFAQ:teaches rdf:resource="http://www.semanticweb.org/suhaspai/ontologies/2021/4/UnivFAQ#CS6852"/>
        <UnivFAQ:name rdf:datatype="http://www.w3.org/2001/XMLSchema#string">P Sreenivasa Kumar</UnivFAQ:name>
        <rdfs:label rdf:datatype="http://www.w3.org/2001/XMLSchema#string">P Sreenivasa Kumar</rdfs:label>
    </owl:NamedIndividual>
    


    <!-- http://www.semanticweb.org/suhaspai/ontologies/2021/4/UnivFAQ#Suhas_Pai -->

    <owl:NamedIndividual rdf:about="http://www.semanticweb.org/suhaspai/ontologies/2021/4/UnivFAQ#Suhas_Pai">
        <rdf:type rdf:resource="http://www.semanticweb.org/suhaspai/ontologies/2021/4/UnivFAQ#Student"/>
        <UnivFAQ:enrolledIn rdf:resource="http://www.semanticweb.org/suhaspai/ontologies/2021/4/UnivFAQ#DD_Computer_Science"/>
        <UnivFAQ:isAdvisedBy rdf:resource="http://www.semanticweb.org/suhaspai/ontologies/2021/4/UnivFAQ#Sreenivasa_Kumar"/>
        <UnivFAQ:name>Suhas Pai</UnivFAQ:name>
        <rdfs:label>Suhas Pai</rdfs:label>
    </owl:NamedIndividual>
    


    <!-- http://www.semanticweb.org/suhaspai/ontologies/2021/4/UnivFAQ#Suresh_Saharan -->

    <owl:NamedIndividual rdf:about="http://www.semanticweb.org/suhaspai/ontologies/2021/4/UnivFAQ#Suresh_Saharan">
        <rdf:type rdf:resource="http://www.semanticweb.org/suhaspai/ontologies/2021/4/UnivFAQ#Student"/>
        <UnivFAQ:enrolledIn rdf:resource="http://www.semanticweb.org/suhaspai/ontologies/2021/4/UnivFAQ#PHD._Computer_Science"/>
        <UnivFAQ:isAdvisedBy rdf:resource="http://www.semanticweb.org/suhaspai/ontologies/2021/4/UnivFAQ#Sreenivasa_Kumar"/>
        <rdfs:label>Suresh Saharan</rdfs:label>
    </owl:NamedIndividual>
    


    <!-- http://www.semanticweb.org/suhaspai/ontologies/2021/4/UnivFAQ#Theoretical_Computer_Science -->

    <owl:NamedIndividual rdf:about="http://www.semanticweb.org/suhaspai/ontologies/2021/4/UnivFAQ#Theoretical_Computer_Science">
        <rdf:type rdf:resource="http://www.semanticweb.org/suhaspai/ontologies/2021/4/UnivFAQ#ResearchFields"/>
        <rdfs:label>Theoretical Computer Science</rdfs:label>
    </owl:NamedIndividual>
    


    <!-- http://www.semanticweb.org/suhaspai/ontologies/2021/4/UnivFAQ#Transportation_Networks -->

    <owl:NamedIndividual rdf:about="http://www.semanticweb.org/suhaspai/ontologies/2021/4/UnivFAQ#Transportation_Networks">
        <rdf:type rdf:resource="http://www.semanticweb.org/suhaspai/ontologies/2021/4/UnivFAQ#ResearchFields"/>
        <rdfs:comment>A transport network, or transportation network is a network or graph in geographic space, describing an infrastructure that permits and constrains movement or flow. Examples include but are not limited to road networks, railways, air routes, pipelines, aqueducts, and power lines</rdfs:comment>
        <rdfs:label>Transportation Networks</rdfs:label>
    </owl:NamedIndividual>
    


    <!-- http://www.semanticweb.org/suhaspai/ontologies/2021/4/UnivFAQ#Treatment_and_Control_Processes -->

    <owl:NamedIndividual rdf:about="http://www.semanticweb.org/suhaspai/ontologies/2021/4/UnivFAQ#Treatment_and_Control_Processes">
        <rdf:type rdf:resource="http://www.semanticweb.org/suhaspai/ontologies/2021/4/UnivFAQ#ResearchFields"/>
        <rdfs:comment>Process control is the study and application of automatic control in the field of chemical engineering.</rdfs:comment>
        <rdfs:label>Treatment and Control Processes</rdfs:label>
    </owl:NamedIndividual>
    


    <!-- http://www.semanticweb.org/suhaspai/ontologies/2021/4/UnivFAQ#Undergraduates_With_BTech -->

    <owl:NamedIndividual rdf:about="http://www.semanticweb.org/suhaspai/ontologies/2021/4/UnivFAQ#Undergraduates_With_BTech">
        <rdf:type rdf:resource="http://www.semanticweb.org/suhaspai/ontologies/2021/4/UnivFAQ#Qualifications"/>
    </owl:NamedIndividual>
    


    <!-- http://www.semanticweb.org/suhaspai/ontologies/2021/4/UnivFAQ#Underground_Coal_Gasification -->

    <owl:NamedIndividual rdf:about="http://www.semanticweb.org/suhaspai/ontologies/2021/4/UnivFAQ#Underground_Coal_Gasification">
        <rdf:type rdf:resource="http://www.semanticweb.org/suhaspai/ontologies/2021/4/UnivFAQ#ResearchFields"/>
        <rdfs:comment>Underground coal gasification is an industrial process which converts coal into product gas. UCG is an in-situ gasification process, carried out in non-mined coal seams using injection of oxidants and steam.</rdfs:comment>
        <rdfs:label>Underground Coal Gasification</rdfs:label>
    </owl:NamedIndividual>
    


    <!-- http://www.semanticweb.org/suhaspai/ontologies/2021/4/UnivFAQ#VLSI_Lab -->

    <owl:NamedIndividual rdf:about="http://www.semanticweb.org/suhaspai/ontologies/2021/4/UnivFAQ#VLSI_Lab">
        <rdf:type rdf:resource="http://www.semanticweb.org/suhaspai/ontologies/2021/4/UnivFAQ#InstituteFacilities"/>
        <rdfs:comment>Involved in research in the areas of analog, mixed signal, and RF design, analysis and simulation of noise in circuits, VLSI DSP architectures, Programmable Analog Pulse Shaping for Ultra-Wideband Applications and reconfigurable computing.</rdfs:comment>
        <rdfs:label>VLSI Lab</rdfs:label>
    </owl:NamedIndividual>
    


    <!-- http://www.semanticweb.org/suhaspai/ontologies/2021/4/UnivFAQ#V_Sriram -->

    <owl:NamedIndividual rdf:about="http://www.semanticweb.org/suhaspai/ontologies/2021/4/UnivFAQ#V_Sriram">
        <rdf:type rdf:resource="http://www.semanticweb.org/suhaspai/ontologies/2021/4/UnivFAQ#Student"/>
        <UnivFAQ:enrolledIn rdf:resource="http://www.semanticweb.org/suhaspai/ontologies/2021/4/UnivFAQ#BTech._Computer_Science"/>
        <rdfs:label>V Sriram</rdfs:label>
    </owl:NamedIndividual>
    


    <!-- http://www.semanticweb.org/suhaspai/ontologies/2021/4/UnivFAQ#12th_Standard -->

    <owl:NamedIndividual rdf:about="http://www.semanticweb.org/suhaspai/ontologies/2021/4/UnivFAQ#12th_Standard">
        <rdf:type rdf:resource="http://www.semanticweb.org/suhaspai/ontologies/2021/4/UnivFAQ#Qualifications"/>
        <rdfs:comment>Candidate must have a 12th standard pass certificiate from a recognized board.</rdfs:comment>
        <rdfs:label>12th Standard</rdfs:label>
    </owl:NamedIndividual>
    


    <!-- http://www.semanticweb.org/suhaspai/ontologies/2021/4/UnivFAQ#Agent-based_supply_chain_management—1:_framework -->

    <owl:NamedIndividual rdf:about="http://www.semanticweb.org/suhaspai/ontologies/2021/4/UnivFAQ#Agent-based_supply_chain_management—1:_framework">
        <rdf:type rdf:resource="http://www.semanticweb.org/suhaspai/ontologies/2021/4/UnivFAQ#Publication"/>
        <UnivFAQ:inResearchField rdf:resource="http://www.semanticweb.org/suhaspai/ontologies/2021/4/UnivFAQ#Process_System_Engineering"/>
        <UnivFAQ:publishedBy rdf:resource="http://www.semanticweb.org/suhaspai/ontologies/2021/4/UnivFAQ#Rajagopalan_Srinivasan"/>
        <rdfs:label>Agent-based supply chain management—1: framework</rdfs:label>
    </owl:NamedIndividual>
    


    <!-- http://www.semanticweb.org/suhaspai/ontologies/2021/4/UnivFAQ#Bearing_diagnosis_based_on_Mahalanobis–Taguchi–Gram–Schmidt_method -->

    <owl:NamedIndividual rdf:about="http://www.semanticweb.org/suhaspai/ontologies/2021/4/UnivFAQ#Bearing_diagnosis_based_on_Mahalanobis–Taguchi–Gram–Schmidt_method">
        <rdf:type rdf:resource="http://www.semanticweb.org/suhaspai/ontologies/2021/4/UnivFAQ#Publication"/>
        <UnivFAQ:inResearchField rdf:resource="http://www.semanticweb.org/suhaspai/ontologies/2021/4/UnivFAQ#Fault_Diagnosis_and_Prognosis"/>
        <UnivFAQ:publishedBy rdf:resource="http://www.semanticweb.org/suhaspai/ontologies/2021/4/UnivFAQ#Piyush_Shakya"/>
        <rdfs:label>Bearing diagnosis based on Mahalanobis–Taguchi–Gram–Schmidt method</rdfs:label>
    </owl:NamedIndividual>
    


    <!-- http://www.semanticweb.org/suhaspai/ontologies/2021/4/UnivFAQ#ERONTO:_a_tool_for_extracting_ontologies_from_extended_E/R_diagrams -->

    <owl:NamedIndividual rdf:about="http://www.semanticweb.org/suhaspai/ontologies/2021/4/UnivFAQ#ERONTO:_a_tool_for_extracting_ontologies_from_extended_E/R_diagrams">
        <rdf:type rdf:resource="http://www.semanticweb.org/suhaspai/ontologies/2021/4/UnivFAQ#Publication"/>
        <UnivFAQ:inResearchField rdf:resource="http://www.semanticweb.org/suhaspai/ontologies/2021/4/UnivFAQ#Ontologies_and_Application"/>
        <UnivFAQ:publishedBy rdf:resource="http://www.semanticweb.org/suhaspai/ontologies/2021/4/UnivFAQ#Sreenivasa_Kumar"/>
        <rdfs:label>ERONTO: a tool for extracting ontologies from extended E/R diagrams</rdfs:label>
    </owl:NamedIndividual>
    


    <!-- http://www.semanticweb.org/suhaspai/ontologies/2021/4/UnivFAQ#Non-cooperative_spectrum_access—The_dedicated_vs._free_spectrum_choice -->

    <owl:NamedIndividual rdf:about="http://www.semanticweb.org/suhaspai/ontologies/2021/4/UnivFAQ#Non-cooperative_spectrum_access—The_dedicated_vs._free_spectrum_choice">
        <rdf:type rdf:resource="http://www.semanticweb.org/suhaspai/ontologies/2021/4/UnivFAQ#Publication"/>
        <UnivFAQ:inResearchField rdf:resource="http://www.semanticweb.org/suhaspai/ontologies/2021/4/UnivFAQ#Network_Control"/>
        <UnivFAQ:publishedBy rdf:resource="http://www.semanticweb.org/suhaspai/ontologies/2021/4/UnivFAQ#Krishna_Jagannathan"/>
        <rdfs:label>Non-cooperative spectrum access—The dedicated vs. free spectrum choice</rdfs:label>
    </owl:NamedIndividual>
    


    <!-- http://www.semanticweb.org/suhaspai/ontologies/2021/4/UnivFAQ#Underground_coal_gasification:_A_new_clean_coal_utilization_technique_for_India -->

    <owl:NamedIndividual rdf:about="http://www.semanticweb.org/suhaspai/ontologies/2021/4/UnivFAQ#Underground_coal_gasification:_A_new_clean_coal_utilization_technique_for_India">
        <rdf:type rdf:resource="http://www.semanticweb.org/suhaspai/ontologies/2021/4/UnivFAQ#Publication"/>
        <UnivFAQ:inResearchField rdf:resource="http://www.semanticweb.org/suhaspai/ontologies/2021/4/UnivFAQ#Underground_Coal_Gasification"/>
        <UnivFAQ:publishedBy rdf:resource="http://www.semanticweb.org/suhaspai/ontologies/2021/4/UnivFAQ#Preeti_Aghalayam"/>
        <rdfs:label>Underground coal gasification: A new clean coal utilization technique for India</rdfs:label>
    </owl:NamedIndividual>
    


    <!-- 
    ///////////////////////////////////////////////////////////////////////////////////////
    //
    // Annotations
    //
    ///////////////////////////////////////////////////////////////////////////////////////
     -->

    <rdf:Description rdf:about="http://www.semanticweb.org/suhaspai/ontologies/2021/4/UnivFAQ#CS3205">
        <rdfs:comment>Concepts and implementation of computer networks; architecture, protocol layers, inter-networking and addressing; network application development.</rdfs:comment>
        <rdfs:label>Introduction to Computer Networks</rdfs:label>
    </rdf:Description>
</rdf:RDF>



<!-- Generated by the OWL API (version 4.5.9.2019-02-01T07:24:44Z) https://github.com/owlcs/owlapi -->

