<?xml version="1.0"?>
<rdf:RDF xmlns="http://www.semanticweb.org/suhaspai/ontologies/2021/4/untitled-ontology-14"
     xml:base="http://www.semanticweb.org/suhaspai/ontologies/2021/4/untitled-ontology-14"
     xmlns:owl="http://www.w3.org/2002/07/owl#"
     xmlns:rdf="http://www.w3.org/1999/02/22-rdf-syntax-ns#"
     xmlns:xml="http://www.w3.org/XML/1998/namespace"
     xmlns:xsd="http://www.w3.org/2001/XMLSchema#"
     xmlns:rdfs="http://www.w3.org/2000/01/rdf-schema#"
     xmlns:UnivFAQ="http://www.semanticweb.org/suhaspai/ontologies/2021/4/UnivFAQ#">
    <owl:Ontology rdf:about="http://www.semanticweb.org/suhaspai/ontologies/2021/4/UnivFAQ"/>
    


    <!-- 
    ///////////////////////////////////////////////////////////////////////////////////////
    //
    // Object Properties
    //
    ///////////////////////////////////////////////////////////////////////////////////////
     -->

    


    <!-- http://www.semanticweb.org/suhaspai/ontologies/2021/4/UnivFAQ#belongsTo -->

    <owl:ObjectProperty rdf:about="http://www.semanticweb.org/suhaspai/ontologies/2021/4/UnivFAQ#belongsTo">
        <rdfs:domain rdf:resource="http://www.semanticweb.org/suhaspai/ontologies/2021/4/UnivFAQ#Professors"/>
        <rdfs:range rdf:resource="http://www.semanticweb.org/suhaspai/ontologies/2021/4/UnivFAQ#Department"/>
    </owl:ObjectProperty>
    


    <!-- http://www.semanticweb.org/suhaspai/ontologies/2021/4/UnivFAQ#hasAdmissionRequisites -->

    <owl:ObjectProperty rdf:about="http://www.semanticweb.org/suhaspai/ontologies/2021/4/UnivFAQ#hasAdmissionRequisites">
        <rdfs:domain rdf:resource="http://www.semanticweb.org/suhaspai/ontologies/2021/4/UnivFAQ#Programs"/>
        <rdfs:range rdf:resource="http://www.semanticweb.org/suhaspai/ontologies/2021/4/UnivFAQ#StandardizedTests"/>
    </owl:ObjectProperty>
    


    <!-- http://www.semanticweb.org/suhaspai/ontologies/2021/4/UnivFAQ#hasFacility -->

    <owl:ObjectProperty rdf:about="http://www.semanticweb.org/suhaspai/ontologies/2021/4/UnivFAQ#hasFacility">
        <rdfs:domain rdf:resource="http://www.semanticweb.org/suhaspai/ontologies/2021/4/UnivFAQ#Department"/>
        <rdfs:range rdf:resource="http://www.semanticweb.org/suhaspai/ontologies/2021/4/UnivFAQ#InstituteFacilities"/>
    </owl:ObjectProperty>
    


    <!-- http://www.semanticweb.org/suhaspai/ontologies/2021/4/UnivFAQ#hasMinimumCriterion -->

    <owl:ObjectProperty rdf:about="http://www.semanticweb.org/suhaspai/ontologies/2021/4/UnivFAQ#hasMinimumCriterion">
        <rdfs:domain rdf:resource="http://www.semanticweb.org/suhaspai/ontologies/2021/4/UnivFAQ#Programs"/>
        <rdfs:range rdf:resource="http://www.semanticweb.org/suhaspai/ontologies/2021/4/UnivFAQ#Qualifications"/>
    </owl:ObjectProperty>
    


    <!-- http://www.semanticweb.org/suhaspai/ontologies/2021/4/UnivFAQ#hasPrerequisite -->

    <owl:ObjectProperty rdf:about="http://www.semanticweb.org/suhaspai/ontologies/2021/4/UnivFAQ#hasPrerequisite">
        <owl:inverseOf rdf:resource="http://www.semanticweb.org/suhaspai/ontologies/2021/4/UnivFAQ#isPrerequisiteFor"/>
        <rdf:type rdf:resource="http://www.w3.org/2002/07/owl#TransitiveProperty"/>
    </owl:ObjectProperty>
    


    <!-- http://www.semanticweb.org/suhaspai/ontologies/2021/4/UnivFAQ#hasPublished -->

    <owl:ObjectProperty rdf:about="http://www.semanticweb.org/suhaspai/ontologies/2021/4/UnivFAQ#hasPublished">
        <rdfs:domain rdf:resource="http://www.semanticweb.org/suhaspai/ontologies/2021/4/UnivFAQ#Professors"/>
        <rdfs:range rdf:resource="http://www.semanticweb.org/suhaspai/ontologies/2021/4/UnivFAQ#Publication"/>
    </owl:ObjectProperty>
    


    <!-- http://www.semanticweb.org/suhaspai/ontologies/2021/4/UnivFAQ#hasScholarship -->

    <owl:ObjectProperty rdf:about="http://www.semanticweb.org/suhaspai/ontologies/2021/4/UnivFAQ#hasScholarship">
        <rdfs:domain rdf:resource="http://www.semanticweb.org/suhaspai/ontologies/2021/4/UnivFAQ#Programs"/>
        <rdfs:range rdf:resource="http://www.semanticweb.org/suhaspai/ontologies/2021/4/UnivFAQ#FinancialScholarship"/>
    </owl:ObjectProperty>
    


    <!-- http://www.semanticweb.org/suhaspai/ontologies/2021/4/UnivFAQ#headsDepartment -->

    <owl:ObjectProperty rdf:about="http://www.semanticweb.org/suhaspai/ontologies/2021/4/UnivFAQ#headsDepartment">
        <rdfs:domain rdf:resource="http://www.semanticweb.org/suhaspai/ontologies/2021/4/UnivFAQ#Professors"/>
        <rdfs:range rdf:resource="http://www.semanticweb.org/suhaspai/ontologies/2021/4/UnivFAQ#Department"/>
    </owl:ObjectProperty>
    


    <!-- http://www.semanticweb.org/suhaspai/ontologies/2021/4/UnivFAQ#isPrerequisiteFor -->

    <owl:ObjectProperty rdf:about="http://www.semanticweb.org/suhaspai/ontologies/2021/4/UnivFAQ#isPrerequisiteFor">
        <rdf:type rdf:resource="http://www.w3.org/2002/07/owl#TransitiveProperty"/>
        <rdfs:domain rdf:resource="http://www.semanticweb.org/suhaspai/ontologies/2021/4/UnivFAQ#Courses"/>
        <rdfs:range rdf:resource="http://www.semanticweb.org/suhaspai/ontologies/2021/4/UnivFAQ#Courses"/>
    </owl:ObjectProperty>
    


    <!-- http://www.semanticweb.org/suhaspai/ontologies/2021/4/UnivFAQ#isSpecializedIn -->

    <owl:ObjectProperty rdf:about="http://www.semanticweb.org/suhaspai/ontologies/2021/4/UnivFAQ#isSpecializedIn">
        <rdfs:domain rdf:resource="http://www.semanticweb.org/suhaspai/ontologies/2021/4/UnivFAQ#Professors"/>
        <rdfs:range rdf:resource="http://www.semanticweb.org/suhaspai/ontologies/2021/4/UnivFAQ#ResearchFields"/>
    </owl:ObjectProperty>
    


    <!-- http://www.semanticweb.org/suhaspai/ontologies/2021/4/UnivFAQ#offeredBy -->

    <owl:ObjectProperty rdf:about="http://www.semanticweb.org/suhaspai/ontologies/2021/4/UnivFAQ#offeredBy">
        <owl:inverseOf rdf:resource="http://www.semanticweb.org/suhaspai/ontologies/2021/4/UnivFAQ#offers"/>
    </owl:ObjectProperty>
    


    <!-- http://www.semanticweb.org/suhaspai/ontologies/2021/4/UnivFAQ#offers -->

    <owl:ObjectProperty rdf:about="http://www.semanticweb.org/suhaspai/ontologies/2021/4/UnivFAQ#offers">
        <rdfs:domain rdf:resource="http://www.semanticweb.org/suhaspai/ontologies/2021/4/UnivFAQ#Department"/>
        <rdfs:range>
            <owl:Class>
                <owl:unionOf rdf:parseType="Collection">
                    <rdf:Description rdf:about="http://www.semanticweb.org/suhaspai/ontologies/2021/4/UnivFAQ#Courses"/>
                    <rdf:Description rdf:about="http://www.semanticweb.org/suhaspai/ontologies/2021/4/UnivFAQ#Programs"/>
                </owl:unionOf>
            </owl:Class>
        </rdfs:range>
    </owl:ObjectProperty>
    


    <!-- http://www.semanticweb.org/suhaspai/ontologies/2021/4/UnivFAQ#requiredForMajor -->

    <owl:ObjectProperty rdf:about="http://www.semanticweb.org/suhaspai/ontologies/2021/4/UnivFAQ#requiredForMajor">
        <rdfs:domain rdf:resource="http://www.semanticweb.org/suhaspai/ontologies/2021/4/UnivFAQ#Programs"/>
        <rdfs:range rdf:resource="http://www.semanticweb.org/suhaspai/ontologies/2021/4/UnivFAQ#Courses"/>
    </owl:ObjectProperty>
    


    <!-- http://www.semanticweb.org/suhaspai/ontologies/2021/4/UnivFAQ#requiredForMinor -->

    <owl:ObjectProperty rdf:about="http://www.semanticweb.org/suhaspai/ontologies/2021/4/UnivFAQ#requiredForMinor"/>
    


    <!-- http://www.semanticweb.org/suhaspai/ontologies/2021/4/UnivFAQ#taughtBy -->

    <owl:ObjectProperty rdf:about="http://www.semanticweb.org/suhaspai/ontologies/2021/4/UnivFAQ#taughtBy">
        <owl:inverseOf rdf:resource="http://www.semanticweb.org/suhaspai/ontologies/2021/4/UnivFAQ#teaches"/>
    </owl:ObjectProperty>
    


    <!-- http://www.semanticweb.org/suhaspai/ontologies/2021/4/UnivFAQ#teaches -->

    <owl:ObjectProperty rdf:about="http://www.semanticweb.org/suhaspai/ontologies/2021/4/UnivFAQ#teaches">
        <rdfs:domain rdf:resource="http://www.semanticweb.org/suhaspai/ontologies/2021/4/UnivFAQ#Professors"/>
        <rdfs:range rdf:resource="http://www.semanticweb.org/suhaspai/ontologies/2021/4/UnivFAQ#Courses"/>
    </owl:ObjectProperty>
    


    <!-- 
    ///////////////////////////////////////////////////////////////////////////////////////
    //
    // Data properties
    //
    ///////////////////////////////////////////////////////////////////////////////////////
     -->

    


    <!-- http://www.semanticweb.org/suhaspai/ontologies/2021/4/UnivFAQ#name -->

    <owl:DatatypeProperty rdf:about="http://www.semanticweb.org/suhaspai/ontologies/2021/4/UnivFAQ#name">
        <rdf:type rdf:resource="http://www.w3.org/2002/07/owl#FunctionalProperty"/>
        <rdfs:domain rdf:resource="http://www.semanticweb.org/suhaspai/ontologies/2021/4/UnivFAQ#Courses"/>
        <rdfs:domain rdf:resource="http://www.semanticweb.org/suhaspai/ontologies/2021/4/UnivFAQ#Department"/>
        <rdfs:domain rdf:resource="http://www.semanticweb.org/suhaspai/ontologies/2021/4/UnivFAQ#Professors"/>
        <rdfs:range rdf:resource="http://www.w3.org/2001/XMLSchema#string"/>
    </owl:DatatypeProperty>
    


    <!-- http://www.semanticweb.org/suhaspai/ontologies/2021/4/UnivFAQ#testProp -->

    <owl:DatatypeProperty rdf:about="http://www.semanticweb.org/suhaspai/ontologies/2021/4/UnivFAQ#testProp">
        <rdf:type rdf:resource="http://www.w3.org/2002/07/owl#FunctionalProperty"/>
        <rdfs:domain rdf:resource="http://www.semanticweb.org/suhaspai/ontologies/2021/4/UnivFAQ#Courses"/>
        <rdfs:domain rdf:resource="http://www.semanticweb.org/suhaspai/ontologies/2021/4/UnivFAQ#Professors"/>
        <rdfs:range rdf:resource="http://www.w3.org/2001/XMLSchema#string"/>
    </owl:DatatypeProperty>
    


    <!-- 
    ///////////////////////////////////////////////////////////////////////////////////////
    //
    // Classes
    //
    ///////////////////////////////////////////////////////////////////////////////////////
     -->

    


    <!-- http://www.semanticweb.org/suhaspai/ontologies/2021/4/UnivFAQ#AdminStaff -->

    <owl:Class rdf:about="http://www.semanticweb.org/suhaspai/ontologies/2021/4/UnivFAQ#AdminStaff">
        <rdfs:subClassOf rdf:resource="http://www.semanticweb.org/suhaspai/ontologies/2021/4/UnivFAQ#Person"/>
    </owl:Class>
    


    <!-- http://www.semanticweb.org/suhaspai/ontologies/2021/4/UnivFAQ#Alumni -->

    <owl:Class rdf:about="http://www.semanticweb.org/suhaspai/ontologies/2021/4/UnivFAQ#Alumni">
        <rdfs:subClassOf rdf:resource="http://www.semanticweb.org/suhaspai/ontologies/2021/4/UnivFAQ#Person"/>
    </owl:Class>
    


    <!-- http://www.semanticweb.org/suhaspai/ontologies/2021/4/UnivFAQ#AssistantProfessor -->

    <owl:Class rdf:about="http://www.semanticweb.org/suhaspai/ontologies/2021/4/UnivFAQ#AssistantProfessor">
        <rdfs:subClassOf rdf:resource="http://www.semanticweb.org/suhaspai/ontologies/2021/4/UnivFAQ#Professors"/>
    </owl:Class>
    


    <!-- http://www.semanticweb.org/suhaspai/ontologies/2021/4/UnivFAQ#AssociateProfessor -->

    <owl:Class rdf:about="http://www.semanticweb.org/suhaspai/ontologies/2021/4/UnivFAQ#AssociateProfessor">
        <rdfs:subClassOf rdf:resource="http://www.semanticweb.org/suhaspai/ontologies/2021/4/UnivFAQ#Professors"/>
    </owl:Class>
    


    <!-- http://www.semanticweb.org/suhaspai/ontologies/2021/4/UnivFAQ#BTech. -->

    <owl:Class rdf:about="http://www.semanticweb.org/suhaspai/ontologies/2021/4/UnivFAQ#BTech.">
        <rdfs:subClassOf rdf:resource="http://www.semanticweb.org/suhaspai/ontologies/2021/4/UnivFAQ#UndergradPrograms"/>
    </owl:Class>
    


    <!-- http://www.semanticweb.org/suhaspai/ontologies/2021/4/UnivFAQ#Courses -->

    <owl:Class rdf:about="http://www.semanticweb.org/suhaspai/ontologies/2021/4/UnivFAQ#Courses"/>
    


    <!-- http://www.semanticweb.org/suhaspai/ontologies/2021/4/UnivFAQ#Department -->

    <owl:Class rdf:about="http://www.semanticweb.org/suhaspai/ontologies/2021/4/UnivFAQ#Department"/>
    


    <!-- http://www.semanticweb.org/suhaspai/ontologies/2021/4/UnivFAQ#Dual_Degree -->

    <owl:Class rdf:about="http://www.semanticweb.org/suhaspai/ontologies/2021/4/UnivFAQ#Dual_Degree">
        <rdfs:subClassOf rdf:resource="http://www.semanticweb.org/suhaspai/ontologies/2021/4/UnivFAQ#UndergradPrograms"/>
    </owl:Class>
    


    <!-- http://www.semanticweb.org/suhaspai/ontologies/2021/4/UnivFAQ#FinancialScholarship -->

    <owl:Class rdf:about="http://www.semanticweb.org/suhaspai/ontologies/2021/4/UnivFAQ#FinancialScholarship"/>
    


    <!-- http://www.semanticweb.org/suhaspai/ontologies/2021/4/UnivFAQ#InstituteFacilities -->

    <owl:Class rdf:about="http://www.semanticweb.org/suhaspai/ontologies/2021/4/UnivFAQ#InstituteFacilities"/>
    


    <!-- http://www.semanticweb.org/suhaspai/ontologies/2021/4/UnivFAQ#MS -->

    <owl:Class rdf:about="http://www.semanticweb.org/suhaspai/ontologies/2021/4/UnivFAQ#MS">
        <rdfs:subClassOf rdf:resource="http://www.semanticweb.org/suhaspai/ontologies/2021/4/UnivFAQ#PostgradPrograms"/>
    </owl:Class>
    


    <!-- http://www.semanticweb.org/suhaspai/ontologies/2021/4/UnivFAQ#MTech. -->

    <owl:Class rdf:about="http://www.semanticweb.org/suhaspai/ontologies/2021/4/UnivFAQ#MTech.">
        <rdfs:subClassOf rdf:resource="http://www.semanticweb.org/suhaspai/ontologies/2021/4/UnivFAQ#PostgradPrograms"/>
    </owl:Class>
    


    <!-- http://www.semanticweb.org/suhaspai/ontologies/2021/4/UnivFAQ#Person -->

    <owl:Class rdf:about="http://www.semanticweb.org/suhaspai/ontologies/2021/4/UnivFAQ#Person"/>
    


    <!-- http://www.semanticweb.org/suhaspai/ontologies/2021/4/UnivFAQ#PhD -->

    <owl:Class rdf:about="http://www.semanticweb.org/suhaspai/ontologies/2021/4/UnivFAQ#PhD">
        <rdfs:subClassOf rdf:resource="http://www.semanticweb.org/suhaspai/ontologies/2021/4/UnivFAQ#PostgradPrograms"/>
    </owl:Class>
    


    <!-- http://www.semanticweb.org/suhaspai/ontologies/2021/4/UnivFAQ#PostgradCourses -->

    <owl:Class rdf:about="http://www.semanticweb.org/suhaspai/ontologies/2021/4/UnivFAQ#PostgradCourses">
        <rdfs:subClassOf rdf:resource="http://www.semanticweb.org/suhaspai/ontologies/2021/4/UnivFAQ#Courses"/>
    </owl:Class>
    


    <!-- http://www.semanticweb.org/suhaspai/ontologies/2021/4/UnivFAQ#PostgradPrograms -->

    <owl:Class rdf:about="http://www.semanticweb.org/suhaspai/ontologies/2021/4/UnivFAQ#PostgradPrograms">
        <rdfs:subClassOf rdf:resource="http://www.semanticweb.org/suhaspai/ontologies/2021/4/UnivFAQ#Programs"/>
    </owl:Class>
    


    <!-- http://www.semanticweb.org/suhaspai/ontologies/2021/4/UnivFAQ#Professor -->

    <owl:Class rdf:about="http://www.semanticweb.org/suhaspai/ontologies/2021/4/UnivFAQ#Professor">
        <rdfs:subClassOf rdf:resource="http://www.semanticweb.org/suhaspai/ontologies/2021/4/UnivFAQ#Professors"/>
    </owl:Class>
    


    <!-- http://www.semanticweb.org/suhaspai/ontologies/2021/4/UnivFAQ#Professors -->

    <owl:Class rdf:about="http://www.semanticweb.org/suhaspai/ontologies/2021/4/UnivFAQ#Professors">
        <rdfs:subClassOf rdf:resource="http://www.semanticweb.org/suhaspai/ontologies/2021/4/UnivFAQ#Person"/>
    </owl:Class>
    


    <!-- http://www.semanticweb.org/suhaspai/ontologies/2021/4/UnivFAQ#Programs -->

    <owl:Class rdf:about="http://www.semanticweb.org/suhaspai/ontologies/2021/4/UnivFAQ#Programs"/>
    


    <!-- http://www.semanticweb.org/suhaspai/ontologies/2021/4/UnivFAQ#Publication -->

    <owl:Class rdf:about="http://www.semanticweb.org/suhaspai/ontologies/2021/4/UnivFAQ#Publication"/>
    


    <!-- http://www.semanticweb.org/suhaspai/ontologies/2021/4/UnivFAQ#Qualifications -->

    <owl:Class rdf:about="http://www.semanticweb.org/suhaspai/ontologies/2021/4/UnivFAQ#Qualifications"/>
    


    <!-- http://www.semanticweb.org/suhaspai/ontologies/2021/4/UnivFAQ#ResearchFields -->

    <owl:Class rdf:about="http://www.semanticweb.org/suhaspai/ontologies/2021/4/UnivFAQ#ResearchFields"/>
    


    <!-- http://www.semanticweb.org/suhaspai/ontologies/2021/4/UnivFAQ#StandardizedTests -->

    <owl:Class rdf:about="http://www.semanticweb.org/suhaspai/ontologies/2021/4/UnivFAQ#StandardizedTests"/>
    


    <!-- http://www.semanticweb.org/suhaspai/ontologies/2021/4/UnivFAQ#Student -->

    <owl:Class rdf:about="http://www.semanticweb.org/suhaspai/ontologies/2021/4/UnivFAQ#Student">
        <rdfs:subClassOf rdf:resource="http://www.semanticweb.org/suhaspai/ontologies/2021/4/UnivFAQ#Person"/>
    </owl:Class>
    


    <!-- http://www.semanticweb.org/suhaspai/ontologies/2021/4/UnivFAQ#UndergradCourses -->

    <owl:Class rdf:about="http://www.semanticweb.org/suhaspai/ontologies/2021/4/UnivFAQ#UndergradCourses">
        <rdfs:subClassOf rdf:resource="http://www.semanticweb.org/suhaspai/ontologies/2021/4/UnivFAQ#Courses"/>
    </owl:Class>
    


    <!-- http://www.semanticweb.org/suhaspai/ontologies/2021/4/UnivFAQ#UndergradPrograms -->

    <owl:Class rdf:about="http://www.semanticweb.org/suhaspai/ontologies/2021/4/UnivFAQ#UndergradPrograms">
        <rdfs:subClassOf rdf:resource="http://www.semanticweb.org/suhaspai/ontologies/2021/4/UnivFAQ#Programs"/>
    </owl:Class>
    


    <!-- http://www.semanticweb.org/suhaspai/ontologies/2021/4/UnivFAQ#VistingProfessor -->

    <owl:Class rdf:about="http://www.semanticweb.org/suhaspai/ontologies/2021/4/UnivFAQ#VistingProfessor">
        <rdfs:subClassOf rdf:resource="http://www.semanticweb.org/suhaspai/ontologies/2021/4/UnivFAQ#Professors"/>
    </owl:Class>
    


    <!-- 
    ///////////////////////////////////////////////////////////////////////////////////////
    //
    // Individuals
    //
    ///////////////////////////////////////////////////////////////////////////////////////
     -->

    


    <!-- http://www.semanticweb.org/suhaspai/ontologies/2021/4/UnivFAQ#AIDB_Lab -->

    <owl:NamedIndividual rdf:about="http://www.semanticweb.org/suhaspai/ontologies/2021/4/UnivFAQ#AIDB_Lab">
        <rdf:type rdf:resource="http://www.semanticweb.org/suhaspai/ontologies/2021/4/UnivFAQ#InstituteFacilities"/>
        <rdfs:comment>Artificial Intelligence and Databases</rdfs:comment>
        <rdfs:label>AIDB Lab</rdfs:label>
    </owl:NamedIndividual>
    


    <!-- http://www.semanticweb.org/suhaspai/ontologies/2021/4/UnivFAQ#Abishek_Sinha -->

    <owl:NamedIndividual rdf:about="http://www.semanticweb.org/suhaspai/ontologies/2021/4/UnivFAQ#Abishek_Sinha">
        <rdf:type rdf:resource="http://www.semanticweb.org/suhaspai/ontologies/2021/4/UnivFAQ#AssistantProfessor"/>
        <UnivFAQ:isSpecializedIn rdf:resource="http://www.semanticweb.org/suhaspai/ontologies/2021/4/UnivFAQ#Information_Theory"/>
        <UnivFAQ:isSpecializedIn rdf:resource="http://www.semanticweb.org/suhaspai/ontologies/2021/4/UnivFAQ#Network_Control"/>
        <UnivFAQ:teaches rdf:resource="http://www.semanticweb.org/suhaspai/ontologies/2021/4/UnivFAQ#EE6112"/>
        <UnivFAQ:name>Abishek Sinha</UnivFAQ:name>
        <rdfs:label>Abishek Sinha</rdfs:label>
    </owl:NamedIndividual>
    


    <!-- http://www.semanticweb.org/suhaspai/ontologies/2021/4/UnivFAQ#Analog -->

    <owl:NamedIndividual rdf:about="http://www.semanticweb.org/suhaspai/ontologies/2021/4/UnivFAQ#Analog">
        <rdf:type rdf:resource="http://www.semanticweb.org/suhaspai/ontologies/2021/4/UnivFAQ#ResearchFields"/>
        <rdfs:label>Analog</rdfs:label>
    </owl:NamedIndividual>
    


    <!-- http://www.semanticweb.org/suhaspai/ontologies/2021/4/UnivFAQ#Artificial_Intelligence -->

    <owl:NamedIndividual rdf:about="http://www.semanticweb.org/suhaspai/ontologies/2021/4/UnivFAQ#Artificial_Intelligence">
        <rdf:type rdf:resource="http://www.semanticweb.org/suhaspai/ontologies/2021/4/UnivFAQ#ResearchFields"/>
        <rdfs:comment>Artificial intelligence is intelligence demonstrated by machines, as opposed to natural intelligence displayed by animals including humans.</rdfs:comment>
        <rdfs:label>Artificial Intelligence</rdfs:label>
    </owl:NamedIndividual>
    


    <!-- http://www.semanticweb.org/suhaspai/ontologies/2021/4/UnivFAQ#Arun_Rajkumar -->

    <owl:NamedIndividual rdf:about="http://www.semanticweb.org/suhaspai/ontologies/2021/4/UnivFAQ#Arun_Rajkumar">
        <rdf:type rdf:resource="http://www.semanticweb.org/suhaspai/ontologies/2021/4/UnivFAQ#AssistantProfessor"/>
        <UnivFAQ:isSpecializedIn rdf:resource="http://www.semanticweb.org/suhaspai/ontologies/2021/4/UnivFAQ#Machine_Learning"/>
        <UnivFAQ:teaches rdf:resource="http://www.semanticweb.org/suhaspai/ontologies/2021/4/UnivFAQ#CS1100"/>
        <UnivFAQ:name>Arun Rajkumar</UnivFAQ:name>
        <rdfs:label>Arun Rajkumar</rdfs:label>
    </owl:NamedIndividual>
    


    <!-- http://www.semanticweb.org/suhaspai/ontologies/2021/4/UnivFAQ#BTech._Computer_Science -->

    <owl:NamedIndividual rdf:about="http://www.semanticweb.org/suhaspai/ontologies/2021/4/UnivFAQ#BTech._Computer_Science">
        <rdf:type rdf:resource="http://www.semanticweb.org/suhaspai/ontologies/2021/4/UnivFAQ#BTech."/>
        <rdfs:comment>The B.Tech. program is a four-year course oriented undergraduate program. The course work is spread accross all the semesters. The courses include a set of core courses offered by the department, a set of departmental electives and some free electives. In total, the academic activities include 7 department electives and 8 free electives. A B.Tech project is optional and the student can take 2 additional department electives in lieu of the B.Tech project.</rdfs:comment>
        <rdfs:label>BTech. Computer Science</rdfs:label>
    </owl:NamedIndividual>
    


    <!-- http://www.semanticweb.org/suhaspai/ontologies/2021/4/UnivFAQ#B_Ravindran -->

    <owl:NamedIndividual rdf:about="http://www.semanticweb.org/suhaspai/ontologies/2021/4/UnivFAQ#B_Ravindran">
        <rdf:type rdf:resource="http://www.semanticweb.org/suhaspai/ontologies/2021/4/UnivFAQ#Professor"/>
        <UnivFAQ:isSpecializedIn rdf:resource="http://www.semanticweb.org/suhaspai/ontologies/2021/4/UnivFAQ#Reinforcement_Learning"/>
        <UnivFAQ:teaches rdf:resource="http://www.semanticweb.org/suhaspai/ontologies/2021/4/UnivFAQ#CS6700"/>
        <UnivFAQ:name rdf:datatype="http://www.w3.org/2001/XMLSchema#string">Balaram Ravindran</UnivFAQ:name>
        <rdfs:label rdf:datatype="http://www.w3.org/2001/XMLSchema#string">Balaram Ravindran</rdfs:label>
    </owl:NamedIndividual>
    


    <!-- http://www.semanticweb.org/suhaspai/ontologies/2021/4/UnivFAQ#CS-DD -->

    <owl:NamedIndividual rdf:about="http://www.semanticweb.org/suhaspai/ontologies/2021/4/UnivFAQ#CS-DD">
        <rdf:type rdf:resource="http://www.semanticweb.org/suhaspai/ontologies/2021/4/UnivFAQ#Dual_Degree"/>
        <UnivFAQ:offeredBy rdf:resource="http://www.semanticweb.org/suhaspai/ontologies/2021/4/UnivFAQ#Computer_Science"/>
        <rdfs:comment>The Dual Degree program is a five year program. At the end of five years, the student is awarded both a B.Tech. and M.Tech. degree.</rdfs:comment>
        <rdfs:label>Dual Degree (BTech. + MTech.) Computer Science</rdfs:label>
    </owl:NamedIndividual>
    


    <!-- http://www.semanticweb.org/suhaspai/ontologies/2021/4/UnivFAQ#CS-MTech -->

    <owl:NamedIndividual rdf:about="http://www.semanticweb.org/suhaspai/ontologies/2021/4/UnivFAQ#CS-MTech">
        <rdf:type rdf:resource="http://www.semanticweb.org/suhaspai/ontologies/2021/4/UnivFAQ#MTech."/>
        <UnivFAQ:offeredBy rdf:resource="http://www.semanticweb.org/suhaspai/ontologies/2021/4/UnivFAQ#Computer_Science"/>
        <rdfs:comment>The M.Tech. program is a two-year course oriented graduate program. The student has to take a set of core courses and a set of electives. The course work is spread accross the first two semesters with an option of taking one elective in the third semester. This is followed by a project in the third and fourth semester in which the student can take up a project of his or her interest, supervised by a faculty member.</rdfs:comment>
        <rdfs:label>MTech. Computer Science</rdfs:label>
    </owl:NamedIndividual>
    


    <!-- http://www.semanticweb.org/suhaspai/ontologies/2021/4/UnivFAQ#CS-PhD -->

    <owl:NamedIndividual rdf:about="http://www.semanticweb.org/suhaspai/ontologies/2021/4/UnivFAQ#CS-PhD">
        <rdf:type rdf:resource="http://www.semanticweb.org/suhaspai/ontologies/2021/4/UnivFAQ#PhD"/>
        <UnivFAQ:offeredBy rdf:resource="http://www.semanticweb.org/suhaspai/ontologies/2021/4/UnivFAQ#Computer_Science"/>
        <rdfs:comment>PhD. programs are postgraduate research oriented programs. The scholar works in an area of his/her interest under the supervision of a faculty member. The scholar has to obtain a minimum number of credits by taking courses. The highlight of the program is the independent research work taken by scholar, leading to a dissertation at the end of the program. The average duration of a PhD. program is between four to five years.</rdfs:comment>
        <rdfs:label>PHD. Computer Science</rdfs:label>
    </owl:NamedIndividual>
    


    <!-- http://www.semanticweb.org/suhaspai/ontologies/2021/4/UnivFAQ#CS1100 -->

    <owl:NamedIndividual rdf:about="http://www.semanticweb.org/suhaspai/ontologies/2021/4/UnivFAQ#CS1100">
        <rdf:type rdf:resource="http://www.semanticweb.org/suhaspai/ontologies/2021/4/UnivFAQ#UndergradCourses"/>
        <UnivFAQ:isPrerequisiteFor rdf:resource="http://www.semanticweb.org/suhaspai/ontologies/2021/4/UnivFAQ#CS1200"/>
        <UnivFAQ:isPrerequisiteFor rdf:resource="http://www.semanticweb.org/suhaspai/ontologies/2021/4/UnivFAQ#CS2800"/>
        <UnivFAQ:isPrerequisiteFor rdf:resource="http://www.semanticweb.org/suhaspai/ontologies/2021/4/UnivFAQ#CS3700"/>
        <UnivFAQ:isPrerequisiteFor rdf:resource="http://www.semanticweb.org/suhaspai/ontologies/2021/4/UnivFAQ#CS6023"/>
        <UnivFAQ:isPrerequisiteFor rdf:resource="http://www.semanticweb.org/suhaspai/ontologies/2021/4/UnivFAQ#CS6910"/>
        <rdfs:comment>The introductory computer science course - teaches basic programming to fresher students</rdfs:comment>
        <rdfs:label>Introduction to Programming</rdfs:label>
    </owl:NamedIndividual>
    


    <!-- http://www.semanticweb.org/suhaspai/ontologies/2021/4/UnivFAQ#CS1200 -->

    <owl:NamedIndividual rdf:about="http://www.semanticweb.org/suhaspai/ontologies/2021/4/UnivFAQ#CS1200">
        <rdf:type rdf:resource="http://www.semanticweb.org/suhaspai/ontologies/2021/4/UnivFAQ#UndergradCourses"/>
        <rdfs:comment>The course is about sets which are discrete in nature. It starts from ways of describing them, then size estimates of sets (combinatorics), and then culminates in studying structured sets. After completing the course, the student will be able to: (1) Use logical notation to define and reason mathematically about the fundamental data types and structures (such as numbers, sets) used in computer algorithms and systems. (2) Comprehend and Evaluate rigour in the definitions and conclusions about mathematical models and identify fallacious reasoning and statements. (3) Identify and Apply properties of combinatorial structures and properties - know the basic techniques in combinatorics and counting. (4) Analyze sets with operations, and identify their structure. (5) Reason and Conclude properties about the structure based on the observations. (6) Gain the conceptual background needed to be able to identify structures of algebraic nature, and discover, prove and use properties about them.</rdfs:comment>
        <rdfs:label>Discrete Mathematics</rdfs:label>
    </owl:NamedIndividual>
    


    <!-- http://www.semanticweb.org/suhaspai/ontologies/2021/4/UnivFAQ#CS2800 -->

    <owl:NamedIndividual rdf:about="http://www.semanticweb.org/suhaspai/ontologies/2021/4/UnivFAQ#CS2800">
        <rdf:type rdf:resource="http://www.semanticweb.org/suhaspai/ontologies/2021/4/UnivFAQ#Courses"/>
        <UnivFAQ:offeredBy rdf:resource="http://www.semanticweb.org/suhaspai/ontologies/2021/4/UnivFAQ#Computer_Science"/>
        <rdfs:comment>The objective of the course is to teach techniques for effective problem solving incomputing. The use of different paradigms of problem solving will be used to illustrate cleverand efficient ways to solve a given problem. In each case emphasis will be placed onrigorously proving correctness of the algorithm. In addition, the analysis of the algorithm will beused to show the efficiency of the algorithm over the naive techniques.</rdfs:comment>
        <rdfs:label>Design and Analysis of Algorithms</rdfs:label>
    </owl:NamedIndividual>
    


    <!-- http://www.semanticweb.org/suhaspai/ontologies/2021/4/UnivFAQ#CS3700 -->

    <owl:NamedIndividual rdf:about="http://www.semanticweb.org/suhaspai/ontologies/2021/4/UnivFAQ#CS3700">
        <rdf:type rdf:resource="http://www.semanticweb.org/suhaspai/ontologies/2021/4/UnivFAQ#Courses"/>
        <UnivFAQ:isPrerequisiteFor rdf:resource="http://www.semanticweb.org/suhaspai/ontologies/2021/4/UnivFAQ#CS6852"/>
        <rdfs:comment>General introduction to database systems; Database - DBMS disctinction, approaches to building a database, data models, database management system, three-schema architecture of a database, challenges in building a DBMS, various components of a DBMS. E/R Model - Conceptual data modeling - motivation, entities, entity types, various types of attributes, relationships, relationship types, E/R diagram notation, examples. Relational Data Model - Concept of relations, schema-instance distinction, keys, referential integrity and foreign keys, relational algebra operators: selection, projection, cross product, various types of joins, division, example queries, tuple relation calculus, domain relational calculus, converting the database specification in E/R notation to the relational schema. SQL - Introduction, data definition in SQL, table, key and foreign key definitions, update behaviors. Querying in SQL - basic select-from-where block and its semantics, nested queries - correlated and uncorrelated, notion of aggregation, aggregation functions group by and having clauses, embedded SQL. Dependencies and Normal forms - Importance of a good schema design, problems encountered with bad schema designs, motivation for normal forms, dependency theory - functional dependencies, Armstrong&apos;s axioms for FD&apos;s, closure of a set of FD&apos;s, minimal covers, definitions of 1NF, 2NF, 3NF and BCNF, decompositions and desirable properties of them, algorithms for 3NF and BCNF normalization, multi-valued dependencies and 4NF, join dependencies and definition of 5NF. Data Storage and Indexes - file organizations, primary, secondary index structures, various index structures - hash-based, dynamic hashing techniques, multi-level indexes, B+ trees. Transaction processing and Error recovery - concepts of transaction processing, ACID properties, concurrency control, locking based protocols for CC, error recovery and logging, undo, redo, undo-redo logging and recovery methods.</rdfs:comment>
        <rdfs:label>Introduction to Database Systems</rdfs:label>
    </owl:NamedIndividual>
    


    <!-- http://www.semanticweb.org/suhaspai/ontologies/2021/4/UnivFAQ#CS6023 -->

    <owl:NamedIndividual rdf:about="http://www.semanticweb.org/suhaspai/ontologies/2021/4/UnivFAQ#CS6023">
        <rdf:type rdf:resource="http://www.semanticweb.org/suhaspai/ontologies/2021/4/UnivFAQ#Courses"/>
        <UnivFAQ:offeredBy rdf:resource="http://www.semanticweb.org/suhaspai/ontologies/2021/4/UnivFAQ#Computer_Science"/>
        <rdfs:comment>To learn parallel programming with graphics processing units (GPUs) Outcomes: Students would learn concepts in parallel programming, implementation of programs on GPUs, debugging and profiling parallel programs.</rdfs:comment>
        <rdfs:label>GPU Programming</rdfs:label>
    </owl:NamedIndividual>
    


    <!-- http://www.semanticweb.org/suhaspai/ontologies/2021/4/UnivFAQ#CS6700 -->

    <owl:NamedIndividual rdf:about="http://www.semanticweb.org/suhaspai/ontologies/2021/4/UnivFAQ#CS6700">
        <rdf:type rdf:resource="http://www.semanticweb.org/suhaspai/ontologies/2021/4/UnivFAQ#Courses"/>
        <UnivFAQ:offeredBy rdf:resource="http://www.semanticweb.org/suhaspai/ontologies/2021/4/UnivFAQ#Computer_Science"/>
        <rdfs:comment>The Reinforcement Learning problem : evaluative feedback, non-associative learning, Rewards and returns, Markov Decision Processes, Value functions, optimality and approximation. Dynamic programming : value iteration, policy iteration, asynchronous DP, generalized policy iteration. Monta-Carlo methods : policy evaluation, roll outs, on policy and off policy learning, importance sampling. Temporal Difference learning : TD prediction, Optimality of TD(0), SARSA, Q-learning, R-learning, Games and after states. Eligibility traces : n-step TD prediction, TD (lambda), forward and backward views, Q (lambda), SARSA (lambda), replacing traces and accumulating traces. Function Approximation : Value prediction, gradient descent methods, linear function approximation, ANN based function approximation, lazy learning, instability issues Policy Gradient methods : non-associative learning – REINFORCE algorithm, exact gradient methods, estimating gradients, approximate policy gradient algorithms, actor-critic methods. Planning and Learning : Model based learning and planning, prioritized sweeping, Dyna, heuristic search, trajectory sampling, E 3 algorithm Hierarchical RL : MAXQ framework, Options framework, HAM framework, airport algorithm, hierarchical policy gradient Case studies : Elevator dispatching, Samuel’s checker player, TDgammon, Acrobot, Helicopter piloting</rdfs:comment>
        <rdfs:label>Reinforcement Learning</rdfs:label>
    </owl:NamedIndividual>
    


    <!-- http://www.semanticweb.org/suhaspai/ontologies/2021/4/UnivFAQ#CS6852 -->

    <owl:NamedIndividual rdf:about="http://www.semanticweb.org/suhaspai/ontologies/2021/4/UnivFAQ#CS6852">
        <rdf:type rdf:resource="http://www.semanticweb.org/suhaspai/ontologies/2021/4/UnivFAQ#Courses"/>
        <UnivFAQ:offeredBy rdf:resource="http://www.semanticweb.org/suhaspai/ontologies/2021/4/UnivFAQ#Computer_Science"/>
        <rdfs:comment>To discuss topics in the emerging areas of Semantic Web Technology, Ontologies for Knowledge Representation and their Applications.</rdfs:comment>
        <rdfs:label>Theory and Applications of Ontologies</rdfs:label>
    </owl:NamedIndividual>
    


    <!-- http://www.semanticweb.org/suhaspai/ontologies/2021/4/UnivFAQ#CS6910 -->

    <owl:NamedIndividual rdf:about="http://www.semanticweb.org/suhaspai/ontologies/2021/4/UnivFAQ#CS6910">
        <rdf:type rdf:resource="http://www.semanticweb.org/suhaspai/ontologies/2021/4/UnivFAQ#Courses"/>
        <UnivFAQ:offeredBy rdf:resource="http://www.semanticweb.org/suhaspai/ontologies/2021/4/UnivFAQ#Computer_Science"/>
        <rdfs:comment>Neural Networks have made tremendous impact on various AI fields in the recent past. In this course, we study the basics of Neural Networks and their various variants such as the Convolutional Neural Networks and Recurrent Neural Networks. We also study the different ways in which they can be used to solve problems in various domains such as Computer Vision, Speech and NLP. We also look at the latest results and trends in the field.</rdfs:comment>
        <rdfs:label>Deep Learning</rdfs:label>
    </owl:NamedIndividual>
    


    <!-- http://www.semanticweb.org/suhaspai/ontologies/2021/4/UnivFAQ#Chandra_Sekhar -->

    <owl:NamedIndividual rdf:about="http://www.semanticweb.org/suhaspai/ontologies/2021/4/UnivFAQ#Chandra_Sekhar">
        <rdf:type rdf:resource="http://www.semanticweb.org/suhaspai/ontologies/2021/4/UnivFAQ#Professor"/>
        <UnivFAQ:headsDepartment rdf:resource="http://www.semanticweb.org/suhaspai/ontologies/2021/4/UnivFAQ#Computer_Science"/>
        <UnivFAQ:teaches rdf:resource="http://www.semanticweb.org/suhaspai/ontologies/2021/4/UnivFAQ#CS6910"/>
        <UnivFAQ:name rdf:datatype="http://www.w3.org/2001/XMLSchema#string">C Chandra Sekhar</UnivFAQ:name>
        <rdfs:label rdf:datatype="http://www.w3.org/2001/XMLSchema#string">C Chandra Sekhar</rdfs:label>
    </owl:NamedIndividual>
    


    <!-- http://www.semanticweb.org/suhaspai/ontologies/2021/4/UnivFAQ#Compilers -->

    <owl:NamedIndividual rdf:about="http://www.semanticweb.org/suhaspai/ontologies/2021/4/UnivFAQ#Compilers">
        <rdf:type rdf:resource="http://www.semanticweb.org/suhaspai/ontologies/2021/4/UnivFAQ#ResearchFields"/>
        <rdfs:comment>research into foundational software tools helping scientists to program for speed, interoperability, interactivity, flexibility, and reproducibility.</rdfs:comment>
        <rdfs:label>Compilers</rdfs:label>
    </owl:NamedIndividual>
    


    <!-- http://www.semanticweb.org/suhaspai/ontologies/2021/4/UnivFAQ#Computer_Science -->

    <owl:NamedIndividual rdf:about="http://www.semanticweb.org/suhaspai/ontologies/2021/4/UnivFAQ#Computer_Science">
        <rdf:type rdf:resource="http://www.semanticweb.org/suhaspai/ontologies/2021/4/UnivFAQ#Department"/>
        <UnivFAQ:hasFacility rdf:resource="http://www.semanticweb.org/suhaspai/ontologies/2021/4/UnivFAQ#AIDB_Lab"/>
        <UnivFAQ:hasFacility rdf:resource="http://www.semanticweb.org/suhaspai/ontologies/2021/4/UnivFAQ#DCF_Lab"/>
        <UnivFAQ:hasFacility rdf:resource="http://www.semanticweb.org/suhaspai/ontologies/2021/4/UnivFAQ#PACE_Lab"/>
        <UnivFAQ:offers rdf:resource="http://www.semanticweb.org/suhaspai/ontologies/2021/4/UnivFAQ#BTech._Computer_Science"/>
        <UnivFAQ:offers rdf:resource="http://www.semanticweb.org/suhaspai/ontologies/2021/4/UnivFAQ#CS1100"/>
        <UnivFAQ:offers rdf:resource="http://www.semanticweb.org/suhaspai/ontologies/2021/4/UnivFAQ#CS1200"/>
        <UnivFAQ:offers rdf:resource="http://www.semanticweb.org/suhaspai/ontologies/2021/4/UnivFAQ#CS3700"/>
        <rdfs:comment>Global excellence and local relevance in research, teaching, and technology development is the vision of the Department. The Department was started as the Computer Centre in 1973 with the acquisition of an IBM 370, perhaps the most powerful computer in India at that time. It offered M.Tech, M.S and PhD degree programmes. In 1983, the B.Tech degree programme was started.

Today the Department has a vibrant student body numbering about 700. Over 60% are postgraduate, mostly supported by scholarships. The Department also offers several attractive industry-sponsored Fellowships for outstanding PhD scholars and liberally supports participation in top-ranking international conferences.

The department has been funded by FIST program from DST, Govt. of India in 2002 and 2017. The Secure Systems Laboratory is funded by FIST program 2017.</rdfs:comment>
        <rdfs:label>Computer Science Department</rdfs:label>
    </owl:NamedIndividual>
    


    <!-- http://www.semanticweb.org/suhaspai/ontologies/2021/4/UnivFAQ#Cryptography -->

    <owl:NamedIndividual rdf:about="http://www.semanticweb.org/suhaspai/ontologies/2021/4/UnivFAQ#Cryptography">
        <rdf:type rdf:resource="http://www.semanticweb.org/suhaspai/ontologies/2021/4/UnivFAQ#ResearchFields"/>
        <rdfs:comment>Cryptography, or cryptology, is the practice and study of techniques for secure communication in the presence of adversarial behavior.</rdfs:comment>
        <rdfs:label>Cryptography</rdfs:label>
    </owl:NamedIndividual>
    


    <!-- http://www.semanticweb.org/suhaspai/ontologies/2021/4/UnivFAQ#DCF_Lab -->

    <owl:NamedIndividual rdf:about="http://www.semanticweb.org/suhaspai/ontologies/2021/4/UnivFAQ#DCF_Lab">
        <rdf:type rdf:resource="http://www.semanticweb.org/suhaspai/ontologies/2021/4/UnivFAQ#InstituteFacilities"/>
        <rdfs:comment>Departmental Computing Facility (DCF) is an exclusive departmental digital laboratory with sophisticated technology</rdfs:comment>
        <rdfs:label>DCF Lab</rdfs:label>
    </owl:NamedIndividual>
    


    <!-- http://www.semanticweb.org/suhaspai/ontologies/2021/4/UnivFAQ#EE3002 -->

    <owl:NamedIndividual rdf:about="http://www.semanticweb.org/suhaspai/ontologies/2021/4/UnivFAQ#EE3002">
        <rdf:type rdf:resource="http://www.semanticweb.org/suhaspai/ontologies/2021/4/UnivFAQ#Courses"/>
        <rdfs:comment>Learning objectives:This course is an introduction to amplifiers using transistors. Students will be introduced to MOS transistors, their characteristics, techniques for biasing them, and amplifiers using them. The basic transistor amplifier stages are seen as realizations of different controlled sources using negative feedback. Small- and large-signal characteristics of each amplifier will be discussed. Frequency ompensation techniques to stabilise higher order systems will be discussed.Learning Outcomes:At the end of this course, students should be able to recognize and analyze the basic amplifiers and biasing arrangements using MOS or bipolar transistors. Students should also be able to perform dominant-pole compensation of higher order systems and stabilise them.</rdfs:comment>
        <rdfs:label>Analog Circuits</rdfs:label>
    </owl:NamedIndividual>
    


    <!-- http://www.semanticweb.org/suhaspai/ontologies/2021/4/UnivFAQ#EE6112 -->

    <owl:NamedIndividual rdf:about="http://www.semanticweb.org/suhaspai/ontologies/2021/4/UnivFAQ#EE6112">
        <rdf:type rdf:resource="http://www.semanticweb.org/suhaspai/ontologies/2021/4/UnivFAQ#Courses"/>
        <rdfs:comment>This is proposed as an advanced graduate course, dealing predominantly with martingale techniques and concentration of probability measures, along with a few allied topics of interest in probability theory. Martingale and measure concentration techniques are becoming increasingly popular is various active areas of research, such as machine learning, resource allocation, complex networks, information theory and coding theory. It is hoped that this course would equip the students with the requisite familiarity and conceptual grasp to tackle various contemporary analysis and proof techniques.</rdfs:comment>
        <rdfs:label>Topics in Random Processes and Concentrations</rdfs:label>
    </owl:NamedIndividual>
    


    <!-- http://www.semanticweb.org/suhaspai/ontologies/2021/4/UnivFAQ#EE6150 -->

    <owl:NamedIndividual rdf:about="http://www.semanticweb.org/suhaspai/ontologies/2021/4/UnivFAQ#EE6150">
        <rdf:type rdf:resource="http://www.semanticweb.org/suhaspai/ontologies/2021/4/UnivFAQ#Courses"/>
        <rdfs:comment>A short tour through basics (not very measure theoretic) of axiomatic probability theory, convergence, and laws of large numbers. 2. Discrete time Markov chains: class properties, stationary distribution, hitting and mixing times, coupling, and applications to queues and social networks. 3. Renewal theory: elementary renewal theorem, Wald’s lemma, renewal reward theorem, and batch biasing (brief discussion on Key and Blackwell’s renewal theorem). 4. Poisson process. 5. Continuous time Markov chains: stationarity, time reversal, Kelly’s lemma, reversibility, and applications to social networks and queues. 6. (If time permits) Chernoff bound and introduction to large deviations; Martingales and concentration</rdfs:comment>
        <rdfs:label>Stochastic Modeling and the Theory of Queues</rdfs:label>
    </owl:NamedIndividual>
    


    <!-- http://www.semanticweb.org/suhaspai/ontologies/2021/4/UnivFAQ#Electrical_Engineering -->

    <owl:NamedIndividual rdf:about="http://www.semanticweb.org/suhaspai/ontologies/2021/4/UnivFAQ#Electrical_Engineering">
        <rdf:type rdf:resource="http://www.semanticweb.org/suhaspai/ontologies/2021/4/UnivFAQ#Department"/>
        <UnivFAQ:hasFacility rdf:resource="http://www.semanticweb.org/suhaspai/ontologies/2021/4/UnivFAQ#Microelectronics_and_MEMS_laboratory"/>
        <UnivFAQ:hasFacility rdf:resource="http://www.semanticweb.org/suhaspai/ontologies/2021/4/UnivFAQ#VLSI_Lab"/>
        <UnivFAQ:offers rdf:resource="http://www.semanticweb.org/suhaspai/ontologies/2021/4/UnivFAQ#EE3002"/>
        <UnivFAQ:offers rdf:resource="http://www.semanticweb.org/suhaspai/ontologies/2021/4/UnivFAQ#EE6112"/>
        <UnivFAQ:offers rdf:resource="http://www.semanticweb.org/suhaspai/ontologies/2021/4/UnivFAQ#EE6150"/>
        <rdfs:comment>The Electrical Engineering department was established in 1959. We currently have about 1000 students, 60 faculty members, 30 supporting staff members and 2 post-doctoral fellows with us.

We perform a variety of research work from absolute fundamentals to component design to system integration to deployment/commercialisation. We have strong industry interaction and have been involved in development of state-of-art products. We house extensive fabrication, calibration and testing facilities for carrying out academic projects, sponsored research and consultancy projects.</rdfs:comment>
        <rdfs:label>Electrical Engineering Department</rdfs:label>
    </owl:NamedIndividual>
    


    <!-- http://www.semanticweb.org/suhaspai/ontologies/2021/4/UnivFAQ#Information_Theory -->

    <owl:NamedIndividual rdf:about="http://www.semanticweb.org/suhaspai/ontologies/2021/4/UnivFAQ#Information_Theory">
        <rdf:type rdf:resource="http://www.semanticweb.org/suhaspai/ontologies/2021/4/UnivFAQ#ResearchFields"/>
        <rdfs:comment>Information theory is the scientific study of the quantification, storage, and communication of digital information.[1] The field was fundamentally established by the works of Harry Nyquist and Ralph Hartley, in the 1920s, and Claude Shannon in the 1940s. The field is at the intersection of probability theory, statistics, computer science, statistical mechanics, information engineering, and electrical engineering.</rdfs:comment>
        <rdfs:label>Information Theory</rdfs:label>
    </owl:NamedIndividual>
    


    <!-- http://www.semanticweb.org/suhaspai/ontologies/2021/4/UnivFAQ#JEE_Advanced -->

    <owl:NamedIndividual rdf:about="http://www.semanticweb.org/suhaspai/ontologies/2021/4/UnivFAQ#JEE_Advanced"/>
    


    <!-- http://www.semanticweb.org/suhaspai/ontologies/2021/4/UnivFAQ#JEE_Mains -->

    <owl:NamedIndividual rdf:about="http://www.semanticweb.org/suhaspai/ontologies/2021/4/UnivFAQ#JEE_Mains"/>
    


    <!-- http://www.semanticweb.org/suhaspai/ontologies/2021/4/UnivFAQ#Krishna_Jagannathan -->

    <owl:NamedIndividual rdf:about="http://www.semanticweb.org/suhaspai/ontologies/2021/4/UnivFAQ#Krishna_Jagannathan">
        <rdf:type rdf:resource="http://www.semanticweb.org/suhaspai/ontologies/2021/4/UnivFAQ#AssociateProfessor"/>
        <UnivFAQ:isSpecializedIn rdf:resource="http://www.semanticweb.org/suhaspai/ontologies/2021/4/UnivFAQ#Network_Control"/>
        <UnivFAQ:isSpecializedIn rdf:resource="http://www.semanticweb.org/suhaspai/ontologies/2021/4/UnivFAQ#Transportation_Networks"/>
        <UnivFAQ:teaches rdf:resource="http://www.semanticweb.org/suhaspai/ontologies/2021/4/UnivFAQ#EE6150"/>
        <UnivFAQ:name rdf:datatype="http://www.w3.org/2001/XMLSchema#string">Krishna Jagannathan</UnivFAQ:name>
        <rdfs:label rdf:datatype="http://www.w3.org/2001/XMLSchema#string">Krishna Jagannathan</rdfs:label>
    </owl:NamedIndividual>
    


    <!-- http://www.semanticweb.org/suhaspai/ontologies/2021/4/UnivFAQ#Machine_Learning -->

    <owl:NamedIndividual rdf:about="http://www.semanticweb.org/suhaspai/ontologies/2021/4/UnivFAQ#Machine_Learning">
        <rdf:type rdf:resource="http://www.semanticweb.org/suhaspai/ontologies/2021/4/UnivFAQ#ResearchFields"/>
        <rdfs:comment>Machine learning is the study of computer algorithms that can improve automatically through experience and by the use of data. It is seen as a part of artificial intelligence</rdfs:comment>
        <rdfs:label>Machine Learning</rdfs:label>
    </owl:NamedIndividual>
    


    <!-- http://www.semanticweb.org/suhaspai/ontologies/2021/4/UnivFAQ#Microelectronics_and_MEMS_laboratory -->

    <owl:NamedIndividual rdf:about="http://www.semanticweb.org/suhaspai/ontologies/2021/4/UnivFAQ#Microelectronics_and_MEMS_laboratory">
        <rdfs:comment>Microelectronics and MEMS Lab is well-equipped for semiconductor device and MEMS fabrication, characterization, modeling and simulation. It has Class-100 and Class-1000 clean rooms which house the major facilities that include a Mask writer, double-sided lithography facility, substrate bond aligner, LPCVD for polysilicon deposition, PECVD for dielectrics, diffusion furnaces, e-beam metallization unit and RIE for dry etching. DC and RF probe stations, parametric analyzer and LCR meter are used for electrical characterization, while a non-contact surface profiler and ellipsometer are used for process characterization. ATLAS, SenTaurus, Coventorware and Intellisuite are some of the commercial softwares used for simulation. The facilities have been used for fabrication and characterization of devices based on Silicon, GaAs and InP based materials, and for modeling various types of devices as listed below. Some activity has also been initiated on GaN and silicon based photonic devices. A wide array of devices, e.g. polysilicon gate n-channel MOSFETs, bipolar junction transistors, pressure sensors with integrated amplifiers, GaAs MESFETs, pigtailed InGaAs/InP PIN photodiodes and variable optical attenuators have been fabricated in the laboratory.</rdfs:comment>
        <rdfs:label>Microelectronics and MEMS laboratory</rdfs:label>
    </owl:NamedIndividual>
    


    <!-- http://www.semanticweb.org/suhaspai/ontologies/2021/4/UnivFAQ#N_S_Narayanaswamy -->

    <owl:NamedIndividual rdf:about="http://www.semanticweb.org/suhaspai/ontologies/2021/4/UnivFAQ#N_S_Narayanaswamy">
        <rdf:type rdf:resource="http://www.semanticweb.org/suhaspai/ontologies/2021/4/UnivFAQ#Professor"/>
        <UnivFAQ:isSpecializedIn rdf:resource="http://www.semanticweb.org/suhaspai/ontologies/2021/4/UnivFAQ#Artificial_Intelligence"/>
        <UnivFAQ:teaches rdf:resource="http://www.semanticweb.org/suhaspai/ontologies/2021/4/UnivFAQ#CS1200"/>
        <UnivFAQ:name rdf:datatype="http://www.w3.org/2001/XMLSchema#string">N.S. Narayanaswamy</UnivFAQ:name>
        <rdfs:label rdf:datatype="http://www.w3.org/2001/XMLSchema#string">N.S. Narayanaswamy</rdfs:label>
    </owl:NamedIndividual>
    


    <!-- http://www.semanticweb.org/suhaspai/ontologies/2021/4/UnivFAQ#Network_Control -->

    <owl:NamedIndividual rdf:about="http://www.semanticweb.org/suhaspai/ontologies/2021/4/UnivFAQ#Network_Control">
        <rdf:type rdf:resource="http://www.semanticweb.org/suhaspai/ontologies/2021/4/UnivFAQ#ResearchFields"/>
        <rdfs:comment>A Networked Control System (NCS) is a control system wherein the control loops are closed through a communication network. The defining feature of an NCS is that control and feedback signals are exchanged among the system&apos;s components in the form of information packages through a network.</rdfs:comment>
        <rdfs:label>Network Control</rdfs:label>
    </owl:NamedIndividual>
    


    <!-- http://www.semanticweb.org/suhaspai/ontologies/2021/4/UnivFAQ#Ontologies_and_Application -->

    <owl:NamedIndividual rdf:about="http://www.semanticweb.org/suhaspai/ontologies/2021/4/UnivFAQ#Ontologies_and_Application">
        <rdf:type rdf:resource="http://www.semanticweb.org/suhaspai/ontologies/2021/4/UnivFAQ#ResearchFields"/>
        <rdfs:comment>An ontology is the specification of conceptualizations, used to help programs and humans share knowledge. An Ontology is a formal and explicit specification of a shared conceptualization.</rdfs:comment>
        <rdfs:label>Ontologies and Applications</rdfs:label>
    </owl:NamedIndividual>
    


    <!-- http://www.semanticweb.org/suhaspai/ontologies/2021/4/UnivFAQ#PACE_Lab -->

    <owl:NamedIndividual rdf:about="http://www.semanticweb.org/suhaspai/ontologies/2021/4/UnivFAQ#PACE_Lab">
        <rdf:type rdf:resource="http://www.semanticweb.org/suhaspai/ontologies/2021/4/UnivFAQ#InstituteFacilities"/>
        <rdfs:comment>Programming Languages, Architecture and Compilers Education Laboratory</rdfs:comment>
        <rdfs:label>PACE Lab</rdfs:label>
    </owl:NamedIndividual>
    


    <!-- http://www.semanticweb.org/suhaspai/ontologies/2021/4/UnivFAQ#RFIC_Design -->

    <owl:NamedIndividual rdf:about="http://www.semanticweb.org/suhaspai/ontologies/2021/4/UnivFAQ#RFIC_Design">
        <rdf:type rdf:resource="http://www.semanticweb.org/suhaspai/ontologies/2021/4/UnivFAQ#ResearchFields"/>
        <rdfs:comment>RF IC design, much like niche areas of analog IC design, is often a custom process that is aided by one, or often, many EDA tools. Part of the precise nature of RF IC design is that parasitics and packaging characteristics have first-order impact on the performance of RF circuits. Therefore, RF IC design is often an iterative process that involves the extensive use of EM simulation, parasitic modeling, and package modeling throughout the IC design process.</rdfs:comment>
        <rdfs:label>RFIC Design</rdfs:label>
    </owl:NamedIndividual>
    


    <!-- http://www.semanticweb.org/suhaspai/ontologies/2021/4/UnivFAQ#Reinforcement_Learning -->

    <owl:NamedIndividual rdf:about="http://www.semanticweb.org/suhaspai/ontologies/2021/4/UnivFAQ#Reinforcement_Learning">
        <rdf:type rdf:resource="http://www.semanticweb.org/suhaspai/ontologies/2021/4/UnivFAQ#ResearchFields"/>
        <rdfs:label>Reinforcement Learning</rdfs:label>
    </owl:NamedIndividual>
    


    <!-- http://www.semanticweb.org/suhaspai/ontologies/2021/4/UnivFAQ#Rupesh_Nasre -->

    <owl:NamedIndividual rdf:about="http://www.semanticweb.org/suhaspai/ontologies/2021/4/UnivFAQ#Rupesh_Nasre">
        <rdf:type rdf:resource="http://www.semanticweb.org/suhaspai/ontologies/2021/4/UnivFAQ#AssociateProfessor"/>
        <UnivFAQ:isSpecializedIn rdf:resource="http://www.semanticweb.org/suhaspai/ontologies/2021/4/UnivFAQ#Compilers"/>
        <UnivFAQ:teaches rdf:resource="http://www.semanticweb.org/suhaspai/ontologies/2021/4/UnivFAQ#CS6023"/>
        <UnivFAQ:name rdf:datatype="http://www.w3.org/2001/XMLSchema#string">Rupesh Nasre</UnivFAQ:name>
        <rdfs:label rdf:datatype="http://www.w3.org/2001/XMLSchema#string">Rupesh Nasre</rdfs:label>
    </owl:NamedIndividual>
    


    <!-- http://www.semanticweb.org/suhaspai/ontologies/2021/4/UnivFAQ#S_Aniruddhan -->

    <owl:NamedIndividual rdf:about="http://www.semanticweb.org/suhaspai/ontologies/2021/4/UnivFAQ#S_Aniruddhan">
        <rdf:type rdf:resource="http://www.semanticweb.org/suhaspai/ontologies/2021/4/UnivFAQ#AssociateProfessor"/>
        <UnivFAQ:isSpecializedIn rdf:resource="http://www.semanticweb.org/suhaspai/ontologies/2021/4/UnivFAQ#Analog"/>
        <UnivFAQ:isSpecializedIn rdf:resource="http://www.semanticweb.org/suhaspai/ontologies/2021/4/UnivFAQ#RFIC_Design"/>
        <UnivFAQ:teaches rdf:resource="http://www.semanticweb.org/suhaspai/ontologies/2021/4/UnivFAQ#EE3002"/>
        <UnivFAQ:name rdf:datatype="http://www.w3.org/2001/XMLSchema#string">S Aniruddhan</UnivFAQ:name>
        <rdfs:label rdf:datatype="http://www.w3.org/2001/XMLSchema#string">S Aniruddhan</rdfs:label>
    </owl:NamedIndividual>
    


    <!-- http://www.semanticweb.org/suhaspai/ontologies/2021/4/UnivFAQ#Scholarship_1 -->

    <owl:NamedIndividual rdf:about="http://www.semanticweb.org/suhaspai/ontologies/2021/4/UnivFAQ#Scholarship_1"/>
    


    <!-- http://www.semanticweb.org/suhaspai/ontologies/2021/4/UnivFAQ#Shweta_Agarwal -->

    <owl:NamedIndividual rdf:about="http://www.semanticweb.org/suhaspai/ontologies/2021/4/UnivFAQ#Shweta_Agarwal">
        <rdf:type rdf:resource="http://www.semanticweb.org/suhaspai/ontologies/2021/4/UnivFAQ#AssociateProfessor"/>
        <UnivFAQ:teaches rdf:resource="http://www.semanticweb.org/suhaspai/ontologies/2021/4/UnivFAQ#CS2800"/>
        <UnivFAQ:name rdf:datatype="http://www.w3.org/2001/XMLSchema#string">Shweta Agarwal</UnivFAQ:name>
        <rdfs:comment>Cryptography, or cryptology, is the practice and study of techniques for secure communication in the presence of adversarial behavior.</rdfs:comment>
        <rdfs:label rdf:datatype="http://www.w3.org/2001/XMLSchema#string">Shweta Agarwal</rdfs:label>
    </owl:NamedIndividual>
    


    <!-- http://www.semanticweb.org/suhaspai/ontologies/2021/4/UnivFAQ#Sreenivasa_Kumar -->

    <owl:NamedIndividual rdf:about="http://www.semanticweb.org/suhaspai/ontologies/2021/4/UnivFAQ#Sreenivasa_Kumar">
        <rdf:type rdf:resource="http://www.semanticweb.org/suhaspai/ontologies/2021/4/UnivFAQ#Professor"/>
        <UnivFAQ:isSpecializedIn rdf:resource="http://www.semanticweb.org/suhaspai/ontologies/2021/4/UnivFAQ#Ontologies_and_Application"/>
        <UnivFAQ:teaches rdf:resource="http://www.semanticweb.org/suhaspai/ontologies/2021/4/UnivFAQ#CS3700"/>
        <UnivFAQ:teaches rdf:resource="http://www.semanticweb.org/suhaspai/ontologies/2021/4/UnivFAQ#CS6852"/>
        <UnivFAQ:name rdf:datatype="http://www.w3.org/2001/XMLSchema#string">P Sreenivasa Kumar</UnivFAQ:name>
        <rdfs:label rdf:datatype="http://www.w3.org/2001/XMLSchema#string">P Sreenivasa Kumar</rdfs:label>
    </owl:NamedIndividual>
    


    <!-- http://www.semanticweb.org/suhaspai/ontologies/2021/4/UnivFAQ#Transportation_Networks -->

    <owl:NamedIndividual rdf:about="http://www.semanticweb.org/suhaspai/ontologies/2021/4/UnivFAQ#Transportation_Networks">
        <rdf:type rdf:resource="http://www.semanticweb.org/suhaspai/ontologies/2021/4/UnivFAQ#ResearchFields"/>
        <rdfs:comment>A transport network, or transportation network is a network or graph in geographic space, describing an infrastructure that permits and constrains movement or flow. Examples include but are not limited to road networks, railways, air routes, pipelines, aqueducts, and power lines</rdfs:comment>
        <rdfs:label>Transportation Networks</rdfs:label>
    </owl:NamedIndividual>
    


    <!-- http://www.semanticweb.org/suhaspai/ontologies/2021/4/UnivFAQ#VLSI_Lab -->

    <owl:NamedIndividual rdf:about="http://www.semanticweb.org/suhaspai/ontologies/2021/4/UnivFAQ#VLSI_Lab">
        <rdf:type rdf:resource="http://www.semanticweb.org/suhaspai/ontologies/2021/4/UnivFAQ#InstituteFacilities"/>
        <rdfs:comment>Involved in research in the areas of analog, mixed signal, and RF design, analysis and simulation of noise in circuits, VLSI DSP architectures, Programmable Analog Pulse Shaping for Ultra-Wideband Applications and reconfigurable computing.</rdfs:comment>
        <rdfs:label>VLSI Lab</rdfs:label>
    </owl:NamedIndividual>
    


    <!-- 
    ///////////////////////////////////////////////////////////////////////////////////////
    //
    // Annotations
    //
    ///////////////////////////////////////////////////////////////////////////////////////
     -->

    <rdf:Description rdf:about="http://www.semanticweb.org/suhaspai/ontologies/2021/4/UnivFAQ#CS3205">
        <rdfs:comment>Concepts and implementation of computer networks; architecture, protocol layers, inter-networking and addressing; network application development.</rdfs:comment>
        <rdfs:label>Introduction to Computer Networks</rdfs:label>
    </rdf:Description>
</rdf:RDF>



<!-- Generated by the OWL API (version 4.5.9.2019-02-01T07:24:44Z) https://github.com/owlcs/owlapi -->

